@prefix app: <https://www.opengis.net/ont/citygml/appearance/> .
@prefix core: <https://www.opengis.net/ont/citygml/core/> .
@prefix gmlowl: <http://www.opengis.net/ont/gml#> .
@prefix iso19111-2007: <http://def.isotc211.org/iso19111/2007/CoordinateReferenceSystems#> .
@prefix iso19150-2: <http://def.isotc211.org/iso19150/-2/2012/base#> .
@prefix owl: <http://www.w3.org/2002/07/owl#> .
@prefix rdf: <http://www.w3.org/1999/02/22-rdf-syntax-ns#> .
@prefix rdfs: <http://www.w3.org/2000/01/rdf-schema#> .
@prefix schema: <https://schema.org/> .
@prefix skos: <http://www.w3.org/2004/02/skos/core#> .
@prefix xsd: <http://www.w3.org/2001/XMLSchema#> .

<https://www.opengis.net/ont/citygml/appearance> a owl:Ontology ;
    rdfs:label "Appearance"@en ;
    owl:imports <http://def.isotc211.org/iso19150/-2/2012/base>,
        <http://www.opengis.net/ont/gml>,
        <https://www.opengis.net/ont/citygml/common>,
        <https://www.opengis.net/ont/citygml/core> ;
    owl:versionIRI <https://www.opengis.net/ont/citygml/appearance/3.0.0/> ;
    owl:versionInfo "3.0.0" ;
    skos:definition "The Appearance module supports the modelling of the observable surface properties of CityGML features in the form of textures and material."@en .

app:Appearance a owl:Class ;
    rdfs:label "Appearance"@en ;
    rdfs:subClassOf [ a owl:Restriction ;
            owl:allValuesFrom app:AbstractSurfaceData ;
            owl:onProperty app:surfaceData ],
        [ a owl:Restriction ;
            owl:allValuesFrom xsd:string ;
            owl:onProperty app:theme ],
        [ a owl:Restriction ;
            owl:maxQualifiedCardinality "1"^^xsd:nonNegativeInteger ;
            owl:onDataRange xsd:string ;
            owl:onProperty app:theme ],
        core:AbstractAppearance .

app:GeoreferencedTexture a owl:Class ;
    rdfs:label "GeoreferencedTexture"@en ;
    rdfs:subClassOf [ a owl:Restriction ;
            owl:allValuesFrom xsd:anyURI ;
            owl:onProperty app:target ],
        [ a owl:Restriction ;
            owl:allValuesFrom xsd:boolean ;
            owl:onProperty app:preferWorldFile ],
        [ a owl:Restriction ;
            owl:allValuesFrom gmlowl:Point ;
            owl:onProperty <https://www.opengis.net/ont/citygml/common/referencePoint> ],
        [ a owl:Restriction ;
            owl:maxQualifiedCardinality "1"^^xsd:nonNegativeInteger ;
            owl:onClass gmlowl:Point ;
            owl:onProperty <https://www.opengis.net/ont/citygml/common/referencePoint> ],
        [ a owl:Restriction ;
            owl:maxQualifiedCardinality "1"^^xsd:nonNegativeInteger ;
            owl:onClass core:TransformationMatrix2x2 ;
            owl:onProperty app:orientation ],
        [ a owl:Restriction ;
            owl:allValuesFrom core:TransformationMatrix2x2 ;
            owl:onProperty app:orientation ],
        [ a owl:Restriction ;
            owl:maxQualifiedCardinality "1"^^xsd:nonNegativeInteger ;
            owl:onDataRange xsd:boolean ;
            owl:onProperty app:preferWorldFile ],
        app:AbstractTexture ;
    owl:disjointWith app:ParameterizedTexture .

app:TexCoordGen a owl:Class ;
    rdfs:label "TexCoordGen"@en ;
    rdfs:subClassOf [ a owl:Restriction ;
            owl:allValuesFrom iso19111-2007:SC_CRS ;
            owl:onProperty app:crs ],
        [ a owl:Restriction ;
            owl:maxQualifiedCardinality "1"^^xsd:nonNegativeInteger ;
            owl:onClass iso19111-2007:SC_CRS ;
            owl:onProperty app:crs ],
        [ a owl:Restriction ;
            owl:allValuesFrom core:TransformationMatrix3x4 ;
            owl:onProperty app:worldToTexture ],
        [ a owl:Restriction ;
            owl:onClass core:TransformationMatrix3x4 ;
            owl:onProperty app:worldToTexture ;
            owl:qualifiedCardinality "1"^^xsd:nonNegativeInteger ],
        app:AbstractTextureParameterization ;
    owl:disjointWith app:TexCoordList ;
    skos:definition "TexCoordGen defines texture parameterization using a transformation matrix."@en .

app:TexCoordList a owl:Class ;
    rdfs:label "TexCoordList"@en ;
    rdfs:subClassOf [ a owl:Restriction ;
            owl:allValuesFrom core:DoubleList ;
            owl:onProperty app:textureCoordinates ],
        [ a owl:Restriction ;
            owl:minQualifiedCardinality "1"^^xsd:nonNegativeInteger ;
            owl:onClass core:DoubleList ;
            owl:onProperty app:textureCoordinates ],
        [ a owl:Restriction ;
            owl:allValuesFrom xsd:anyURI ;
            owl:onProperty app:ring ],
        [ a owl:Restriction ;
            owl:minQualifiedCardinality "1"^^xsd:nonNegativeInteger ;
            owl:onDataRange xsd:anyURI ;
            owl:onProperty app:ring ],
        app:AbstractTextureParameterization ;
    skos:definition "TexCoordList defines texture parameterization using texture coordinates."@en .

app:X3DMaterial a owl:Class ;
    rdfs:label "X3DMaterial"@en ;
    rdfs:subClassOf [ a owl:Restriction ;
            owl:maxQualifiedCardinality "1"^^xsd:nonNegativeInteger ;
            owl:onClass core:DoubleBetween0and1 ;
            owl:onProperty app:ambientIntensity ],
        [ a owl:Restriction ;
            owl:maxQualifiedCardinality "1"^^xsd:nonNegativeInteger ;
            owl:onClass app:Color ;
            owl:onProperty app:diffuseColor ],
        [ a owl:Restriction ;
            owl:allValuesFrom core:DoubleBetween0and1 ;
            owl:onProperty app:ambientIntensity ],
        [ a owl:Restriction ;
            owl:allValuesFrom xsd:anyURI ;
            owl:onProperty app:target ],
        [ a owl:Restriction ;
            owl:maxQualifiedCardinality "1"^^xsd:nonNegativeInteger ;
            owl:onDataRange xsd:boolean ;
            owl:onProperty app:isSmooth ],
        [ a owl:Restriction ;
            owl:allValuesFrom core:DoubleBetween0and1 ;
            owl:onProperty app:shininess ],
        [ a owl:Restriction ;
            owl:allValuesFrom app:Color ;
            owl:onProperty app:diffuseColor ],
        [ a owl:Restriction ;
            owl:allValuesFrom app:Color ;
            owl:onProperty app:emissiveColor ],
        [ a owl:Restriction ;
            owl:maxQualifiedCardinality "1"^^xsd:nonNegativeInteger ;
            owl:onClass app:Color ;
            owl:onProperty app:specularColor ],
        [ a owl:Restriction ;
            owl:maxQualifiedCardinality "1"^^xsd:nonNegativeInteger ;
            owl:onClass app:Color ;
            owl:onProperty app:emissiveColor ],
        [ a owl:Restriction ;
            owl:maxQualifiedCardinality "1"^^xsd:nonNegativeInteger ;
            owl:onClass core:DoubleBetween0and1 ;
            owl:onProperty app:transparency ],
        [ a owl:Restriction ;
            owl:maxQualifiedCardinality "1"^^xsd:nonNegativeInteger ;
            owl:onClass core:DoubleBetween0and1 ;
            owl:onProperty app:shininess ],
        [ a owl:Restriction ;
            owl:allValuesFrom xsd:boolean ;
            owl:onProperty app:isSmooth ],
        [ a owl:Restriction ;
            owl:allValuesFrom core:DoubleBetween0and1 ;
            owl:onProperty app:transparency ],
        [ a owl:Restriction ;
            owl:allValuesFrom app:Color ;
            owl:onProperty app:specularColor ],
        app:AbstractSurfaceData .

app:surfaceData a owl:ObjectProperty ;
    rdfs:label "surfaceData"@en ;
    rdfs:domain app:Appearance ;
    rdfs:range app:AbstractSurfaceData ;
    skos:definition "Relates to the surface data that are part of the Appearance."@en .

app:AbstractTexture a owl:Class ;
    rdfs:label "AbstractTexture"@en ;
    iso19150-2:isAbstract true ;
    rdfs:subClassOf [ a owl:Restriction ;
            owl:allValuesFrom core:MimeTypeValue ;
            owl:onProperty <https://www.opengis.net/ont/citygml/common/mimeType> ],
        [ a owl:Restriction ;
            owl:maxQualifiedCardinality "1"^^xsd:nonNegativeInteger ;
            owl:onClass app:ColorPlusOpacity ;
            owl:onProperty app:borderColor ],
        [ a owl:Restriction ;
            owl:maxQualifiedCardinality "1"^^xsd:nonNegativeInteger ;
            owl:onDataRange app:WrapMode ;
            owl:onProperty app:wrapMode ],
        [ a owl:Restriction ;
            owl:allValuesFrom app:ColorPlusOpacity ;
            owl:onProperty app:borderColor ],
        [ a owl:Restriction ;
            owl:maxQualifiedCardinality "1"^^xsd:nonNegativeInteger ;
            owl:onClass core:MimeTypeValue ;
            owl:onProperty <https://www.opengis.net/ont/citygml/common/mimeType> ],
        [ a owl:Restriction ;
            owl:allValuesFrom app:WrapMode ;
            owl:onProperty app:wrapMode ],
        [ a owl:Restriction ;
            owl:allValuesFrom xsd:anyURI ;
            owl:onProperty app:imageURI ],
        [ a owl:Restriction ;
            owl:maxQualifiedCardinality "1"^^xsd:nonNegativeInteger ;
            owl:onDataRange app:TextureType ;
            owl:onProperty app:textureType ],
        [ a owl:Restriction ;
            owl:allValuesFrom app:TextureType ;
            owl:onProperty app:textureType ],
        [ a owl:Restriction ;
            owl:onDataRange xsd:anyURI ;
            owl:onProperty app:imageURI ;
            owl:qualifiedCardinality "1"^^xsd:nonNegativeInteger ],
        app:AbstractSurfaceData ;
    owl:disjointWith app:X3DMaterial .

app:ParameterizedTexture a owl:Class ;
    rdfs:label "ParameterizedTexture"@en ;
    rdfs:subClassOf [ a owl:Restriction ;
            owl:allValuesFrom app:TextureAssociation ;
            owl:onProperty <https://www.opengis.net/ont/citygml/common/textureParameterization> ],
        app:AbstractTexture .

app:ambientIntensity a owl:ObjectProperty ;
    rdfs:label "ambientIntensity"@en ;
    rdfs:range core:DoubleBetween0and1 ;
    skos:definition "Specifies the minimum percentage of diffuseColor that is visible regardless of light sources."@en .

app:borderColor a owl:ObjectProperty ;
    rdfs:label "borderColor"@en ;
    rdfs:range app:ColorPlusOpacity ;
    skos:definition "Specifies the color of that part of the surface that is not covered by the texture."@en .

app:crs a owl:ObjectProperty ;
    rdfs:label "crs"@en ;
    rdfs:domain app:TexCoordGen ;
    rdfs:range iso19111-2007:SC_CRS ;
    skos:definition "Relates to the coordinate reference system of the transformation matrix."@en .

app:diffuseColor a owl:ObjectProperty ;
    rdfs:label "diffuseColor"@en ;
    rdfs:range app:Color ;
    skos:definition "Specifies the color of the light diffusely reflected by the surface geometry object."@en .

app:emissiveColor a owl:ObjectProperty ;
    rdfs:label "emissiveColor"@en ;
    rdfs:range app:Color ;
    skos:definition "Specifies the color of the light emitted by the surface geometry object."@en .

app:imageURI a owl:DatatypeProperty ;
    rdfs:label "imageURI"@en ;
    rdfs:range xsd:anyURI ;
    skos:definition "Specifies the URI that points to the external image data file."@en .

app:isFront a owl:DatatypeProperty ;
    rdfs:label "isFront"@en ;
    rdfs:range xsd:boolean ;
    skos:definition "Indicates whether the texture or material is assigned to the front side or the back side of the surface geometry object."@en .

app:isSmooth a owl:DatatypeProperty ;
    rdfs:label "isSmooth"@en ;
    rdfs:range xsd:boolean ;
    skos:definition "Specifies which interpolation method is used for the shading of the surface geometry object. If the attribute is set to true, vertex normals should be used for shading (Gouraud shading). Otherwise, normals should be constant for a surface patch (flat shading)."@en .

app:orientation a owl:ObjectProperty ;
    rdfs:label "orientation"@en ;
    rdfs:range core:TransformationMatrix2x2 ;
    skos:definition "Specifies the rotation and scaling of the image in form of a 2x2 matrix."@en .

app:preferWorldFile a owl:DatatypeProperty ;
    rdfs:label "preferWorldFile"@en ;
    rdfs:range xsd:boolean ;
    skos:definition "Indicates whether the georeference from the image file or the accompanying world file should be preferred."@en .

app:ring a owl:DatatypeProperty ;
    rdfs:label "ring"@en ;
    rdfs:range xsd:anyURI ;
    skos:definition "Specifies the URIs that point to the LinearRings that are parameterized using the given texture coordinates."@en .

app:shininess a owl:ObjectProperty ;
    rdfs:label "shininess"@en ;
    rdfs:range core:DoubleBetween0and1 ;
    skos:definition "Specifies the sharpness of the specular highlight."@en .

app:specularColor a owl:ObjectProperty ;
    rdfs:label "specularColor"@en ;
    rdfs:range app:Color ;
    skos:definition "Specifies the color of the light directly reflected by the surface geometry object."@en .

app:textureCoordinates a owl:ObjectProperty ;
    rdfs:label "textureCoordinates"@en ;
    rdfs:range core:DoubleList ;
    skos:definition "Specifies the coordinates of texture used for parameterization. The texture coordinates are provided separately for each LinearRing of the surface geometry object."@en .

app:textureType a owl:DatatypeProperty ;
    rdfs:label "textureType"@en ;
    rdfs:range app:TextureType ;
    skos:definition "Indicates the specific type of the texture."@en .

app:theme a owl:DatatypeProperty ;
    rdfs:label "theme"@en ;
    rdfs:range xsd:string ;
    skos:definition "Specifies the topic of the Appearance. Each Appearance contains surface data for one theme only. Examples of themes are infrared radiation, noise pollution, or earthquake-induced structural stress."@en .

app:transparency a owl:ObjectProperty ;
    rdfs:label "transparency"@en ;
    rdfs:range core:DoubleBetween0and1 ;
    skos:definition "Specifies the degree of transparency of the surface geometry object."@en .

app:worldToTexture a owl:ObjectProperty ;
    rdfs:label "worldToTexture"@en ;
    rdfs:range core:TransformationMatrix3x4 ;
    skos:definition "Specifies the 3x4 transformation matrix that defines the transformation between world coordinates and texture coordinates."@en .

app:wrapMode a owl:DatatypeProperty ;
    rdfs:label "wrapMode"@en ;
    rdfs:range app:WrapMode ;
    skos:definition "Specifies the behaviour of the texture when the texture is smaller than the surface to which it is applied."@en .

<https://www.opengis.net/ont/citygml/common/mimeType> rdfs:label "mimeType"@en ;
    skos:definition "Specifies the MIME type of the external point cloud file."@en ;
    schema:rangeIncludes core:MimeTypeValue .

<https://www.opengis.net/ont/citygml/common/referencePoint> skos:definition "Relates to the 2D Point geometry that represents the center of the upper left image pixel in world space."@en ;
    schema:domainIncludes app:GeoreferencedTexture ;
    schema:rangeIncludes gmlowl:Point .

app:TextureAssociation a owl:Class ;
    rdfs:label "TextureAssociation"@en ;
    rdfs:subClassOf [ a owl:Restriction ;
            owl:allValuesFrom app:AbstractTextureParameterization ;
            owl:onProperty <https://www.opengis.net/ont/citygml/common/textureParameterization> ],
        [ a owl:Restriction ;
            owl:onClass app:AbstractTextureParameterization ;
            owl:onProperty <https://www.opengis.net/ont/citygml/common/textureParameterization> ;
            owl:qualifiedCardinality "1"^^xsd:nonNegativeInteger ],
        [ a owl:Restriction ;
            owl:allValuesFrom xsd:anyURI ;
            owl:onProperty app:target ],
        [ a owl:Restriction ;
            owl:onDataRange xsd:anyURI ;
            owl:onProperty app:target ;
            owl:qualifiedCardinality "1"^^xsd:nonNegativeInteger ] ;
    skos:definition "TextureAssociation denotes the relation of a texture to a surface geometry object."@en .

app:TextureType a rdfs:Datatype ;
    rdfs:label "TextureType"@en ;
    owl:equivalentClass [ a rdfs:Datatype ;
            owl:oneOf ( "specific" "typical" "unknown" ) ] ;
    skos:definition "TextureType enumerates the different texture types."@en .

app:WrapMode a rdfs:Datatype ;
    rdfs:label "WrapMode"@en ;
    owl:equivalentClass [ a rdfs:Datatype ;
            owl:oneOf ( "none" "wrap" "mirror" "clamp" "border" ) ] ;
    skos:definition "WrapMode enumerates the different fill modes for textures."@en .

<https://www.opengis.net/ont/citygml/common/textureParameterization> skos:definition "Relates to the texture coordinates or transformation matrices used for parameterization."@en ;
    schema:domainIncludes app:ParameterizedTexture,
        app:TextureAssociation ;
    schema:rangeIncludes app:AbstractTextureParameterization,
        app:TextureAssociation .

app:AbstractSurfaceData a owl:Class ;
    rdfs:label "AbstractSurfaceData"@en ;
    iso19150-2:isAbstract true ;
    rdfs:subClassOf [ a owl:Restriction ;
            owl:allValuesFrom xsd:boolean ;
            owl:onProperty app:isFront ],
        [ a owl:Restriction ;
            owl:maxQualifiedCardinality "1"^^xsd:nonNegativeInteger ;
            owl:onDataRange xsd:boolean ;
            owl:onProperty app:isFront ],
        core:AbstractFeature .

app:ColorPlusOpacity a owl:Class ;
    rdfs:label "ColorPlusOpacity"@en ;
    rdfs:subClassOf core:DoubleBetween0and1List ;
    skos:definition "Color is a list of four double values between 0 and 1 defining an RGBA color value. Opacity value of 0 means transparent."@en .

app:target a owl:DatatypeProperty ;
    rdfs:label "target"@en ;
    rdfs:range xsd:anyURI ;
    skos:definition "Specifies the URI that points to the surface geometry objects to which the texture is applied."@en .

app:AbstractTextureParameterization a owl:Class ;
    rdfs:label "AbstractTextureParameterization"@en ;
    iso19150-2:isAbstract true ;
    skos:definition "AbstractTextureParameterization is the abstract superclass for different kinds of texture parameterizations."@en .

app:Color a owl:Class ;
    rdfs:label "Color"@en ;
    rdfs:subClassOf core:DoubleBetween0and1List ;
    owl:disjointWith app:ColorPlusOpacity ;
    skos:definition "Color is a list of three double values between 0 and 1 defining an RGB color value."@en .

@prefix brid: <https://www.opengis.net/ont/citygml/bridge/> .
@prefix con: <https://www.opengis.net/ont/citygml/construction/> .
@prefix core: <https://www.opengis.net/ont/citygml/core/> .
@prefix iso19150-2: <http://def.isotc211.org/iso19150/-2/2012/base#> .
@prefix owl: <http://www.w3.org/2002/07/owl#> .
@prefix rdfs: <http://www.w3.org/2000/01/rdf-schema#> .
@prefix schema: <https://schema.org/> .
@prefix skos: <http://www.w3.org/2004/02/skos/core#> .
@prefix xsd: <http://www.w3.org/2001/XMLSchema#> .

<https://www.opengis.net/ont/citygml/bridge> a owl:Ontology ;
    rdfs:label "Bridge"@en ;
    owl:imports <http://def.isotc211.org/iso19150/-2/2012/base>,
        <https://www.opengis.net/ont/citygml/common>,
        <https://www.opengis.net/ont/citygml/construction>,
        <https://www.opengis.net/ont/citygml/core> ;
    owl:versionIRI <https://www.opengis.net/ont/citygml/bridge/3.0.0/> ;
    owl:versionInfo "3.0.0" ;
    skos:definition "The Bridge module supports representation of thematic and spatial aspects of bridges, bridge parts, bridge installations, and interior bridge structures."@en .

brid:BridgeClassValue a owl:Class ;
    rdfs:label "BridgeClassValue"@en ;
    rdfs:subClassOf skos:Concept ;
    skos:definition "BridgeClassValue is a code list used to further classify a Bridge."@en .

brid:BridgeFunctionValue a owl:Class ;
    rdfs:label "BridgeFunctionValue"@en ;
    rdfs:subClassOf skos:Concept ;
    skos:definition "BridgeFunctionValue is a code list that enumerates the different purposes of a Bridge."@en .

brid:BridgeFurnitureClassValue a owl:Class ;
    rdfs:label "BridgeFurnitureClassValue"@en ;
    rdfs:subClassOf skos:Concept ;
    skos:definition "BridgeFurnitureClassValue is a code list used to further classify a BridgeFurniture."@en .

brid:BridgeFurnitureFunctionValue a owl:Class ;
    rdfs:label "BridgeFurnitureFunctionValue"@en ;
    rdfs:subClassOf skos:Concept ;
    skos:definition "BridgeFurnitureFunctionValue is a code list that enumerates the different purposes of a BridgeFurniture."@en .

brid:BridgeFurnitureUsageValue a owl:Class ;
    rdfs:label "BridgeFurnitureUsageValue"@en ;
    rdfs:subClassOf skos:Concept ;
    skos:definition "BridgeFurnitureUsageValue is a code list that enumerates the different uses of a BridgeFurniture."@en .

brid:BridgeInstallationClassValue a owl:Class ;
    rdfs:label "BridgeInstallationClassValue"@en ;
    rdfs:subClassOf skos:Concept ;
    skos:definition "BridgeInstallationClassValue is a code list used to further classify a BridgeInstallation."@en .

brid:BridgeInstallationFunctionValue a owl:Class ;
    rdfs:label "BridgeInstallationFunctionValue"@en ;
    rdfs:subClassOf skos:Concept ;
    skos:definition "BridgeInstallationFunctionValue is a code list that enumerates the different purposes of a BridgeInstallation."@en .

brid:BridgeInstallationUsageValue a owl:Class ;
    rdfs:label "BridgeInstallationUsageValue"@en ;
    rdfs:subClassOf skos:Concept ;
    skos:definition "BridgeInstallationUsageValue is a code list that enumerates the different uses of a BridgeInstallation."@en .

brid:BridgeRoomClassValue a owl:Class ;
    rdfs:label "BridgeRoomClassValue"@en ;
    rdfs:subClassOf skos:Concept ;
    skos:definition "BridgeRoomClassValue is a code list used to further classify a BridgeRoom."@en .

brid:BridgeRoomFunctionValue a owl:Class ;
    rdfs:label "BridgeRoomFunctionValue"@en ;
    rdfs:subClassOf skos:Concept ;
    skos:definition "BridgeRoomFunctionValue is a code list that enumerates the different purposes of a BridgeRoom."@en .

brid:BridgeRoomUsageValue a owl:Class ;
    rdfs:label "BridgeRoomUsageValue"@en ;
    rdfs:subClassOf skos:Concept ;
    skos:definition "BridgeRoomUsageValue is a code list that enumerates the different uses of a BridgeRoom."@en .

brid:BridgeUsageValue a owl:Class ;
    rdfs:label "BridgeUsageValue"@en ;
    rdfs:subClassOf skos:Concept ;
    skos:definition "BridgeUsageValue is a code list that enumerates the different uses of a Bridge."@en .

brid:Bridge a owl:Class ;
    rdfs:label "Bridge"@en ;
    rdfs:subClassOf [ a owl:Restriction ;
            owl:allValuesFrom brid:BridgePart ;
            owl:onProperty brid:bridgePart ],
        brid:AbstractBridge ;
    owl:disjointWith brid:BridgePart .

brid:bridgeConstructiveElement a owl:ObjectProperty ;
    rdfs:label "bridgeConstructiveElement"@en ;
    rdfs:domain brid:AbstractBridge ;
    rdfs:range brid:BridgeConstructiveElement ;
    skos:definition "Relates the constructive elements to the Bridge or BridgePart."@en .

brid:bridgePart a owl:ObjectProperty ;
    rdfs:label "bridgePart"@en ;
    rdfs:domain brid:Bridge ;
    rdfs:range brid:BridgePart ;
    skos:definition "Relates the bridge parts to the Bridge."@en .

brid:bridgeRoom a owl:ObjectProperty ;
    rdfs:label "bridgeRoom"@en ;
    rdfs:domain brid:AbstractBridge ;
    rdfs:range brid:BridgeRoom ;
    skos:definition "Relates the rooms to the Bridge or BridgePart."@en .

<https://www.opengis.net/ont/citygml/common/address> skos:definition "Relates the addresses to the Bridge or BridgePart."@en ;
    schema:domainIncludes brid:AbstractBridge ;
    schema:rangeIncludes core:Address .

<https://www.opengis.net/ont/citygml/common/boundary> skos:definition "Relates to the surfaces that bound the BridgeRoom. This relation is inherited from the Core module."@en ;
    schema:domainIncludes brid:BridgeRoom ;
    schema:rangeIncludes core:AbstractThematicSurface .

brid:BridgeConstructiveElement a owl:Class ;
    rdfs:label "BridgeConstructiveElement"@en ;
    rdfs:subClassOf [ a owl:Restriction ;
            owl:allValuesFrom brid:BridgeConstructiveElementUsageValue ;
            owl:onProperty <https://www.opengis.net/ont/citygml/common/usage> ],
        [ a owl:Restriction ;
            owl:allValuesFrom brid:BridgeConstructiveElementFunctionValue ;
            owl:onProperty <https://www.opengis.net/ont/citygml/common/function> ],
        [ a owl:Restriction ;
            owl:allValuesFrom brid:BridgeConstructiveElementClassValue ;
            owl:onProperty <https://www.opengis.net/ont/citygml/common/class> ],
        [ a owl:Restriction ;
            owl:maxQualifiedCardinality "1"^^xsd:nonNegativeInteger ;
            owl:onClass brid:BridgeConstructiveElementClassValue ;
            owl:onProperty <https://www.opengis.net/ont/citygml/common/class> ],
        con:AbstractConstructiveElement .

brid:isMovable a owl:DatatypeProperty ;
    rdfs:label "isMovable"@en ;
    rdfs:range xsd:boolean ;
    skos:definition "Indicates whether the Bridge or BridgePart can be moved to allow for watercraft to pass."@en .

<https://www.opengis.net/ont/citygml/common/bridgeFurniture> skos:definition "Relates the furniture objects to the Bridge or BridgePart."@en,
        "Relates the furniture objects to the BridgeRoom."@en ;
    schema:domainIncludes brid:AbstractBridge,
        brid:BridgeRoom ;
    schema:rangeIncludes brid:BridgeFurniture .

<https://www.opengis.net/ont/citygml/common/bridgeInstallation> skos:definition "Relates the installation objects to the Bridge or BridgePart."@en,
        "Relates to the installation objects to the BridgeRoom."@en ;
    schema:domainIncludes brid:AbstractBridge,
        brid:BridgeRoom ;
    schema:rangeIncludes brid:BridgeInstallation .

brid:BridgeFurniture a owl:Class ;
    rdfs:label "BridgeFurniture"@en ;
    rdfs:subClassOf [ a owl:Restriction ;
            owl:allValuesFrom brid:BridgeConstructiveElementClassValue ;
            owl:onProperty <https://www.opengis.net/ont/citygml/common/class> ],
        [ a owl:Restriction ;
            owl:maxQualifiedCardinality "1"^^xsd:nonNegativeInteger ;
            owl:onClass brid:BridgeConstructiveElementClassValue ;
            owl:onProperty <https://www.opengis.net/ont/citygml/common/class> ],
        [ a owl:Restriction ;
            owl:allValuesFrom brid:BridgeConstructiveElementUsageValue ;
            owl:onProperty <https://www.opengis.net/ont/citygml/common/usage> ],
        [ a owl:Restriction ;
            owl:allValuesFrom brid:BridgeConstructiveElementFunctionValue ;
            owl:onProperty <https://www.opengis.net/ont/citygml/common/function> ],
        con:AbstractFurniture .

brid:BridgeInstallation a owl:Class ;
    rdfs:label "BridgeInstallation"@en ;
    rdfs:subClassOf [ a owl:Restriction ;
            owl:allValuesFrom brid:BridgeConstructiveElementFunctionValue ;
            owl:onProperty <https://www.opengis.net/ont/citygml/common/function> ],
        [ a owl:Restriction ;
            owl:allValuesFrom brid:BridgeConstructiveElementClassValue ;
            owl:onProperty <https://www.opengis.net/ont/citygml/common/class> ],
        [ a owl:Restriction ;
            owl:maxQualifiedCardinality "1"^^xsd:nonNegativeInteger ;
            owl:onClass brid:BridgeConstructiveElementClassValue ;
            owl:onProperty <https://www.opengis.net/ont/citygml/common/class> ],
        [ a owl:Restriction ;
            owl:allValuesFrom brid:BridgeConstructiveElementUsageValue ;
            owl:onProperty <https://www.opengis.net/ont/citygml/common/usage> ],
        con:AbstractInstallation .

brid:BridgePart a owl:Class ;
    rdfs:label "BridgePart"@en ;
    rdfs:subClassOf brid:AbstractBridge .

brid:BridgeRoom a owl:Class ;
    rdfs:label "BridgeRoom"@en ;
    rdfs:subClassOf [ a owl:Restriction ;
            owl:allValuesFrom brid:BridgeConstructiveElementClassValue ;
            owl:onProperty <https://www.opengis.net/ont/citygml/common/class> ],
        [ a owl:Restriction ;
            owl:allValuesFrom core:AbstractThematicSurface ;
            owl:onProperty <https://www.opengis.net/ont/citygml/common/boundary> ],
        [ a owl:Restriction ;
            owl:allValuesFrom brid:BridgeConstructiveElementUsageValue ;
            owl:onProperty <https://www.opengis.net/ont/citygml/common/usage> ],
        [ a owl:Restriction ;
            owl:maxQualifiedCardinality "1"^^xsd:nonNegativeInteger ;
            owl:onClass brid:BridgeConstructiveElementClassValue ;
            owl:onProperty <https://www.opengis.net/ont/citygml/common/class> ],
        [ a owl:Restriction ;
            owl:allValuesFrom brid:BridgeConstructiveElementFunctionValue ;
            owl:onProperty <https://www.opengis.net/ont/citygml/common/function> ],
        [ a owl:Restriction ;
            owl:allValuesFrom brid:BridgeFurniture ;
            owl:onProperty <https://www.opengis.net/ont/citygml/common/bridgeFurniture> ],
        [ a owl:Restriction ;
            owl:allValuesFrom brid:BridgeInstallation ;
            owl:onProperty <https://www.opengis.net/ont/citygml/common/bridgeInstallation> ],
        core:AbstractUnoccupiedSpace .

<https://www.opengis.net/ont/citygml/common/function> rdfs:label "function"@en ;
    skos:definition "Specifies the intended purposes of the BridgeConstructiveElement."@en ;
    schema:rangeIncludes brid:BridgeConstructiveElementFunctionValue .

<https://www.opengis.net/ont/citygml/common/usage> rdfs:label "usage"@en ;
    skos:definition "Specifies the actual uses of the BridgeConstructiveElement."@en ;
    schema:rangeIncludes brid:BridgeConstructiveElementUsageValue .

brid:BridgeConstructiveElementFunctionValue a owl:Class ;
    rdfs:label "BridgeConstructiveElementFunctionValue"@en ;
    rdfs:subClassOf skos:Concept ;
    skos:definition "BridgeConstructiveElementFunctionValue is a code list that enumerates the different purposes of a BridgeConstructiveElement."@en .

brid:BridgeConstructiveElementUsageValue a owl:Class ;
    rdfs:label "BridgeConstructiveElementUsageValue"@en ;
    rdfs:subClassOf skos:Concept ;
    skos:definition "BridgeConstructiveElementUsageValue is a code list that enumerates the different uses of a BridgeConstructiveElement."@en .

brid:AbstractBridge a owl:Class ;
    rdfs:label "AbstractBridge"@en ;
    iso19150-2:isAbstract true ;
    rdfs:subClassOf [ a owl:Restriction ;
            owl:allValuesFrom xsd:boolean ;
            owl:onProperty brid:isMovable ],
        [ a owl:Restriction ;
            owl:allValuesFrom core:Address ;
            owl:onProperty <https://www.opengis.net/ont/citygml/common/address> ],
        [ a owl:Restriction ;
            owl:allValuesFrom brid:BridgeConstructiveElementFunctionValue ;
            owl:onProperty <https://www.opengis.net/ont/citygml/common/function> ],
        [ a owl:Restriction ;
            owl:maxQualifiedCardinality "1"^^xsd:nonNegativeInteger ;
            owl:onDataRange xsd:boolean ;
            owl:onProperty brid:isMovable ],
        [ a owl:Restriction ;
            owl:allValuesFrom brid:BridgeFurniture ;
            owl:onProperty <https://www.opengis.net/ont/citygml/common/bridgeFurniture> ],
        [ a owl:Restriction ;
            owl:allValuesFrom brid:BridgeConstructiveElementUsageValue ;
            owl:onProperty <https://www.opengis.net/ont/citygml/common/usage> ],
        [ a owl:Restriction ;
            owl:allValuesFrom brid:BridgeRoom ;
            owl:onProperty brid:bridgeRoom ],
        [ a owl:Restriction ;
            owl:maxQualifiedCardinality "1"^^xsd:nonNegativeInteger ;
            owl:onClass brid:BridgeConstructiveElementClassValue ;
            owl:onProperty <https://www.opengis.net/ont/citygml/common/class> ],
        [ a owl:Restriction ;
            owl:allValuesFrom brid:BridgeConstructiveElementClassValue ;
            owl:onProperty <https://www.opengis.net/ont/citygml/common/class> ],
        [ a owl:Restriction ;
            owl:allValuesFrom brid:BridgeInstallation ;
            owl:onProperty <https://www.opengis.net/ont/citygml/common/bridgeInstallation> ],
        [ a owl:Restriction ;
            owl:allValuesFrom brid:BridgeConstructiveElement ;
            owl:onProperty brid:bridgeConstructiveElement ],
        con:AbstractConstruction .

<https://www.opengis.net/ont/citygml/common/class> rdfs:label "class"@en ;
    skos:definition "Indicates the specific type of the BridgeConstructiveElement."@en ;
    schema:rangeIncludes brid:BridgeConstructiveElementClassValue .

brid:BridgeConstructiveElementClassValue a owl:Class ;
    rdfs:label "BridgeConstructiveElementClassValue"@en ;
    rdfs:subClassOf skos:Concept ;
    skos:definition "BridgeConstructiveElementClassValue is a code list used to further classify a BridgeConstructiveElement."@en .

@prefix bldg: <https://www.opengis.net/ont/citygml/building/> .
@prefix con: <https://www.opengis.net/ont/citygml/construction/> .
@prefix core: <https://www.opengis.net/ont/citygml/core/> .
@prefix iso19136-bt: <http://def.isotc211.org/iso19136/2007/BasicTypes#> .
@prefix iso19150-2: <http://def.isotc211.org/iso19150/-2/2012/base#> .
@prefix owl: <http://www.w3.org/2002/07/owl#> .
@prefix rdfs: <http://www.w3.org/2000/01/rdf-schema#> .
@prefix sc: <http://shapechange.net/resources/ont/base#> .
@prefix schema: <https://schema.org/> .
@prefix skos: <http://www.w3.org/2004/02/skos/core#> .
@prefix xsd: <http://www.w3.org/2001/XMLSchema#> .

<https://www.opengis.net/ont/citygml/building> a owl:Ontology ;
    rdfs:label "Building"@en ;
    owl:imports <http://def.isotc211.org/iso19150/-2/2012/base>,
        <http://shapechange.net/resources/ont/base>,
        <https://www.opengis.net/ont/citygml/common>,
        <https://www.opengis.net/ont/citygml/construction>,
        <https://www.opengis.net/ont/citygml/core> ;
    owl:versionIRI <https://www.opengis.net/ont/citygml/building/3.0.0/> ;
    owl:versionInfo "3.0.0" ;
    skos:definition "The Building module supports representation of thematic and spatial aspects of buildings, building parts, building installations, building subdivisions, and interior building structures."@en .

bldg:BuildingClassValue a owl:Class ;
    rdfs:label "BuildingClassValue"@en ;
    rdfs:subClassOf skos:Concept ;
    skos:definition "BuildingClassValue is a code list used to further classify a Building."@en .

bldg:BuildingConstructiveElementClassValue a owl:Class ;
    rdfs:label "BuildingConstructiveElementClassValue"@en ;
    rdfs:subClassOf skos:Concept ;
    skos:definition "BuildingConstructiveElementClassValue is a code list used to further classify a BuildingConstructiveElement."@en .

bldg:BuildingConstructiveElementFunctionValue a owl:Class ;
    rdfs:label "BuildingConstructiveElementFunctionValue"@en ;
    rdfs:subClassOf skos:Concept ;
    skos:definition "BuildingConstructiveElementFunctionValue is a code list that enumerates the different purposes of a BuildingConstructiveElement."@en .

bldg:BuildingConstructiveElementUsageValue a owl:Class ;
    rdfs:label "BuildingConstructiveElementUsageValue"@en ;
    rdfs:subClassOf skos:Concept ;
    skos:definition "BuildingConstructiveElementUsageValue is a code list that enumerates the different uses of a BuildingConstructiveElement."@en .

bldg:BuildingFunctionValue a owl:Class ;
    rdfs:label "BuildingFunctionValue"@en ;
    rdfs:subClassOf skos:Concept ;
    skos:definition "BuildingFunctionValue is a code list that enumerates the different purposes of a Building."@en .

bldg:BuildingFurnitureClassValue a owl:Class ;
    rdfs:label "BuildingFurnitureClassValue"@en ;
    rdfs:subClassOf skos:Concept ;
    skos:definition "BuildingFurnitureClassValue is a code list used to further classify a BuildingFurniture."@en .

bldg:BuildingFurnitureFunctionValue a owl:Class ;
    rdfs:label "BuildingFurnitureFunctionValue"@en ;
    rdfs:subClassOf skos:Concept ;
    skos:definition "BuildingFurnitureFunctionValue is a code list that enumerates the different purposes of a BuildingFurniture."@en .

bldg:BuildingFurnitureUsageValue a owl:Class ;
    rdfs:label "BuildingFurnitureUsageValue"@en ;
    rdfs:subClassOf skos:Concept ;
    skos:definition "BuildingFurnitureUsageValue is a code list that enumerates the different uses of a BuildingFurniture."@en .

bldg:BuildingRoomClassValue a owl:Class ;
    rdfs:label "BuildingRoomClassValue"@en ;
    rdfs:subClassOf skos:Concept ;
    skos:definition "BuildingRoomClassValue is a code list used to further classify a BuildingRoom."@en .

bldg:BuildingRoomFunctionValue a owl:Class ;
    rdfs:label "BuildingRoomFunctionValue"@en ;
    rdfs:subClassOf skos:Concept ;
    skos:definition "BuildingRoomFunctionValue is a code list that enumerates the different purposes of a BuildingRoom."@en .

bldg:BuildingRoomUsageValue a owl:Class ;
    rdfs:label "BuildingRoomUsageValue"@en ;
    rdfs:subClassOf skos:Concept ;
    skos:definition "BuildingRoomUsageValue is a code list that enumerates the different uses of a BuildingRoom."@en .

bldg:BuildingSubdivisionClassValue a owl:Class ;
    rdfs:label "BuildingSubdivisionClassValue"@en ;
    rdfs:subClassOf skos:Concept ;
    skos:definition "BuildingSubdivisionClassValue is a code list used to further classify a BuildingSubdivision."@en .

bldg:BuildingSubdivisionFunctionValue a owl:Class ;
    rdfs:label "BuildingSubdivisionFunctionValue"@en ;
    rdfs:subClassOf skos:Concept ;
    skos:definition "BuildingSubdivisionFunctionValue is a code list that enumerates the different purposes of a BuildingSubdivision."@en .

bldg:BuildingSubdivisionUsageValue a owl:Class ;
    rdfs:label "BuildingSubdivisionUsageValue"@en ;
    rdfs:subClassOf skos:Concept ;
    skos:definition "BuildingSubdivisionUsageValue is a code list that enumerates the different uses of a BuildingSubdivision."@en .

bldg:BuildingUsageValue a owl:Class ;
    rdfs:label "BuildingUsageValue"@en ;
    rdfs:subClassOf skos:Concept ;
    skos:definition "BuildingUsageValue is a code list that enumerates the different uses of a Building."@en .

bldg:Building a owl:Class ;
    rdfs:label "Building"@en ;
    rdfs:subClassOf [ a owl:Restriction ;
            owl:allValuesFrom bldg:BuildingPart ;
            owl:onProperty bldg:buildingPart ],
        bldg:AbstractBuilding ;
    owl:disjointWith bldg:BuildingPart .

bldg:buildingPart a owl:ObjectProperty ;
    rdfs:label "buildingPart"@en ;
    rdfs:domain bldg:Building ;
    rdfs:range bldg:BuildingPart ;
    skos:definition "Relates the building parts to the Building."@en .

bldg:buildingSubdivision a owl:ObjectProperty ;
    rdfs:label "buildingSubdivision"@en ;
    rdfs:domain bldg:AbstractBuilding ;
    rdfs:range bldg:AbstractBuildingSubdivision ;
    skos:definition "Relates the logical subdivisions to the Building or BuildingPart."@en .

bldg:buildingUnit a owl:ObjectProperty ;
    rdfs:label "buildingUnit"@en ;
    rdfs:domain bldg:Storey ;
    rdfs:range bldg:BuildingUnit ;
    skos:definition "Relates to the building units that belong to the Storey."@en .

bldg:roomHeight a owl:ObjectProperty ;
    rdfs:label "roomHeight"@en ;
    rdfs:range bldg:RoomHeight ;
    skos:definition "Specifies qualified heights of the BuildingRoom."@en .

bldg:storey a owl:ObjectProperty ;
    rdfs:label "storey"@en ;
    rdfs:domain bldg:BuildingUnit ;
    rdfs:range bldg:Storey ;
    skos:definition "Relates to the storeys on which the BuildingUnit is located."@en .

<https://www.opengis.net/ont/citygml/common/elevation> rdfs:label "elevation"@en ;
    skos:definition "Specifies qualified elevations of the building subdivision in relation to a well-defined surface which is commonly taken as origin (e.g. geoid or water level). [cf. INSPIRE]"@en ;
    schema:rangeIncludes con:Elevation .

bldg:RoomHeight a owl:Class ;
    rdfs:label "RoomHeight"@en ;
    rdfs:subClassOf [ a owl:Restriction ;
            owl:allValuesFrom bldg:RoomElevationReferenceValue ;
            owl:onProperty <https://www.opengis.net/ont/citygml/common/highReference> ],
        [ a owl:Restriction ;
            owl:allValuesFrom con:HeightStatusValue ;
            owl:onProperty <https://www.opengis.net/ont/citygml/common/status> ],
        [ a owl:Restriction ;
            owl:onClass bldg:RoomElevationReferenceValue ;
            owl:onProperty <https://www.opengis.net/ont/citygml/common/highReference> ;
            owl:qualifiedCardinality "1"^^xsd:nonNegativeInteger ],
        [ a owl:Restriction ;
            owl:allValuesFrom sc:Measure ;
            owl:onProperty <https://www.opengis.net/ont/citygml/common/value> ],
        [ a owl:Restriction ;
            owl:allValuesFrom bldg:RoomElevationReferenceValue ;
            owl:onProperty <https://www.opengis.net/ont/citygml/common/lowReference> ],
        [ a owl:Restriction ;
            owl:onClass bldg:RoomElevationReferenceValue ;
            owl:onProperty <https://www.opengis.net/ont/citygml/common/lowReference> ;
            owl:qualifiedCardinality "1"^^xsd:nonNegativeInteger ],
        [ a owl:Restriction ;
            owl:onDataRange sc:Measure ;
            owl:onProperty <https://www.opengis.net/ont/citygml/common/value> ;
            owl:qualifiedCardinality "1"^^xsd:nonNegativeInteger ],
        [ a owl:Restriction ;
            owl:onDataRange con:HeightStatusValue ;
            owl:onProperty <https://www.opengis.net/ont/citygml/common/status> ;
            owl:qualifiedCardinality "1"^^xsd:nonNegativeInteger ] ;
    skos:definition "The RoomHeight represents a vertical distance (measured or estimated) between a low reference and a high reference. [cf. INSPIRE]"@en .

bldg:roofType a owl:ObjectProperty ;
    rdfs:label "roofType"@en ;
    rdfs:range bldg:RoofTypeValue ;
    skos:definition "Indicates the shape of the roof of the Building or BuildingPart."@en .

bldg:sortKey a owl:DatatypeProperty ;
    rdfs:label "sortKey"@en ;
    rdfs:range xsd:double ;
    skos:definition "Defines an order among the objects that belong to the building subdivision. An example is the sorting of storeys."@en .

bldg:storeyHeightsAboveGround a owl:ObjectProperty ;
    rdfs:label "storeyHeightsAboveGround"@en ;
    rdfs:range iso19136-bt:MeasureOrNilReasonList ;
    skos:definition "Lists the heights of each storey above ground. The first value in the list denotes the height of the storey closest to the ground level, the last value denotes the height furthest away."@en .

bldg:storeyHeightsBelowGround a owl:ObjectProperty ;
    rdfs:label "storeyHeightsBelowGround"@en ;
    rdfs:range iso19136-bt:MeasureOrNilReasonList ;
    skos:definition "Lists the height of each storey below ground. The first value in the list denotes the height of the storey closest to the ground level, the last value denotes the height furthest away."@en .

bldg:storeysAboveGround a owl:DatatypeProperty ;
    rdfs:label "storeysAboveGround"@en ;
    rdfs:range xsd:integer ;
    skos:definition "Indicates the number of storeys positioned above ground level."@en .

bldg:storeysBelowGround a owl:DatatypeProperty ;
    rdfs:label "storeysBelowGround"@en ;
    rdfs:range xsd:integer ;
    skos:definition "Indicates the number of storeys positioned below ground level."@en .

<https://www.opengis.net/ont/citygml/common/address> skos:definition "Relates the addresses to the Building or BuildingPart."@en,
        "Relates to the addresses that are assigned to the BuildingUnit."@en ;
    schema:domainIncludes bldg:AbstractBuilding,
        bldg:BuildingUnit ;
    schema:rangeIncludes core:Address .

<https://www.opengis.net/ont/citygml/common/boundary> skos:definition "Relates to the surfaces that bound the BuildingRoom. This relation is inherited from the Core module."@en,
        "Relates to the surfaces that bound the Storey. This relation is inherited from the Core module."@en ;
    schema:domainIncludes bldg:BuildingRoom,
        bldg:Storey ;
    schema:rangeIncludes core:AbstractThematicSurface .

<https://www.opengis.net/ont/citygml/common/buildingConstructiveElement> skos:definition "Relates the constructive elements to the Building or BuildingPart."@en,
        "Relates the constructive elements to the building subdivision."@en ;
    schema:domainIncludes bldg:AbstractBuilding,
        bldg:AbstractBuildingSubdivision ;
    schema:rangeIncludes bldg:BuildingConstructiveElement .

<https://www.opengis.net/ont/citygml/common/buildingRoom> skos:definition "Relates the rooms to the Building or BuildingPart."@en,
        "Relates the rooms to the building subdivision."@en ;
    schema:domainIncludes bldg:AbstractBuilding,
        bldg:AbstractBuildingSubdivision ;
    schema:rangeIncludes bldg:BuildingRoom .

<https://www.opengis.net/ont/citygml/common/highReference> rdfs:label "highReference"@en ;
    skos:definition "Indicates the high point used to calculate the value of the room height."@en ;
    schema:rangeIncludes bldg:RoomElevationReferenceValue .

<https://www.opengis.net/ont/citygml/common/lowReference> rdfs:label "lowReference"@en ;
    skos:definition "Indicates the low point used to calculate the value of the room height."@en ;
    schema:rangeIncludes bldg:RoomElevationReferenceValue .

<https://www.opengis.net/ont/citygml/common/status> rdfs:label "status"@en ;
    skos:definition "Indicates the way the room height has been captured."@en ;
    schema:rangeIncludes con:HeightStatusValue .

<https://www.opengis.net/ont/citygml/common/value> rdfs:label "value"@en ;
    skos:definition "Specifies the value of the room height."@en ;
    schema:rangeIncludes sc:Measure .

bldg:BuildingConstructiveElement a owl:Class ;
    rdfs:label "BuildingConstructiveElement"@en ;
    rdfs:subClassOf [ a owl:Restriction ;
            owl:allValuesFrom bldg:BuildingInstallationUsageValue ;
            owl:onProperty <https://www.opengis.net/ont/citygml/common/usage> ],
        [ a owl:Restriction ;
            owl:allValuesFrom bldg:BuildingInstallationFunctionValue ;
            owl:onProperty <https://www.opengis.net/ont/citygml/common/function> ],
        [ a owl:Restriction ;
            owl:allValuesFrom bldg:BuildingInstallationClassValue ;
            owl:onProperty <https://www.opengis.net/ont/citygml/common/class> ],
        [ a owl:Restriction ;
            owl:maxQualifiedCardinality "1"^^xsd:nonNegativeInteger ;
            owl:onClass bldg:BuildingInstallationClassValue ;
            owl:onProperty <https://www.opengis.net/ont/citygml/common/class> ],
        con:AbstractConstructiveElement .

bldg:BuildingPart a owl:Class ;
    rdfs:label "BuildingPart"@en ;
    rdfs:subClassOf bldg:AbstractBuilding .

bldg:RoofTypeValue a owl:Class ;
    rdfs:label "RoofTypeValue"@en ;
    rdfs:subClassOf skos:Concept ;
    skos:definition "RoofTypeValue is a code list that enumerates different roof types."@en .

<https://www.opengis.net/ont/citygml/common/buildingFurniture> skos:definition "Relates the furniture objects to the Building or BuildingPart."@en,
        "Relates the furniture objects to the BuildingRoom."@en,
        "Relates the furniture objects to the building subdivision."@en ;
    schema:domainIncludes bldg:AbstractBuilding,
        bldg:AbstractBuildingSubdivision,
        bldg:BuildingRoom ;
    schema:rangeIncludes bldg:BuildingFurniture .

<https://www.opengis.net/ont/citygml/common/buildingInstallation> skos:definition "Relates the installation objects to the Building or BuildingPart."@en,
        "Relates the installation objects to the BuildingRoom."@en,
        "Relates the installation objects to the building subdivision."@en ;
    schema:domainIncludes bldg:AbstractBuilding,
        bldg:AbstractBuildingSubdivision,
        bldg:BuildingRoom ;
    schema:rangeIncludes bldg:BuildingInstallation .

bldg:BuildingFurniture a owl:Class ;
    rdfs:label "BuildingFurniture"@en ;
    rdfs:subClassOf [ a owl:Restriction ;
            owl:allValuesFrom bldg:BuildingInstallationUsageValue ;
            owl:onProperty <https://www.opengis.net/ont/citygml/common/usage> ],
        [ a owl:Restriction ;
            owl:allValuesFrom bldg:BuildingInstallationFunctionValue ;
            owl:onProperty <https://www.opengis.net/ont/citygml/common/function> ],
        [ a owl:Restriction ;
            owl:allValuesFrom bldg:BuildingInstallationClassValue ;
            owl:onProperty <https://www.opengis.net/ont/citygml/common/class> ],
        [ a owl:Restriction ;
            owl:maxQualifiedCardinality "1"^^xsd:nonNegativeInteger ;
            owl:onClass bldg:BuildingInstallationClassValue ;
            owl:onProperty <https://www.opengis.net/ont/citygml/common/class> ],
        con:AbstractFurniture .

bldg:BuildingInstallation a owl:Class ;
    rdfs:label "BuildingInstallation"@en ;
    rdfs:subClassOf [ a owl:Restriction ;
            owl:allValuesFrom bldg:BuildingInstallationUsageValue ;
            owl:onProperty <https://www.opengis.net/ont/citygml/common/usage> ],
        [ a owl:Restriction ;
            owl:allValuesFrom bldg:BuildingInstallationFunctionValue ;
            owl:onProperty <https://www.opengis.net/ont/citygml/common/function> ],
        [ a owl:Restriction ;
            owl:allValuesFrom bldg:BuildingInstallationClassValue ;
            owl:onProperty <https://www.opengis.net/ont/citygml/common/class> ],
        [ a owl:Restriction ;
            owl:maxQualifiedCardinality "1"^^xsd:nonNegativeInteger ;
            owl:onClass bldg:BuildingInstallationClassValue ;
            owl:onProperty <https://www.opengis.net/ont/citygml/common/class> ],
        con:AbstractInstallation .

bldg:BuildingUnit a owl:Class ;
    rdfs:label "BuildingUnit"@en ;
    rdfs:subClassOf [ a owl:Restriction ;
            owl:allValuesFrom core:Address ;
            owl:onProperty <https://www.opengis.net/ont/citygml/common/address> ],
        [ a owl:Restriction ;
            owl:allValuesFrom bldg:Storey ;
            owl:onProperty bldg:storey ],
        bldg:AbstractBuildingSubdivision ;
    owl:disjointWith bldg:Storey .

bldg:Storey a owl:Class ;
    rdfs:label "Storey"@en ;
    rdfs:subClassOf [ a owl:Restriction ;
            owl:allValuesFrom core:AbstractThematicSurface ;
            owl:onProperty <https://www.opengis.net/ont/citygml/common/boundary> ],
        [ a owl:Restriction ;
            owl:allValuesFrom bldg:BuildingUnit ;
            owl:onProperty bldg:buildingUnit ],
        bldg:AbstractBuildingSubdivision .

bldg:BuildingRoom a owl:Class ;
    rdfs:label "BuildingRoom"@en ;
    rdfs:subClassOf [ a owl:Restriction ;
            owl:allValuesFrom bldg:BuildingInstallationClassValue ;
            owl:onProperty <https://www.opengis.net/ont/citygml/common/class> ],
        [ a owl:Restriction ;
            owl:allValuesFrom bldg:RoomHeight ;
            owl:onProperty bldg:roomHeight ],
        [ a owl:Restriction ;
            owl:allValuesFrom bldg:BuildingFurniture ;
            owl:onProperty <https://www.opengis.net/ont/citygml/common/buildingFurniture> ],
        [ a owl:Restriction ;
            owl:allValuesFrom bldg:BuildingInstallationFunctionValue ;
            owl:onProperty <https://www.opengis.net/ont/citygml/common/function> ],
        [ a owl:Restriction ;
            owl:allValuesFrom bldg:BuildingInstallation ;
            owl:onProperty <https://www.opengis.net/ont/citygml/common/buildingInstallation> ],
        [ a owl:Restriction ;
            owl:allValuesFrom core:AbstractThematicSurface ;
            owl:onProperty <https://www.opengis.net/ont/citygml/common/boundary> ],
        [ a owl:Restriction ;
            owl:maxQualifiedCardinality "1"^^xsd:nonNegativeInteger ;
            owl:onClass bldg:BuildingInstallationClassValue ;
            owl:onProperty <https://www.opengis.net/ont/citygml/common/class> ],
        [ a owl:Restriction ;
            owl:allValuesFrom bldg:BuildingInstallationUsageValue ;
            owl:onProperty <https://www.opengis.net/ont/citygml/common/usage> ],
        core:AbstractUnoccupiedSpace .

bldg:RoomElevationReferenceValue a owl:Class ;
    rdfs:label "RoomElevationReferenceValue"@en ;
    rdfs:subClassOf skos:Concept ;
    skos:definition "RoomElevationReferenceValue is a code list that enumerates the different elevation reference levels used to measure room heights."@en .

<https://www.opengis.net/ont/citygml/common/function> rdfs:label "function"@en ;
    skos:definition "Specifies the intended purposes of the BuildingInstallation."@en ;
    schema:rangeIncludes bldg:BuildingInstallationFunctionValue .

<https://www.opengis.net/ont/citygml/common/usage> rdfs:label "usage"@en ;
    skos:definition "Specifies the actual uses of the BuildingInstallation."@en ;
    schema:rangeIncludes bldg:BuildingInstallationUsageValue .

bldg:BuildingInstallationFunctionValue a owl:Class ;
    rdfs:label "BuildingInstallationFunctionValue"@en ;
    rdfs:subClassOf skos:Concept ;
    skos:definition "BuildingInstallationFunctionValue is a code list that enumerates the different purposes of a BuildingInstallation."@en .

bldg:BuildingInstallationUsageValue a owl:Class ;
    rdfs:label "BuildingInstallationUsageValue"@en ;
    rdfs:subClassOf skos:Concept ;
    skos:definition "BuildingInstallationUsageValue is a code list that enumerates the different uses of a BuildingInstallation."@en .

bldg:AbstractBuilding a owl:Class ;
    rdfs:label "AbstractBuilding"@en ;
    iso19150-2:isAbstract true ;
    rdfs:subClassOf [ a owl:Restriction ;
            owl:allValuesFrom bldg:BuildingInstallationClassValue ;
            owl:onProperty <https://www.opengis.net/ont/citygml/common/class> ],
        [ a owl:Restriction ;
            owl:allValuesFrom bldg:BuildingInstallationUsageValue ;
            owl:onProperty <https://www.opengis.net/ont/citygml/common/usage> ],
        [ a owl:Restriction ;
            owl:allValuesFrom bldg:BuildingInstallation ;
            owl:onProperty <https://www.opengis.net/ont/citygml/common/buildingInstallation> ],
        [ a owl:Restriction ;
            owl:allValuesFrom bldg:BuildingRoom ;
            owl:onProperty <https://www.opengis.net/ont/citygml/common/buildingRoom> ],
        [ a owl:Restriction ;
            owl:allValuesFrom iso19136-bt:MeasureOrNilReasonList ;
            owl:onProperty bldg:storeyHeightsBelowGround ],
        [ a owl:Restriction ;
            owl:allValuesFrom bldg:BuildingConstructiveElement ;
            owl:onProperty <https://www.opengis.net/ont/citygml/common/buildingConstructiveElement> ],
        [ a owl:Restriction ;
            owl:maxQualifiedCardinality "1"^^xsd:nonNegativeInteger ;
            owl:onDataRange xsd:integer ;
            owl:onProperty bldg:storeysBelowGround ],
        [ a owl:Restriction ;
            owl:allValuesFrom xsd:integer ;
            owl:onProperty bldg:storeysBelowGround ],
        [ a owl:Restriction ;
            owl:maxQualifiedCardinality "1"^^xsd:nonNegativeInteger ;
            owl:onClass iso19136-bt:MeasureOrNilReasonList ;
            owl:onProperty bldg:storeyHeightsBelowGround ],
        [ a owl:Restriction ;
            owl:allValuesFrom xsd:integer ;
            owl:onProperty bldg:storeysAboveGround ],
        [ a owl:Restriction ;
            owl:maxQualifiedCardinality "1"^^xsd:nonNegativeInteger ;
            owl:onClass iso19136-bt:MeasureOrNilReasonList ;
            owl:onProperty bldg:storeyHeightsAboveGround ],
        [ a owl:Restriction ;
            owl:allValuesFrom bldg:BuildingFurniture ;
            owl:onProperty <https://www.opengis.net/ont/citygml/common/buildingFurniture> ],
        [ a owl:Restriction ;
            owl:allValuesFrom core:Address ;
            owl:onProperty <https://www.opengis.net/ont/citygml/common/address> ],
        [ a owl:Restriction ;
            owl:maxQualifiedCardinality "1"^^xsd:nonNegativeInteger ;
            owl:onClass bldg:BuildingInstallationClassValue ;
            owl:onProperty <https://www.opengis.net/ont/citygml/common/class> ],
        [ a owl:Restriction ;
            owl:maxQualifiedCardinality "1"^^xsd:nonNegativeInteger ;
            owl:onClass bldg:RoofTypeValue ;
            owl:onProperty bldg:roofType ],
        [ a owl:Restriction ;
            owl:maxQualifiedCardinality "1"^^xsd:nonNegativeInteger ;
            owl:onDataRange xsd:integer ;
            owl:onProperty bldg:storeysAboveGround ],
        [ a owl:Restriction ;
            owl:allValuesFrom iso19136-bt:MeasureOrNilReasonList ;
            owl:onProperty bldg:storeyHeightsAboveGround ],
        [ a owl:Restriction ;
            owl:allValuesFrom bldg:BuildingInstallationFunctionValue ;
            owl:onProperty <https://www.opengis.net/ont/citygml/common/function> ],
        [ a owl:Restriction ;
            owl:allValuesFrom bldg:AbstractBuildingSubdivision ;
            owl:onProperty bldg:buildingSubdivision ],
        [ a owl:Restriction ;
            owl:allValuesFrom bldg:RoofTypeValue ;
            owl:onProperty bldg:roofType ],
        con:AbstractConstruction .

bldg:AbstractBuildingSubdivision a owl:Class ;
    rdfs:label "AbstractBuildingSubdivision"@en ;
    iso19150-2:isAbstract true ;
    rdfs:subClassOf [ a owl:Restriction ;
            owl:allValuesFrom con:Elevation ;
            owl:onProperty <https://www.opengis.net/ont/citygml/common/elevation> ],
        [ a owl:Restriction ;
            owl:allValuesFrom bldg:BuildingInstallationUsageValue ;
            owl:onProperty <https://www.opengis.net/ont/citygml/common/usage> ],
        [ a owl:Restriction ;
            owl:allValuesFrom bldg:BuildingInstallationClassValue ;
            owl:onProperty <https://www.opengis.net/ont/citygml/common/class> ],
        [ a owl:Restriction ;
            owl:maxQualifiedCardinality "1"^^xsd:nonNegativeInteger ;
            owl:onDataRange xsd:double ;
            owl:onProperty bldg:sortKey ],
        [ a owl:Restriction ;
            owl:allValuesFrom bldg:BuildingRoom ;
            owl:onProperty <https://www.opengis.net/ont/citygml/common/buildingRoom> ],
        [ a owl:Restriction ;
            owl:allValuesFrom bldg:BuildingFurniture ;
            owl:onProperty <https://www.opengis.net/ont/citygml/common/buildingFurniture> ],
        [ a owl:Restriction ;
            owl:allValuesFrom xsd:double ;
            owl:onProperty bldg:sortKey ],
        [ a owl:Restriction ;
            owl:allValuesFrom bldg:BuildingInstallationFunctionValue ;
            owl:onProperty <https://www.opengis.net/ont/citygml/common/function> ],
        [ a owl:Restriction ;
            owl:allValuesFrom bldg:BuildingInstallation ;
            owl:onProperty <https://www.opengis.net/ont/citygml/common/buildingInstallation> ],
        [ a owl:Restriction ;
            owl:allValuesFrom bldg:BuildingConstructiveElement ;
            owl:onProperty <https://www.opengis.net/ont/citygml/common/buildingConstructiveElement> ],
        [ a owl:Restriction ;
            owl:maxQualifiedCardinality "1"^^xsd:nonNegativeInteger ;
            owl:onClass bldg:BuildingInstallationClassValue ;
            owl:onProperty <https://www.opengis.net/ont/citygml/common/class> ],
        core:AbstractLogicalSpace .

<https://www.opengis.net/ont/citygml/common/class> rdfs:label "class"@en ;
    skos:definition "Indicates the specific type of the BuildingInstallation."@en ;
    schema:rangeIncludes bldg:BuildingInstallationClassValue .

bldg:BuildingInstallationClassValue a owl:Class ;
    rdfs:label "BuildingInstallationClassValue"@en ;
    rdfs:subClassOf skos:Concept ;
    skos:definition "BuildingInstallationClassValue is a code list used to further classify a BuildingInstallation."@en .

@prefix core: <https://www.opengis.net/ont/citygml/core/> .
@prefix frn: <https://www.opengis.net/ont/citygml/cityfurniture/> .
@prefix owl: <http://www.w3.org/2002/07/owl#> .
@prefix rdfs: <http://www.w3.org/2000/01/rdf-schema#> .
@prefix schema: <https://schema.org/> .
@prefix skos: <http://www.w3.org/2004/02/skos/core#> .
@prefix xsd: <http://www.w3.org/2001/XMLSchema#> .

<https://www.opengis.net/ont/citygml/cityfurniture> a owl:Ontology ;
    rdfs:label "CityFurniture"@en ;
    owl:imports <http://def.isotc211.org/iso19150/-2/2012/base>,
        <https://www.opengis.net/ont/citygml/common>,
        <https://www.opengis.net/ont/citygml/core> ;
    owl:versionIRI <https://www.opengis.net/ont/citygml/cityfurniture/3.0.0/> ;
    owl:versionInfo "3.0.0" ;
    skos:definition "The CityFurniture module supports representation of city furniture objects. City furniture objects are immovable objects like lanterns, traffic signs, advertising columns, benches, or bus stops that can be found in traffic areas, residential areas, on squares, or in built-up areas."@en .

frn:CityFurniture a owl:Class ;
    rdfs:label "CityFurniture"@en ;
    rdfs:subClassOf [ a owl:Restriction ;
            owl:allValuesFrom frn:CityFurnitureUsageValue ;
            owl:onProperty <https://www.opengis.net/ont/citygml/common/usage> ],
        [ a owl:Restriction ;
            owl:allValuesFrom frn:CityFurnitureFunctionValue ;
            owl:onProperty <https://www.opengis.net/ont/citygml/common/function> ],
        [ a owl:Restriction ;
            owl:allValuesFrom frn:CityFurnitureClassValue ;
            owl:onProperty <https://www.opengis.net/ont/citygml/common/class> ],
        [ a owl:Restriction ;
            owl:maxQualifiedCardinality "1"^^xsd:nonNegativeInteger ;
            owl:onClass frn:CityFurnitureClassValue ;
            owl:onProperty <https://www.opengis.net/ont/citygml/common/class> ],
        core:AbstractOccupiedSpace .

<https://www.opengis.net/ont/citygml/common/function> rdfs:label "function"@en ;
    skos:definition "Specifies the intended purposes of the CityFurniture."@en ;
    schema:rangeIncludes frn:CityFurnitureFunctionValue .

<https://www.opengis.net/ont/citygml/common/usage> rdfs:label "usage"@en ;
    skos:definition "Specifies the actual uses of the CityFurniture."@en ;
    schema:rangeIncludes frn:CityFurnitureUsageValue .

frn:CityFurnitureFunctionValue a owl:Class ;
    rdfs:label "CityFurnitureFunctionValue"@en ;
    rdfs:subClassOf skos:Concept ;
    skos:definition "CityFurnitureFunctionValue is a code list that enumerates the different purposes of a CityFurniture."@en .

frn:CityFurnitureUsageValue a owl:Class ;
    rdfs:label "CityFurnitureUsageValue"@en ;
    rdfs:subClassOf skos:Concept ;
    skos:definition "CityFurnitureUsageValue is a code list that enumerates the different uses of a CityFurniture."@en .

<https://www.opengis.net/ont/citygml/common/class> rdfs:label "class"@en ;
    skos:definition "Indicates the specific type of the CityFurniture."@en ;
    schema:rangeIncludes frn:CityFurnitureClassValue .

frn:CityFurnitureClassValue a owl:Class ;
    rdfs:label "CityFurnitureClassValue"@en ;
    rdfs:subClassOf skos:Concept ;
    skos:definition "CityFurnitureClassValue is a code list used to further classify a CityFurniture."@en .

@prefix core: <https://www.opengis.net/ont/citygml/core/> .
@prefix grp: <https://www.opengis.net/ont/citygml/cityobjectgroup/> .
@prefix owl: <http://www.w3.org/2002/07/owl#> .
@prefix rdfs: <http://www.w3.org/2000/01/rdf-schema#> .
@prefix schema: <https://schema.org/> .
@prefix skos: <http://www.w3.org/2004/02/skos/core#> .
@prefix xsd: <http://www.w3.org/2001/XMLSchema#> .

<https://www.opengis.net/ont/citygml/cityobjectgroup> a owl:Ontology ;
    rdfs:label "CityObjectGroup"@en ;
    owl:imports <http://def.isotc211.org/iso19150/-2/2012/base>,
        <https://www.opengis.net/ont/citygml/common>,
        <https://www.opengis.net/ont/citygml/core> ;
    owl:versionIRI <https://www.opengis.net/ont/citygml/cityobjectgroup/3.0.0/> ;
    owl:versionInfo "3.0.0" ;
    skos:definition "The CityObjectGroup module supports grouping of city objects. Arbitrary city objects may be aggregated in groups according to user-defined criteria. A group may be further classified by application-specific attributes."@en .

<https://www.opengis.net/ont/citygml/common/function> rdfs:label "function"@en ;
    skos:definition "Specifies the intended purposes of the CityObjectGroup."@en ;
    schema:rangeIncludes grp:CityObjectGroupFunctionValue .

<https://www.opengis.net/ont/citygml/common/usage> rdfs:label "usage"@en ;
    skos:definition "Specifies the actual usages of the CityObjectGroup."@en ;
    schema:rangeIncludes grp:CityObjectGroupUsageValue .

grp:CityObjectGroup a owl:Class ;
    rdfs:label "CityObjectGroup"@en ;
    rdfs:subClassOf [ a owl:Restriction ;
            owl:maxQualifiedCardinality "1"^^xsd:nonNegativeInteger ;
            owl:onClass grp:CityObjectGroupClassValue ;
            owl:onProperty <https://www.opengis.net/ont/citygml/common/class> ],
        [ a owl:Restriction ;
            owl:allValuesFrom core:AbstractCityObject ;
            owl:onProperty grp:parent ],
        [ a owl:Restriction ;
            owl:maxQualifiedCardinality "1"^^xsd:nonNegativeInteger ;
            owl:onClass core:AbstractCityObject ;
            owl:onProperty grp:parent ],
        [ a owl:Restriction ;
            owl:allValuesFrom grp:CityObjectGroupUsageValue ;
            owl:onProperty <https://www.opengis.net/ont/citygml/common/usage> ],
        [ a owl:Restriction ;
            owl:allValuesFrom grp:Role ;
            owl:onProperty <https://www.opengis.net/ont/citygml/common/groupMember> ],
        [ a owl:Restriction ;
            owl:allValuesFrom grp:CityObjectGroupFunctionValue ;
            owl:onProperty <https://www.opengis.net/ont/citygml/common/function> ],
        [ a owl:Restriction ;
            owl:allValuesFrom grp:CityObjectGroupClassValue ;
            owl:onProperty <https://www.opengis.net/ont/citygml/common/class> ],
        core:AbstractLogicalSpace .

grp:CityObjectGroupFunctionValue a owl:Class ;
    rdfs:label "CityObjectGroupFunctionValue"@en ;
    rdfs:subClassOf skos:Concept ;
    skos:definition "CityObjectGroupFunctionValue is a code list that enumerates the different purposes of a CityObjectGroup."@en .

grp:CityObjectGroupUsageValue a owl:Class ;
    rdfs:label "CityObjectGroupUsageValue"@en ;
    rdfs:subClassOf skos:Concept ;
    skos:definition "CityObjectGroupUsageValue is a code list that enumerates the different uses of a CityObjectGroup."@en .

grp:parent a owl:ObjectProperty ;
    rdfs:label "parent"@en ;
    rdfs:domain grp:CityObjectGroup ;
    rdfs:range core:AbstractCityObject ;
    skos:definition "Relates to a city object to which the CityObjectGroup belongs."@en .

grp:role a owl:DatatypeProperty ;
    rdfs:label "role"@en ;
    rdfs:range xsd:string ;
    skos:definition "Describes the role the city object plays within the CityObjectGroup."@en .

<https://www.opengis.net/ont/citygml/common/class> rdfs:label "class"@en ;
    skos:definition "Indicates the specific type of the CityObjectGroup."@en ;
    schema:rangeIncludes grp:CityObjectGroupClassValue .

grp:CityObjectGroupClassValue a owl:Class ;
    rdfs:label "CityObjectGroupClassValue"@en ;
    rdfs:subClassOf skos:Concept ;
    skos:definition "CityObjectGroupClassValue is a code list used to further classify a CityObjectGroup."@en .

grp:Role a owl:Class ;
    rdfs:label "Role"@en ;
    rdfs:subClassOf [ a owl:Restriction ;
            owl:maxQualifiedCardinality "1"^^xsd:nonNegativeInteger ;
            owl:onDataRange xsd:string ;
            owl:onProperty grp:role ],
        [ a owl:Restriction ;
            owl:allValuesFrom core:AbstractCityObject ;
            owl:onProperty <https://www.opengis.net/ont/citygml/common/groupMember> ],
        [ a owl:Restriction ;
            owl:onClass core:AbstractCityObject ;
            owl:onProperty <https://www.opengis.net/ont/citygml/common/groupMember> ;
            owl:qualifiedCardinality "1"^^xsd:nonNegativeInteger ],
        [ a owl:Restriction ;
            owl:allValuesFrom xsd:string ;
            owl:onProperty grp:role ] ;
    skos:definition "Role qualifies the function of a city object within the CityObjectGroup."@en .

<https://www.opengis.net/ont/citygml/common/groupMember> skos:definition "Relates to the city objects that are part of the CityObjectGroup."@en ;
    schema:domainIncludes grp:CityObjectGroup,
        grp:Role ;
    schema:rangeIncludes grp:Role,
        core:AbstractCityObject .

@prefix owl:  <http://www.w3.org/2002/07/owl#> .
@prefix rdfs: <http://www.w3.org/2000/01/rdf-schema#> .
@prefix common: <https://www.opengis.net/ont/citygml/common/> .
@prefix geo: <http://www.opengis.net/ont/geosparql#> .

common:class rdf:type owl:ObjectProperty; rdfs:label "class"@en.
common:usage rdf:type owl:ObjectProperty; rdfs:label "usage"@en.
common:function rdf:type owl:ObjectProperty; rdfs:label "function"@en.

common:address rdf:type owl:ObjectProperty; rdfs:label "address"@en.
common:appearance  rdf:type owl:ObjectProperty; rdfs:label "appearance"@en .
common:area  rdf:type owl:ObjectProperty; rdfs:label "area"@en .
common:boundary rdf:type owl:ObjectProperty; rdfs:label "boundary"@en.
common:bridgeFurniture  rdf:type owl:ObjectProperty; rdfs:label "bridgeFurniture"@en .
common:bridgeInstallation  rdf:type owl:ObjectProperty; rdfs:label "bridgeInstallation"@en .
common:buildingConstructiveElement  rdf:type owl:ObjectProperty; rdfs:label "buildingConstructiveElement"@en .
common:buildingFurniture  rdf:type owl:ObjectProperty; rdfs:label "buildingFurniture"@en .
common:buildingInstallation  rdf:type owl:ObjectProperty; rdfs:label "buildingInstallation"@en .
common:buildingRoom  rdf:type owl:ObjectProperty; rdfs:label "buildingRoom"@en .
common:elevation  rdf:type owl:ObjectProperty; rdfs:label "elevation"@en .
common:genericAttribute  rdf:type owl:ObjectProperty; rdfs:label "genericAttribute"@en .
common:groupMember  rdf:type owl:ObjectProperty; rdfs:label "groupMember"@en .
common:highReference  rdf:type owl:ObjectProperty; rdfs:label "highReference"@en .
common:intersection  rdf:type owl:ObjectProperty; rdfs:label "intersection"@en .
common:lod0MultiCurve  rdf:type owl:ObjectProperty; rdfs:label "lod0MultiCurve"@en .
common:lod0MultiSurface  rdf:type owl:ObjectProperty; rdfs:label "lod0MultiSurface"@en .
common:lod2MultiSurface  rdf:type owl:ObjectProperty; rdfs:label "lod2MultiSurface"@en .
common:lod3MultiSurface  rdf:type owl:ObjectProperty; rdfs:label "lod3MultiSurface"@en .
common:lowReference  rdf:type owl:ObjectProperty; rdfs:label "lowReference"@en .
common:mimeType rdf:type owl:ObjectProperty; rdfs:label "mimeType"@en.
common:occupancy  rdf:type owl:ObjectProperty; rdfs:label "occupancy"@en .
common:occupancy rdf:type owl:ObjectProperty; rdfs:label "occupancy"@en.
common:pointCloud  rdf:type owl:ObjectProperty; rdfs:label "pointCloud"@en .
common:referencePoint  rdf:type owl:ObjectProperty; rdfs:label "referencePoint"@en .
common:referringTo  rdf:type owl:ObjectProperty; rdfs:label "referringTo"@en .
common:relatedTo  rdf:type owl:ObjectProperty; rdfs:label "relatedTo"@en .
common:section  rdf:type owl:ObjectProperty; rdfs:label "section"@en .
common:textureParameterization  rdf:type owl:ObjectProperty; rdfs:label "textureParameterization"@en .
common:tunnelFurniture  rdf:type owl:ObjectProperty; rdfs:label "tunnelFurniture"@en .
common:tunnelInstallation  rdf:type owl:ObjectProperty; rdfs:label "tunnelInstallation"@en .
common:versionMember  rdf:type owl:ObjectProperty; rdfs:label "versionMember"@en .

common:name rdf:type owl:DatatypeProperty; rdfs:label "name"@en .
common:description rdf:type owl:DatatypeProperty; rdfs:label "description"@en .
common:value rdf:type owl:DatatypeProperty; rdfs:label "value"@en.
common:status rdf:type owl:DatatypeProperty; rdfs:label "status"@en.

# GeoSPARQL alignments for common properties
common:lod0MultiCurve rdfs:subPropertyOf geo:hasGeometry .
common:lod0MultiSurface rdfs:subPropertyOf geo:hasGeometry .
common:lod2MultiSurface rdfs:subPropertyOf geo:hasGeometry .
common:lod3MultiSurface rdfs:subPropertyOf geo:hasGeometry .
common:referencePoint rdfs:subPropertyOf geo:hasGeometry .

#this property axiom is NOT officially declared in the CityGML 3.0, but we need it to do change request
common:boundary rdfs:subPropertyOf geo:hasGeometry .
@prefix bldg: <https://www.opengis.net/ont/citygml/building/> .
@prefix brid: <https://www.opengis.net/ont/citygml/bridge/> .
@prefix con: <https://www.opengis.net/ont/citygml/construction/> .
@prefix core: <https://www.opengis.net/ont/citygml/core/> .
@prefix gmlowl: <http://www.opengis.net/ont/gml#> .
@prefix iso19150-2: <http://def.isotc211.org/iso19150/-2/2012/base#> .
@prefix owl: <http://www.w3.org/2002/07/owl#> .
@prefix rdf: <http://www.w3.org/1999/02/22-rdf-syntax-ns#> .
@prefix rdfs: <http://www.w3.org/2000/01/rdf-schema#> .
@prefix sc: <http://shapechange.net/resources/ont/base#> .
@prefix schema: <https://schema.org/> .
@prefix skos: <http://www.w3.org/2004/02/skos/core#> .
@prefix tun: <https://www.opengis.net/ont/citygml/tunnel/> .
@prefix xsd: <http://www.w3.org/2001/XMLSchema#> .

<https://www.opengis.net/ont/citygml/construction> a owl:Ontology ;
    rdfs:label "Construction"@en ;
    owl:imports <http://def.isotc211.org/iso19150/-2/2012/base>,
        <http://shapechange.net/resources/ont/base>,
        <http://www.opengis.net/ont/gml>,
        <https://www.opengis.net/ont/citygml/bridge>,
        <https://www.opengis.net/ont/citygml/building>,
        <https://www.opengis.net/ont/citygml/common>,
        <https://www.opengis.net/ont/citygml/core>,
        <https://www.opengis.net/ont/citygml/tunnel> ;
    owl:versionIRI <https://www.opengis.net/ont/citygml/construction/3.0.0/> ;
    owl:versionInfo "3.0.0" ;
    skos:definition "The Construction module supports representation of key elements of different types of constructions. These key elements include construction surfaces (e.g floor and ceiling), windows and doors, constructive elements (e.g. beams and slabs), installations, and furniture."@en .

con:AbstractFurniture a owl:Class ;
    rdfs:label "AbstractFurniture"@en ;
    iso19150-2:isAbstract true ;
    rdfs:subClassOf core:AbstractOccupiedSpace .

con:OtherConstructionClassValue a owl:Class ;
    rdfs:label "OtherConstructionClassValue"@en ;
    rdfs:subClassOf skos:Concept ;
    skos:definition "OtherConstructionClassValue is a code list used to further classify an OtherConstruction."@en .

con:OtherConstructionFunctionValue a owl:Class ;
    rdfs:label "OtherConstructionFunctionValue"@en ;
    rdfs:subClassOf skos:Concept ;
    skos:definition "OtherConstructionFunctionValue is a code list that enumerates the different purposes of an OtherConstruction."@en .

con:OtherConstructionUsageValue a owl:Class ;
    rdfs:label "OtherConstructionUsageValue"@en ;
    rdfs:subClassOf skos:Concept ;
    skos:definition "OtherConstructionUsageValue is a code list that enumerates the different uses of an OtherConstruction."@en .

con:WindowClassValue a owl:Class ;
    rdfs:label "WindowClassValue"@en ;
    rdfs:subClassOf skos:Concept ;
    skos:definition "WindowClassValue is a code list used to further classify a Window."@en .

con:WindowFunctionValue a owl:Class ;
    rdfs:label "WindowFunctionValue"@en ;
    rdfs:subClassOf skos:Concept ;
    skos:definition "WindowFunctionValue is a code list that enumerates the different purposes of a Window."@en .

con:WindowUsageValue a owl:Class ;
    rdfs:label "WindowUsageValue"@en ;
    rdfs:subClassOf skos:Concept ;
    skos:definition "WindowUsageValue is a code list that enumerates the different uses of a Window."@en .

<https://www.opengis.net/ont/citygml/common/elevation> rdfs:label "elevation"@en ;
    skos:definition "Specifies qualified elevations of the construction in relation to a well-defined surface which is commonly taken as origin (e.g. geoid or water level). [cf. INSPIRE]"@en ;
    schema:rangeIncludes con:Elevation .

<https://www.opengis.net/ont/citygml/common/occupancy> rdfs:label "occupancy"@en ;
    skos:definition "Provides qualified information on the residency of persons, animals, or other moveable objects in the construction."@en ;
    schema:rangeIncludes core:Occupancy .

con:AbstractInstallation a owl:Class ;
    rdfs:label "AbstractInstallation"@en ;
    iso19150-2:isAbstract true ;
    rdfs:subClassOf [ a owl:Restriction ;
            owl:allValuesFrom core:AbstractThematicSurface ;
            owl:onProperty <https://www.opengis.net/ont/citygml/common/boundary> ],
        [ a owl:Restriction ;
            owl:allValuesFrom con:RelationToConstruction ;
            owl:onProperty con:relationToConstruction ],
        [ a owl:Restriction ;
            owl:maxQualifiedCardinality "1"^^xsd:nonNegativeInteger ;
            owl:onDataRange con:RelationToConstruction ;
            owl:onProperty con:relationToConstruction ],
        core:AbstractOccupiedSpace .

con:CeilingSurface a owl:Class ;
    rdfs:label "CeilingSurface"@en ;
    rdfs:subClassOf con:AbstractConstructionSurface .

con:FloorSurface a owl:Class ;
    rdfs:label "FloorSurface"@en ;
    rdfs:subClassOf con:AbstractConstructionSurface .

con:GroundSurface a owl:Class ;
    rdfs:label "GroundSurface"@en ;
    rdfs:subClassOf con:AbstractConstructionSurface .

con:InteriorWallSurface a owl:Class ;
    rdfs:label "InteriorWallSurface"@en ;
    rdfs:subClassOf con:AbstractConstructionSurface .

con:OtherConstruction a owl:Class ;
    rdfs:label "OtherConstruction"@en ;
    rdfs:subClassOf [ a owl:Restriction ;
            owl:allValuesFrom con:DoorUsageValue ;
            owl:onProperty <https://www.opengis.net/ont/citygml/common/usage> ],
        [ a owl:Restriction ;
            owl:allValuesFrom con:DoorFunctionValue ;
            owl:onProperty <https://www.opengis.net/ont/citygml/common/function> ],
        [ a owl:Restriction ;
            owl:allValuesFrom con:DoorClassValue ;
            owl:onProperty <https://www.opengis.net/ont/citygml/common/class> ],
        [ a owl:Restriction ;
            owl:maxQualifiedCardinality "1"^^xsd:nonNegativeInteger ;
            owl:onClass con:DoorClassValue ;
            owl:onProperty <https://www.opengis.net/ont/citygml/common/class> ],
        con:AbstractConstruction .

con:OuterCeilingSurface a owl:Class ;
    rdfs:label "OuterCeilingSurface"@en ;
    rdfs:subClassOf con:AbstractConstructionSurface .

con:OuterFloorSurface a owl:Class ;
    rdfs:label "OuterFloorSurface"@en ;
    rdfs:subClassOf con:AbstractConstructionSurface .

con:RoofSurface a owl:Class ;
    rdfs:label "RoofSurface"@en ;
    rdfs:subClassOf con:AbstractConstructionSurface .

con:WallSurface a owl:Class ;
    rdfs:label "WallSurface"@en ;
    rdfs:subClassOf con:AbstractConstructionSurface .

con:constructionEvent a owl:ObjectProperty ;
    rdfs:label "constructionEvent"@en ;
    rdfs:range con:ConstructionEvent ;
    skos:definition "Describes specific events in the life-time of the construction."@en .

con:filling a owl:ObjectProperty ;
    rdfs:label "filling"@en ;
    rdfs:domain con:AbstractConstructiveElement ;
    rdfs:range con:AbstractFillingElement ;
    skos:definition "Relates to the elements that fill the opening of the constructive element."@en .

con:fillingSurface a owl:ObjectProperty ;
    rdfs:label "fillingSurface"@en ;
    rdfs:domain con:AbstractConstructionSurface ;
    rdfs:range con:AbstractFillingSurface ;
    skos:definition "Relates to the surfaces that seal the openings of the construction surface."@en .

con:height a owl:ObjectProperty ;
    rdfs:label "height"@en ;
    rdfs:range con:Height ;
    skos:definition "Specifies qualified heights of the construction above ground or below ground. [cf. INSPIRE]"@en .

<https://www.opengis.net/ont/citygml/common/address> skos:definition "Relates to the addresses that are assigned to the Door."@en,
        "Relates to the addresses that are assigned to the DoorSurface."@en ;
    schema:domainIncludes con:Door,
        con:DoorSurface ;
    schema:rangeIncludes core:Address .

<https://www.opengis.net/ont/citygml/common/description> rdfs:label "description"@en ;
    skos:definition "Provides additional information on the event."@en ;
    schema:rangeIncludes xsd:string .

<https://www.opengis.net/ont/citygml/common/highReference> rdfs:label "highReference"@en ;
    skos:definition "Indicates the high point used to calculate the value of the height. [cf. INSPIRE]"@en ;
    schema:rangeIncludes con:ElevationReferenceValue .

<https://www.opengis.net/ont/citygml/common/lowReference> rdfs:label "lowReference"@en ;
    skos:definition "Indicates the low point used to calculate the value of the height. [cf. INSPIRE]"@en ;
    schema:rangeIncludes con:ElevationReferenceValue .

<https://www.opengis.net/ont/citygml/common/status> rdfs:label "status"@en ;
    skos:definition "Indicates the way the height has been captured. [cf. INSPIRE]"@en ;
    schema:rangeIncludes con:HeightStatusValue .

<https://www.opengis.net/ont/citygml/common/value> rdfs:label "value"@en ;
    skos:definition "Specifies the value of the height above or below ground. [cf. INSPIRE]"@en ;
    schema:rangeIncludes sc:Measure .

con:AbstractConstruction a owl:Class ;
    rdfs:label "AbstractConstruction"@en ;
    iso19150-2:isAbstract true ;
    rdfs:subClassOf [ a owl:Restriction ;
            owl:allValuesFrom xsd:date ;
            owl:onProperty con:dateOfDemolition ],
        [ a owl:Restriction ;
            owl:allValuesFrom xsd:date ;
            owl:onProperty con:dateOfConstruction ],
        [ a owl:Restriction ;
            owl:maxQualifiedCardinality "1"^^xsd:nonNegativeInteger ;
            owl:onDataRange xsd:date ;
            owl:onProperty con:dateOfConstruction ],
        [ a owl:Restriction ;
            owl:allValuesFrom core:AbstractThematicSurface ;
            owl:onProperty <https://www.opengis.net/ont/citygml/common/boundary> ],
        [ a owl:Restriction ;
            owl:allValuesFrom con:Height ;
            owl:onProperty con:height ],
        [ a owl:Restriction ;
            owl:allValuesFrom con:ConstructionEvent ;
            owl:onProperty con:constructionEvent ],
        [ a owl:Restriction ;
            owl:maxQualifiedCardinality "1"^^xsd:nonNegativeInteger ;
            owl:onDataRange xsd:date ;
            owl:onProperty con:dateOfDemolition ],
        [ a owl:Restriction ;
            owl:allValuesFrom core:Occupancy ;
            owl:onProperty <https://www.opengis.net/ont/citygml/common/occupancy> ],
        [ a owl:Restriction ;
            owl:allValuesFrom con:ConditionOfConstructionValue ;
            owl:onProperty con:conditionOfConstruction ],
        [ a owl:Restriction ;
            owl:allValuesFrom con:Elevation ;
            owl:onProperty <https://www.opengis.net/ont/citygml/common/elevation> ],
        [ a owl:Restriction ;
            owl:maxQualifiedCardinality "1"^^xsd:nonNegativeInteger ;
            owl:onDataRange con:ConditionOfConstructionValue ;
            owl:onProperty con:conditionOfConstruction ],
        core:AbstractOccupiedSpace .

con:AbstractConstructiveElement a owl:Class ;
    rdfs:label "AbstractConstructiveElement"@en ;
    iso19150-2:isAbstract true ;
    rdfs:subClassOf [ a owl:Restriction ;
            owl:allValuesFrom con:AbstractFillingElement ;
            owl:onProperty con:filling ],
        [ a owl:Restriction ;
            owl:maxQualifiedCardinality "1"^^xsd:nonNegativeInteger ;
            owl:onDataRange xsd:boolean ;
            owl:onProperty con:isStructuralElement ],
        [ a owl:Restriction ;
            owl:allValuesFrom xsd:boolean ;
            owl:onProperty con:isStructuralElement ],
        [ a owl:Restriction ;
            owl:allValuesFrom core:AbstractThematicSurface ;
            owl:onProperty <https://www.opengis.net/ont/citygml/common/boundary> ],
        core:AbstractOccupiedSpace .

con:ConstructionEvent a owl:Class ;
    rdfs:label "ConstructionEvent"@en ;
    rdfs:subClassOf [ a owl:Restriction ;
            owl:allValuesFrom xsd:date ;
            owl:onProperty con:dateOfEvent ],
        [ a owl:Restriction ;
            owl:onDataRange xsd:date ;
            owl:onProperty con:dateOfEvent ;
            owl:qualifiedCardinality "1"^^xsd:nonNegativeInteger ],
        [ a owl:Restriction ;
            owl:allValuesFrom con:EventValue ;
            owl:onProperty con:event ],
        [ a owl:Restriction ;
            owl:onClass con:EventValue ;
            owl:onProperty con:event ;
            owl:qualifiedCardinality "1"^^xsd:nonNegativeInteger ],
        [ a owl:Restriction ;
            owl:allValuesFrom xsd:string ;
            owl:onProperty <https://www.opengis.net/ont/citygml/common/description> ],
        [ a owl:Restriction ;
            owl:maxQualifiedCardinality "1"^^xsd:nonNegativeInteger ;
            owl:onDataRange xsd:string ;
            owl:onProperty <https://www.opengis.net/ont/citygml/common/description> ] ;
    skos:definition "A ConstructionEvent is a data type used to describe a specific event that is associated with a construction. Examples are the issuing of a building permit or the renovation of a building."@en .

con:Door a owl:Class ;
    rdfs:label "Door"@en ;
    rdfs:subClassOf [ a owl:Restriction ;
            owl:allValuesFrom con:DoorClassValue ;
            owl:onProperty <https://www.opengis.net/ont/citygml/common/class> ],
        [ a owl:Restriction ;
            owl:allValuesFrom core:Address ;
            owl:onProperty <https://www.opengis.net/ont/citygml/common/address> ],
        [ a owl:Restriction ;
            owl:allValuesFrom con:DoorFunctionValue ;
            owl:onProperty <https://www.opengis.net/ont/citygml/common/function> ],
        [ a owl:Restriction ;
            owl:maxQualifiedCardinality "1"^^xsd:nonNegativeInteger ;
            owl:onClass con:DoorClassValue ;
            owl:onProperty <https://www.opengis.net/ont/citygml/common/class> ],
        [ a owl:Restriction ;
            owl:allValuesFrom con:DoorUsageValue ;
            owl:onProperty <https://www.opengis.net/ont/citygml/common/usage> ],
        [ a owl:Restriction ;
            owl:allValuesFrom con:DoorSurface ;
            owl:onProperty <https://www.opengis.net/ont/citygml/common/boundary> ],
        con:AbstractFillingElement ;
    owl:disjointWith con:Window .

con:Elevation a owl:Class ;
    rdfs:label "Elevation"@en ;
    rdfs:subClassOf [ a owl:Restriction ;
            owl:allValuesFrom gmlowl:Point ;
            owl:onProperty con:elevationValue ],
        [ a owl:Restriction ;
            owl:onClass gmlowl:Point ;
            owl:onProperty con:elevationValue ;
            owl:qualifiedCardinality "1"^^xsd:nonNegativeInteger ],
        [ a owl:Restriction ;
            owl:allValuesFrom con:ElevationReferenceValue ;
            owl:onProperty con:elevationReference ],
        [ a owl:Restriction ;
            owl:onClass con:ElevationReferenceValue ;
            owl:onProperty con:elevationReference ;
            owl:qualifiedCardinality "1"^^xsd:nonNegativeInteger ] ;
    skos:definition "Elevation is a data type that includes the elevation value itself and information on how this elevation was measured. [cf. INSPIRE]"@en .

con:Height a owl:Class ;
    rdfs:label "Height"@en ;
    rdfs:subClassOf [ a owl:Restriction ;
            owl:allValuesFrom sc:Measure ;
            owl:onProperty <https://www.opengis.net/ont/citygml/common/value> ],
        [ a owl:Restriction ;
            owl:onDataRange sc:Measure ;
            owl:onProperty <https://www.opengis.net/ont/citygml/common/value> ;
            owl:qualifiedCardinality "1"^^xsd:nonNegativeInteger ],
        [ a owl:Restriction ;
            owl:onClass con:ElevationReferenceValue ;
            owl:onProperty <https://www.opengis.net/ont/citygml/common/lowReference> ;
            owl:qualifiedCardinality "1"^^xsd:nonNegativeInteger ],
        [ a owl:Restriction ;
            owl:allValuesFrom con:HeightStatusValue ;
            owl:onProperty <https://www.opengis.net/ont/citygml/common/status> ],
        [ a owl:Restriction ;
            owl:onDataRange con:HeightStatusValue ;
            owl:onProperty <https://www.opengis.net/ont/citygml/common/status> ;
            owl:qualifiedCardinality "1"^^xsd:nonNegativeInteger ],
        [ a owl:Restriction ;
            owl:allValuesFrom con:ElevationReferenceValue ;
            owl:onProperty <https://www.opengis.net/ont/citygml/common/lowReference> ],
        [ a owl:Restriction ;
            owl:allValuesFrom con:ElevationReferenceValue ;
            owl:onProperty <https://www.opengis.net/ont/citygml/common/highReference> ],
        [ a owl:Restriction ;
            owl:onClass con:ElevationReferenceValue ;
            owl:onProperty <https://www.opengis.net/ont/citygml/common/highReference> ;
            owl:qualifiedCardinality "1"^^xsd:nonNegativeInteger ] ;
    skos:definition "Height represents a vertical distance (measured or estimated) between a low reference and a high reference. [cf. INSPIRE]"@en .

con:Window a owl:Class ;
    rdfs:label "Window"@en ;
    rdfs:subClassOf [ a owl:Restriction ;
            owl:allValuesFrom con:DoorFunctionValue ;
            owl:onProperty <https://www.opengis.net/ont/citygml/common/function> ],
        [ a owl:Restriction ;
            owl:allValuesFrom con:DoorClassValue ;
            owl:onProperty <https://www.opengis.net/ont/citygml/common/class> ],
        [ a owl:Restriction ;
            owl:allValuesFrom con:WindowSurface ;
            owl:onProperty <https://www.opengis.net/ont/citygml/common/boundary> ],
        [ a owl:Restriction ;
            owl:allValuesFrom con:DoorUsageValue ;
            owl:onProperty <https://www.opengis.net/ont/citygml/common/usage> ],
        [ a owl:Restriction ;
            owl:maxQualifiedCardinality "1"^^xsd:nonNegativeInteger ;
            owl:onClass con:DoorClassValue ;
            owl:onProperty <https://www.opengis.net/ont/citygml/common/class> ],
        con:AbstractFillingElement .

con:conditionOfConstruction a owl:DatatypeProperty ;
    rdfs:label "conditionOfConstruction"@en ;
    rdfs:range con:ConditionOfConstructionValue ;
    skos:definition "Indicates the life-cycle status of the construction. [cf. INSPIRE]"@en .

con:dateOfConstruction a owl:DatatypeProperty ;
    rdfs:label "dateOfConstruction"@en ;
    rdfs:range xsd:date ;
    skos:definition "Indicates the date at which the construction was completed."@en .

con:dateOfDemolition a owl:DatatypeProperty ;
    rdfs:label "dateOfDemolition"@en ;
    rdfs:range xsd:date ;
    skos:definition "Indicates the date at which the construction was demolished."@en .

con:dateOfEvent a owl:DatatypeProperty ;
    rdfs:label "dateOfEvent"@en ;
    rdfs:range xsd:date ;
    skos:definition "Specifies the date at which the event took or will take place."@en .

con:elevationReference a owl:ObjectProperty ;
    rdfs:label "elevationReference"@en ;
    rdfs:range con:ElevationReferenceValue ;
    skos:definition "Specifies the level from which the elevation was measured. [cf. INSPIRE]"@en .

con:elevationValue a owl:ObjectProperty ;
    rdfs:label "elevationValue"@en ;
    rdfs:range gmlowl:Point ;
    skos:definition "Specifies the value of the elevation. [cf. INSPIRE]"@en .

con:event a owl:ObjectProperty ;
    rdfs:label "event"@en ;
    rdfs:range con:EventValue ;
    skos:definition "Indicates the specific event type."@en .

con:isStructuralElement a owl:DatatypeProperty ;
    rdfs:label "isStructuralElement"@en ;
    rdfs:range xsd:boolean ;
    skos:definition "Indicates whether the constructive element is essential from a structural point of view. A structural element cannot be omitted without collapsing of the construction. Examples are pylons and anchorages of bridges."@en .

con:relationToConstruction a owl:DatatypeProperty ;
    rdfs:label "relationToConstruction"@en ;
    rdfs:range con:RelationToConstruction ;
    skos:definition "Indicates whether the installation is located inside and/or outside of the construction."@en .

<https://www.opengis.net/ont/citygml/common/function> rdfs:label "function"@en ;
    skos:definition "Specifies the intended purposes of the Door."@en ;
    schema:rangeIncludes con:DoorFunctionValue .

<https://www.opengis.net/ont/citygml/common/usage> rdfs:label "usage"@en ;
    skos:definition "Specifies the actual uses of the Door."@en ;
    schema:rangeIncludes con:DoorUsageValue .

con:ConditionOfConstructionValue a rdfs:Datatype ;
    rdfs:label "ConditionOfConstructionValue"@en ;
    owl:equivalentClass [ a rdfs:Datatype ;
            owl:oneOf ( "declined" "demolished" "functional" "projected" "ruin" "underConstruction" ) ] ;
    skos:definition "ConditionOfConstructionValue enumerates different conditions of a construction. [cf. INSPIRE]"@en .

con:DoorSurface a owl:Class ;
    rdfs:label "DoorSurface"@en ;
    rdfs:subClassOf [ a owl:Restriction ;
            owl:allValuesFrom core:Address ;
            owl:onProperty <https://www.opengis.net/ont/citygml/common/address> ],
        con:AbstractFillingSurface ;
    owl:disjointWith con:WindowSurface .

con:EventValue a owl:Class ;
    rdfs:label "EventValue"@en ;
    rdfs:subClassOf skos:Concept ;
    skos:definition "EventValue is a code list that enumerates the different events of a construction."@en .

con:HeightStatusValue a rdfs:Datatype ;
    rdfs:label "HeightStatusValue"@en ;
    owl:equivalentClass [ a rdfs:Datatype ;
            owl:oneOf ( "estimated" "measured" ) ] ;
    skos:definition "HeightStatusValue enumerates the different methods used to capture a height. [cf. INSPIRE]"@en .

con:RelationToConstruction a rdfs:Datatype ;
    rdfs:label "RelationToConstruction"@en ;
    owl:equivalentClass [ a rdfs:Datatype ;
            owl:oneOf ( "inside" "outside" "bothInsideAndOutside" ) ] ;
    skos:definition "RelationToConstruction is an enumeration used to describe whether an installation is positioned inside and/or outside of a construction."@en .

con:WindowSurface a owl:Class ;
    rdfs:label "WindowSurface"@en ;
    rdfs:subClassOf con:AbstractFillingSurface .

con:AbstractFillingElement a owl:Class ;
    rdfs:label "AbstractFillingElement"@en ;
    iso19150-2:isAbstract true ;
    rdfs:subClassOf core:AbstractOccupiedSpace .

con:AbstractFillingSurface a owl:Class ;
    rdfs:label "AbstractFillingSurface"@en ;
    iso19150-2:isAbstract true ;
    rdfs:subClassOf core:AbstractThematicSurface .

con:DoorFunctionValue a owl:Class ;
    rdfs:label "DoorFunctionValue"@en ;
    rdfs:subClassOf skos:Concept ;
    skos:definition "DoorFunctionValue is a code list that enumerates the different purposes of a Door."@en .

con:DoorUsageValue a owl:Class ;
    rdfs:label "DoorUsageValue"@en ;
    rdfs:subClassOf skos:Concept ;
    skos:definition "DoorUsageValue is a code list that enumerates the different uses of a Door."@en .

<https://www.opengis.net/ont/citygml/common/boundary> skos:definition "Relates to the door surfaces that bound the Door. This relation is inherited from the Core module."@en,
        "Relates to the surfaces that bound the construction. This relation is inherited from the Core module."@en,
        "Relates to the surfaces that bound the constructive element. This relation is inherited from the Core module."@en,
        "Relates to the surfaces that bound the installation. This relation is inherited from the Core module."@en,
        "Relates to the window surfaces that bound the Window. This relation is inherited from the Core module."@en ;
    schema:domainIncludes con:AbstractConstruction,
        con:AbstractConstructiveElement,
        con:AbstractInstallation,
        con:Door,
        con:Window ;
    schema:rangeIncludes con:DoorSurface,
        con:WindowSurface,
        core:AbstractThematicSurface .

<https://www.opengis.net/ont/citygml/common/class> rdfs:label "class"@en ;
    skos:definition "Indicates the specific type of the Door."@en ;
    schema:rangeIncludes con:DoorClassValue .

con:DoorClassValue a owl:Class ;
    rdfs:label "DoorClassValue"@en ;
    rdfs:subClassOf skos:Concept ;
    skos:definition "DoorClassValue is a code list used to further classify a Door."@en .

con:AbstractConstructionSurface a owl:Class ;
    rdfs:label "AbstractConstructionSurface"@en ;
    iso19150-2:isAbstract true ;
    rdfs:subClassOf [ a owl:Restriction ;
            owl:allValuesFrom con:AbstractFillingSurface ;
            owl:onProperty con:fillingSurface ],
        core:AbstractThematicSurface .

con:ElevationReferenceValue a owl:Class ;
    rdfs:label "ElevationReferenceValue"@en ;
    rdfs:subClassOf skos:Concept ;
    skos:definition "ElevationReferenceValue is a code list that enumerates the different elevation reference levels used to measure construction heights."@en .

[] a owl:AllDisjointClasses ;
    owl:members ( brid:BridgeFurniture bldg:BuildingFurniture tun:TunnelFurniture ) .

[] a owl:AllDisjointClasses ;
    owl:members ( brid:BridgeConstructiveElement bldg:BuildingConstructiveElement tun:TunnelConstructiveElement ) .

[] a owl:AllDisjointClasses ;
    owl:members ( brid:AbstractBridge bldg:AbstractBuilding con:OtherConstruction tun:AbstractTunnel ) .

[] a owl:AllDisjointClasses ;
    owl:members ( brid:BridgeInstallation bldg:BuildingInstallation tun:TunnelInstallation ) .

[] a owl:AllDisjointClasses ;
    owl:members ( con:CeilingSurface con:FloorSurface con:GroundSurface con:InteriorWallSurface con:OuterCeilingSurface con:OuterFloorSurface con:RoofSurface con:WallSurface ) .

@prefix app: <https://www.opengis.net/ont/citygml/appearance/> .
@prefix bldg: <https://www.opengis.net/ont/citygml/building/> .
@prefix brid: <https://www.opengis.net/ont/citygml/bridge/> .
@prefix con: <https://www.opengis.net/ont/citygml/construction/> .
@prefix core: <https://www.opengis.net/ont/citygml/core/> .
@prefix dem: <https://www.opengis.net/ont/citygml/relief/> .
@prefix doc: <https://www.opengis.net/ont/citygml/document/> .
@prefix dyn: <https://www.opengis.net/ont/citygml/dynamizer/> .
@prefix frn: <https://www.opengis.net/ont/citygml/cityfurniture/> .
@prefix gen: <https://www.opengis.net/ont/citygml/generics/> .
@prefix geo: <http://www.opengis.net/ont/geosparql#> .
@prefix gmlowl: <http://www.opengis.net/ont/gml#> .
@prefix grp: <https://www.opengis.net/ont/citygml/cityobjectgroup/> .
@prefix iso19109: <http://def.isotc211.org/iso19109/2015/GeneralFeatureModel#> .
@prefix iso19111-2019: <http://def.isotc211.org/iso19111/2019/CoordinateReferenceSystems#> .
@prefix iso19150-2: <http://def.isotc211.org/iso19150/-2/2012/base#> .
@prefix luse: <https://www.opengis.net/ont/citygml/landuse/> .
@prefix owl: <http://www.w3.org/2002/07/owl#> .
@prefix rdf: <http://www.w3.org/1999/02/22-rdf-syntax-ns#> .
@prefix rdfs: <http://www.w3.org/2000/01/rdf-schema#> .
@prefix schema: <https://schema.org/> .
@prefix skos: <http://www.w3.org/2004/02/skos/core#> .
@prefix tran: <https://www.opengis.net/ont/citygml/transportation/> .
@prefix tun: <https://www.opengis.net/ont/citygml/tunnel/> .
@prefix veg: <https://www.opengis.net/ont/citygml/vegetation/> .
@prefix wksp: <https://www.opengis.net/ont/citygml/workspace/> .
@prefix wtr: <https://www.opengis.net/ont/citygml/waterbody/> .
@prefix xsd: <http://www.w3.org/2001/XMLSchema#> .

<https://www.opengis.net/ont/citygml/core> a owl:Ontology ;
    rdfs:label "Core"@en ;
    owl:imports <http://def.isotc211.org/iso19150/-2/2012/base>,
        <http://www.opengis.net/ont/gml>,
        <https://www.opengis.net/ont/citygml/appearance>,
        <https://www.opengis.net/ont/citygml/bridge>,
        <https://www.opengis.net/ont/citygml/building>,
        <https://www.opengis.net/ont/citygml/cityfurniture>,
        <https://www.opengis.net/ont/citygml/cityobjectgroup>,
        <https://www.opengis.net/ont/citygml/common>,
        <https://www.opengis.net/ont/citygml/construction>,
        <https://www.opengis.net/ont/citygml/document>,
        <https://www.opengis.net/ont/citygml/dynamizer>,
        <https://www.opengis.net/ont/citygml/generics>,
        <https://www.opengis.net/ont/citygml/landuse>,
        <https://www.opengis.net/ont/citygml/relief>,
        <https://www.opengis.net/ont/citygml/transportation>,
        <https://www.opengis.net/ont/citygml/tunnel>,
        <https://www.opengis.net/ont/citygml/vegetation>,
        <https://www.opengis.net/ont/citygml/waterbody>,
        <https://www.opengis.net/ont/citygml/workspace> ;
    owl:versionIRI <https://www.opengis.net/ont/citygml/core/3.0.0/> ;
    owl:versionInfo "3.0.0" ;
    skos:definition "The Core module defines the basic components of the CityGML conceptual model. This includes abstract base classes that define the core properties of more specialized thematic classes defined in other modules as well as concrete classes that are common to other modules, for example basic data types."@en .

core:AbstractLogicalSpace a owl:Class ;
    rdfs:label "AbstractLogicalSpace"@en ;
    iso19150-2:isAbstract true ;
    rdfs:subClassOf core:AbstractSpace ;
    owl:disjointWith core:AbstractPhysicalSpace .

core:DoubleBetween0and1 a owl:Class ;
    rdfs:label "DoubleBetween0and1"@en ;
    skos:definition "DoubleBetween0and1 is a basic type for values, which are greater or equal than 0 and less or equal than 1. The type is used for color encoding, for example."@en .

core:DoubleBetween0and1List a owl:Class ;
    rdfs:label "DoubleBetween0and1List"@en ;
    rdfs:subClassOf [ a owl:Restriction ;
            owl:allValuesFrom xsd:double ;
            owl:onProperty core:list ],
        [ a owl:Restriction ;
            owl:onDataRange xsd:double ;
            owl:onProperty core:list ;
            owl:qualifiedCardinality "1"^^xsd:nonNegativeInteger ] ;
    skos:definition "DoubleBetween0and1List is a basic type that represents a list of double values greater or equal than 0 and less or equal than 1. The type is used for color encoding, for example."@en .

core:DoubleOrNilReason a owl:Class ;
    rdfs:label "DoubleOrNilReason"@en ;
    rdfs:subClassOf [ a owl:Restriction ;
            owl:allValuesFrom core:NilReason ;
            owl:onProperty core:nilReason ],
        [ a owl:Restriction ;
            owl:allValuesFrom xsd:double ;
            owl:onProperty <https://www.opengis.net/ont/citygml/common/value> ],
        [ a owl:Class ;
            owl:unionOf ( [ a owl:Class ;
                        owl:intersectionOf ( [ a owl:Restriction ;
                                    owl:onDataRange xsd:double ;
                                    owl:onProperty <https://www.opengis.net/ont/citygml/common/value> ;
                                    owl:qualifiedCardinality "1"^^xsd:nonNegativeInteger ] [ a owl:Restriction ;
                                    owl:cardinality "0"^^xsd:nonNegativeInteger ;
                                    owl:onProperty core:nilReason ] ) ] [ a owl:Class ;
                        owl:intersectionOf ( [ a owl:Restriction ;
                                    owl:cardinality "0"^^xsd:nonNegativeInteger ;
                                    owl:onProperty <https://www.opengis.net/ont/citygml/common/value> ] [ a owl:Restriction ;
                                    owl:onClass core:NilReason ;
                                    owl:onProperty core:nilReason ;
                                    owl:qualifiedCardinality "1"^^xsd:nonNegativeInteger ] ) ] ) ] ;
    skos:definition "DoubleOrNilReason is a union type that allows for choosing between a double value and a nil reason."@en .

core:DoubleOrNilReasonList a owl:Class ;
    rdfs:label "DoubleOrNilReasonList"@en ;
    rdfs:subClassOf [ a owl:Restriction ;
            owl:allValuesFrom xsd:double ;
            owl:onProperty core:list ],
        [ a owl:Restriction ;
            owl:onDataRange xsd:double ;
            owl:onProperty core:list ;
            owl:qualifiedCardinality "1"^^xsd:nonNegativeInteger ] ;
    skos:definition "DoubleOrNilReasonList is a basic type that represents a list of double values and/or nil reasons."@en .

core:IntegerBetween0and3 a owl:Class ;
    rdfs:label "IntegerBetween0and3"@en ;
    skos:definition "IntegerBetween0and3 is a basic type for integer values, which are greater or equal than 0 and less or equal than 3. The type is used for encoding the LOD number."@en .

core:Occupancy a owl:Class ;
    rdfs:label "Occupancy"@en ;
    rdfs:subClassOf [ a owl:Restriction ;
            owl:allValuesFrom core:OccupantTypeValue ;
            owl:onProperty core:occupantType ],
        [ a owl:Restriction ;
            owl:maxQualifiedCardinality "1"^^xsd:nonNegativeInteger ;
            owl:onClass core:OccupantTypeValue ;
            owl:onProperty core:occupantType ],
        [ a owl:Restriction ;
            owl:allValuesFrom core:IntervalValue ;
            owl:onProperty core:interval ],
        [ a owl:Restriction ;
            owl:maxQualifiedCardinality "1"^^xsd:nonNegativeInteger ;
            owl:onClass core:IntervalValue ;
            owl:onProperty core:interval ],
        [ a owl:Restriction ;
            owl:allValuesFrom xsd:integer ;
            owl:onProperty core:numberOfOccupants ],
        [ a owl:Restriction ;
            owl:onDataRange xsd:integer ;
            owl:onProperty core:numberOfOccupants ;
            owl:qualifiedCardinality "1"^^xsd:nonNegativeInteger ] ;
    skos:definition "Occupancy is an application-dependent indication of what is contained by a feature."@en .

core:OtherRelationTypeValue a owl:Class ;
    rdfs:label "OtherRelationTypeValue"@en ;
    rdfs:subClassOf skos:Concept ;
    skos:definition "OtherRelationTypeValue is a code list used to classify other types of city object relations."@en .

core:TemporalRelationTypeValue a owl:Class ;
    rdfs:label "TemporalRelationTypeValue"@en ;
    rdfs:subClassOf skos:Concept ;
    skos:definition "TemporalRelationTypeValue is a code list used to classify temporal city object relations."@en .

core:TopologicalRelationTypeValue a owl:Class ;
    rdfs:label "TopologicalRelationTypeValue"@en ;
    rdfs:subClassOf skos:Concept ;
    skos:definition "TopologicalRelationTypeValue is a code list used to classify topological city object relations."@en .

core:creationDate a owl:DatatypeProperty ;
    rdfs:label "creationDate"@en ;
    rdfs:range xsd:dateTime ;
    skos:definition "Indicates the date at which a CityGML feature was added to the CityModel."@en .

core:terminationDate a owl:DatatypeProperty ;
    rdfs:label "terminationDate"@en ;
    rdfs:range xsd:dateTime ;
    skos:definition "Indicates the date at which a CityGML feature was removed from the CityModel."@en .

core:validFrom a owl:DatatypeProperty ;
    rdfs:label "validFrom"@en ;
    rdfs:range xsd:dateTime ;
    skos:definition "Indicates the date at which a CityGML feature started to exist in the real world."@en .

core:validTo a owl:DatatypeProperty ;
    rdfs:label "validTo"@en ;
    rdfs:range xsd:dateTime ;
    skos:definition "Indicates the date at which a CityGML feature ended to exist in the real world."@en .

<https://www.opengis.net/ont/citygml/common/boundary> skos:definition "Relates to surfaces that bound the space."@en ;
    schema:domainIncludes core:AbstractSpace ;
    schema:rangeIncludes core:AbstractSpaceBoundary .

<https://www.opengis.net/ont/citygml/common/name> rdfs:label "name"@en ;
    skos:definition "Specifies the name of the feature."@en ;
    schema:rangeIncludes xsd:Name .

core:AbstractUnoccupiedSpace a owl:Class ;
    rdfs:label "AbstractUnoccupiedSpace"@en ;
    iso19150-2:isAbstract true ;
    rdfs:subClassOf core:AbstractPhysicalSpace .

core:ClosureSurface a owl:Class ;
    rdfs:label "ClosureSurface"@en ;
    rdfs:subClassOf core:AbstractThematicSurface .

core:TransformationMatrix2x2 a owl:Class ;
    rdfs:label "TransformationMatrix2x2"@en ;
    rdfs:subClassOf core:DoubleList ;
    skos:definition "TransformationMatrix2x2 is a 2 by 2 matrix represented as a list of four double values in row major order."@en .

core:TransformationMatrix3x4 a owl:Class ;
    rdfs:label "TransformationMatrix3x4"@en ;
    rdfs:subClassOf core:DoubleList ;
    skos:definition "TransformationMatrix3x4 is a 3 by 4 matrix represented as a list of twelve double values in row major order."@en .

core:cityModelMember a owl:ObjectProperty ;
    rdfs:label "cityModelMember"@en ;
    rdfs:domain core:CityModel ;
    rdfs:range core:CityModelMember ;
    skos:definition "Relates to all objects that are part of the CityModel."@en .

core:dynamizer a owl:ObjectProperty ;
    rdfs:label "dynamizer"@en ;
    rdfs:domain core:AbstractCityObject ;
    rdfs:range core:AbstractDynamizer ;
    skos:definition "Relates Dynamizer objects to the city object. These allow timeseries data to override static attribute values of the city object."@en .

core:externalReference a owl:ObjectProperty ;
    rdfs:label "externalReference"@en ;
    rdfs:domain core:AbstractCityObject ;
    rdfs:range core:ExternalReference ;
    skos:definition "References external objects in other information systems that have a relation to the city object."@en .

core:generalizesTo a owl:ObjectProperty ;
    rdfs:label "generalizesTo"@en ;
    rdfs:domain core:AbstractCityObject ;
    rdfs:range core:AbstractCityObject ;
    skos:definition "Relates generalized representations of the same real-world object in different Levels of Detail to the city object. The direction of this relation is from the city object to the corresponding generalized city objects."@en .

<https://www.opengis.net/ont/citygml/common/appearance> skos:definition "Relates appearances to the ImplicitGeometry."@en,
        "Relates appearances to the city object."@en ;
    schema:domainIncludes core:AbstractCityObject,
        core:ImplicitGeometry ;
    schema:rangeIncludes core:AbstractAppearance .

<https://www.opengis.net/ont/citygml/common/description> rdfs:label "description"@en ;
    skos:definition "Provides further information on the feature."@en ;
    schema:rangeIncludes xsd:string .

<https://www.opengis.net/ont/citygml/common/genericAttribute> skos:definition "Relates generic attributes to the CityObjectRelation."@en,
        "Relates generic attributes to the city object."@en ;
    schema:domainIncludes core:AbstractCityObject,
        core:CityObjectRelation ;
    schema:rangeIncludes core:AbstractGenericAttribute .

<https://www.opengis.net/ont/citygml/common/mimeType> rdfs:label "mimeType"@en ;
    skos:definition "Specifies the MIME type of the external file that stores the prototypical geometry."@en ;
    schema:rangeIncludes core:MimeTypeValue .

<https://www.opengis.net/ont/citygml/common/referencePoint> skos:definition "Relates to a 3D Point geometry that represents the base point of the object in the world coordinate system."@en ;
    schema:domainIncludes core:ImplicitGeometry ;
    schema:rangeIncludes gmlowl:Point .

core:CityModel a owl:Class ;
    rdfs:label "CityModel"@en ;
    rdfs:subClassOf [ a owl:Restriction ;
            owl:allValuesFrom core:CityModelMember ;
            owl:onProperty core:cityModelMember ],
        [ a owl:Restriction ;
            owl:allValuesFrom iso19111-2019:EngineeringCRS ;
            owl:onProperty core:engineeringCRS ],
        [ a owl:Restriction ;
            owl:maxQualifiedCardinality "1"^^xsd:nonNegativeInteger ;
            owl:onClass iso19111-2019:EngineeringCRS ;
            owl:onProperty core:engineeringCRS ],
        core:AbstractFeatureWithLifespan .

core:CityModelMember a owl:Class ;
    rdfs:label "CityModelMember"@en ;
    rdfs:subClassOf [ a owl:Restriction ;
            owl:allValuesFrom core:AbstractFeature ;
            owl:onProperty core:featureMember ],
        [ a owl:Restriction ;
            owl:allValuesFrom core:AbstractVersionTransition ;
            owl:onProperty core:versionTransitionMember ],
        [ a owl:Restriction ;
            owl:allValuesFrom core:AbstractVersion ;
            owl:onProperty core:versionMember ],
        [ a owl:Restriction ;
            owl:allValuesFrom core:AbstractAppearance ;
            owl:onProperty core:appearanceMember ],
        [ a owl:Restriction ;
            owl:allValuesFrom core:AbstractCityObject ;
            owl:onProperty core:cityObjectMember ],
        [ a owl:Class ;
            owl:unionOf ( [ a owl:Class ;
                        owl:intersectionOf ( [ a owl:Restriction ;
                                    owl:onClass core:AbstractCityObject ;
                                    owl:onProperty core:cityObjectMember ;
                                    owl:qualifiedCardinality "1"^^xsd:nonNegativeInteger ] [ a owl:Restriction ;
                                    owl:cardinality "0"^^xsd:nonNegativeInteger ;
                                    owl:onProperty core:appearanceMember ] [ a owl:Restriction ;
                                    owl:cardinality "0"^^xsd:nonNegativeInteger ;
                                    owl:onProperty core:versionMember ] [ a owl:Restriction ;
                                    owl:cardinality "0"^^xsd:nonNegativeInteger ;
                                    owl:onProperty core:versionTransitionMember ] [ a owl:Restriction ;
                                    owl:cardinality "0"^^xsd:nonNegativeInteger ;
                                    owl:onProperty core:featureMember ] ) ] [ a owl:Class ;
                        owl:intersectionOf ( [ a owl:Restriction ;
                                    owl:cardinality "0"^^xsd:nonNegativeInteger ;
                                    owl:onProperty core:cityObjectMember ] [ a owl:Restriction ;
                                    owl:onClass core:AbstractAppearance ;
                                    owl:onProperty core:appearanceMember ;
                                    owl:qualifiedCardinality "1"^^xsd:nonNegativeInteger ] [ a owl:Restriction ;
                                    owl:cardinality "0"^^xsd:nonNegativeInteger ;
                                    owl:onProperty core:versionMember ] [ a owl:Restriction ;
                                    owl:cardinality "0"^^xsd:nonNegativeInteger ;
                                    owl:onProperty core:versionTransitionMember ] [ a owl:Restriction ;
                                    owl:cardinality "0"^^xsd:nonNegativeInteger ;
                                    owl:onProperty core:featureMember ] ) ] [ a owl:Class ;
                        owl:intersectionOf ( [ a owl:Restriction ;
                                    owl:cardinality "0"^^xsd:nonNegativeInteger ;
                                    owl:onProperty core:cityObjectMember ] [ a owl:Restriction ;
                                    owl:cardinality "0"^^xsd:nonNegativeInteger ;
                                    owl:onProperty core:appearanceMember ] [ a owl:Restriction ;
                                    owl:onClass core:AbstractVersion ;
                                    owl:onProperty core:versionMember ;
                                    owl:qualifiedCardinality "1"^^xsd:nonNegativeInteger ] [ a owl:Restriction ;
                                    owl:cardinality "0"^^xsd:nonNegativeInteger ;
                                    owl:onProperty core:versionTransitionMember ] [ a owl:Restriction ;
                                    owl:cardinality "0"^^xsd:nonNegativeInteger ;
                                    owl:onProperty core:featureMember ] ) ] [ a owl:Class ;
                        owl:intersectionOf ( [ a owl:Restriction ;
                                    owl:cardinality "0"^^xsd:nonNegativeInteger ;
                                    owl:onProperty core:cityObjectMember ] [ a owl:Restriction ;
                                    owl:cardinality "0"^^xsd:nonNegativeInteger ;
                                    owl:onProperty core:appearanceMember ] [ a owl:Restriction ;
                                    owl:cardinality "0"^^xsd:nonNegativeInteger ;
                                    owl:onProperty core:versionMember ] [ a owl:Restriction ;
                                    owl:onClass core:AbstractVersionTransition ;
                                    owl:onProperty core:versionTransitionMember ;
                                    owl:qualifiedCardinality "1"^^xsd:nonNegativeInteger ] [ a owl:Restriction ;
                                    owl:cardinality "0"^^xsd:nonNegativeInteger ;
                                    owl:onProperty core:featureMember ] ) ] [ a owl:Class ;
                        owl:intersectionOf ( [ a owl:Restriction ;
                                    owl:cardinality "0"^^xsd:nonNegativeInteger ;
                                    owl:onProperty core:cityObjectMember ] [ a owl:Restriction ;
                                    owl:cardinality "0"^^xsd:nonNegativeInteger ;
                                    owl:onProperty core:appearanceMember ] [ a owl:Restriction ;
                                    owl:cardinality "0"^^xsd:nonNegativeInteger ;
                                    owl:onProperty core:versionMember ] [ a owl:Restriction ;
                                    owl:cardinality "0"^^xsd:nonNegativeInteger ;
                                    owl:onProperty core:versionTransitionMember ] [ a owl:Restriction ;
                                    owl:onClass core:AbstractFeature ;
                                    owl:onProperty core:featureMember ;
                                    owl:qualifiedCardinality "1"^^xsd:nonNegativeInteger ] ) ] ) ] ;
    skos:definition "CityModelMember is a union type that enumerates the different types of objects that can occur as members of a city model."@en .

core:ExternalReference a owl:Class ;
    rdfs:label "ExternalReference"@en ;
    rdfs:subClassOf [ a owl:Restriction ;
            owl:allValuesFrom xsd:anyURI ;
            owl:onProperty core:informationSystem ],
        [ a owl:Restriction ;
            owl:maxQualifiedCardinality "1"^^xsd:nonNegativeInteger ;
            owl:onDataRange xsd:anyURI ;
            owl:onProperty core:informationSystem ],
        [ a owl:Restriction ;
            owl:allValuesFrom xsd:anyURI ;
            owl:onProperty core:targetResource ],
        [ a owl:Restriction ;
            owl:onDataRange xsd:anyURI ;
            owl:onProperty core:targetResource ;
            owl:qualifiedCardinality "1"^^xsd:nonNegativeInteger ],
        [ a owl:Restriction ;
            owl:allValuesFrom core:RelationTypeValue ;
            owl:onProperty core:relationType ],
        [ a owl:Restriction ;
            owl:maxQualifiedCardinality "1"^^xsd:nonNegativeInteger ;
            owl:onClass core:RelationTypeValue ;
            owl:onProperty core:relationType ] ;
    skos:definition "ExternalReference is a reference to a corresponding object in another information system, for example in the German cadastre (ALKIS), the German topographic information system (ATKIS), or the OS UK MasterMap®."@en .

core:engineeringCRS a owl:ObjectProperty ;
    rdfs:label "engineeringCRS"@en ;
    rdfs:range iso19111-2019:EngineeringCRS ;
    skos:definition "Specifies the local engineering coordinate reference system of the CityModel that can be provided inline the CityModel instead of referencing a well-known CRS definition. The definition of an engineering CRS requires an anchor point which relates the origin of the local coordinate system to a point on the earth’s surface in order to facilitate the transformation of coordinates from the local engineering CRS."@en .

core:featureID a owl:ObjectProperty ;
    rdfs:label "featureID"@en ;
    rdfs:range core:ID ;
    skos:definition "Specifies the unique identifier of the feature that is valid in the instance document within which it occurs."@en .

core:identifier a owl:ObjectProperty ;
    rdfs:label "identifier"@en ;
    rdfs:range rdfs:Resource ;
    skos:definition "Specifies the unique identifier of the feature that is valid globally."@en .

core:informationSystem a owl:DatatypeProperty ;
    rdfs:label "informationSystem"@en ;
    rdfs:range xsd:anyURI ;
    skos:definition "Specifies the URI that points to the external information system."@en .

core:interval a owl:ObjectProperty ;
    rdfs:label "interval"@en ;
    rdfs:range core:IntervalValue ;
    skos:definition "Indicates the time period the occupants are contained by a feature."@en .

core:libraryObject a owl:DatatypeProperty ;
    rdfs:label "libraryObject"@en ;
    rdfs:range xsd:anyURI ;
    skos:definition "Specifies the URI that points to the prototypical geometry stored in an external file."@en .

core:lod0Point a owl:ObjectProperty ;
    rdfs:label "lod0Point"@en ;
    rdfs:domain core:AbstractSpace ;
    rdfs:range gmlowl:Point ;
    rdfs:subPropertyOf geo:hasGeometry ;
    skos:definition "Relates to a 3D Point geometry that represents the space in Level of Detail 0."@en .

core:lod1ImplicitRepresentation a owl:ObjectProperty ;
    rdfs:label "lod1ImplicitRepresentation"@en ;
    rdfs:domain core:AbstractOccupiedSpace ;
    rdfs:range core:ImplicitGeometry ;
    skos:definition "Relates to an implicit geometry that represents the occupied space in Level of Detail 1."@en .

core:lod1MultiSurface a owl:ObjectProperty ;
    rdfs:label "lod1MultiSurface"@en ;
    rdfs:domain core:AbstractThematicSurface ;
    rdfs:range gmlowl:MultiSurface ;
    rdfs:subPropertyOf geo:hasGeometry ;
    skos:definition "Relates to a 3D MultiSurface geometry that represents the thematic surface in Level of Detail 1."@en .

core:lod1Solid a owl:ObjectProperty ;
    rdfs:label "lod1Solid"@en ;
    rdfs:domain core:AbstractSpace ;
    rdfs:range gmlowl:Solid ;
    rdfs:subPropertyOf geo:hasGeometry ;
    skos:definition "Relates to a 3D Solid geometry that represents the space in Level of Detail 1."@en .

core:lod1TerrainIntersectionCurve a owl:ObjectProperty ;
    rdfs:label "lod1TerrainIntersectionCurve"@en ;
    rdfs:domain core:AbstractPhysicalSpace ;
    rdfs:range gmlowl:MultiCurve ;
    skos:definition "Relates to a 3D MultiCurve geometry that represents the terrain intersection curve of the physical space in Level of Detail 1."@en .

core:lod2ImplicitRepresentation a owl:ObjectProperty ;
    rdfs:label "lod2ImplicitRepresentation"@en ;
    rdfs:domain core:AbstractOccupiedSpace ;
    rdfs:range core:ImplicitGeometry ;
    skos:definition "Relates to an implicit geometry that represents the occupied space in Level of Detail 2."@en .

core:lod2MultiCurve a owl:ObjectProperty ;
    rdfs:label "lod2MultiCurve"@en ;
    rdfs:domain core:AbstractSpace ;
    rdfs:range gmlowl:MultiCurve ;
    rdfs:subPropertyOf geo:hasGeometry ;
    skos:definition "Relates to a 3D MultiCurve geometry that represents the space in Level of Detail 2."@en .

core:lod2Solid a owl:ObjectProperty ;
    rdfs:label "lod2Solid"@en ;
    rdfs:domain core:AbstractSpace ;
    rdfs:range gmlowl:Solid ;
    rdfs:subPropertyOf geo:hasGeometry ;
    skos:definition "Relates to a 3D Solid geometry that represents the space in Level of Detail 2."@en .

core:lod2TerrainIntersectionCurve a owl:ObjectProperty ;
    rdfs:label "lod2TerrainIntersectionCurve"@en ;
    rdfs:domain core:AbstractPhysicalSpace ;
    rdfs:range gmlowl:MultiCurve ;
    skos:definition "Relates to a 3D MultiCurve geometry that represents the terrain intersection curve of the physical space in Level of Detail 2."@en .

core:lod3ImplicitRepresentation a owl:ObjectProperty ;
    rdfs:label "lod3ImplicitRepresentation"@en ;
    rdfs:domain core:AbstractOccupiedSpace ;
    rdfs:range core:ImplicitGeometry ;
    skos:definition "Relates to an implicit geometry that represents the occupied space in Level of Detail 3."@en .

core:lod3MultiCurve a owl:ObjectProperty ;
    rdfs:label "lod3MultiCurve"@en ;
    rdfs:domain core:AbstractSpace ;
    rdfs:range gmlowl:MultiCurve ;
    rdfs:subPropertyOf geo:hasGeometry ;
    skos:definition "Relates to a 3D MultiCurve geometry that represents the space in Level of Detail 3."@en .

core:lod3Solid a owl:ObjectProperty ;
    rdfs:label "lod3Solid"@en ;
    rdfs:domain core:AbstractSpace ;
    rdfs:range gmlowl:Solid ;
    rdfs:subPropertyOf geo:hasGeometry ;
    skos:definition "Relates to a 3D Solid geometry that represents the space in Level of Detail 3."@en .

core:lod3TerrainIntersectionCurve a owl:ObjectProperty ;
    rdfs:label "lod3TerrainIntersectionCurve"@en ;
    rdfs:domain core:AbstractPhysicalSpace ;
    rdfs:range gmlowl:MultiCurve ;
    skos:definition "Relates to a 3D MultiCurve geometry that represents the terrain intersection curve of the physical space in Level of Detail 3."@en .

core:multiPoint a owl:ObjectProperty ;
    rdfs:label "multiPoint"@en ;
    rdfs:domain core:Address ;
    rdfs:range gmlowl:MultiPoint ;
    rdfs:subPropertyOf geo:hasGeometry ;
    skos:definition "Relates to the MultiPoint geometry of the Address. The geometry relates the address spatially to a city object."@en .

core:numberOfOccupants a owl:DatatypeProperty ;
    rdfs:label "numberOfOccupants"@en ;
    rdfs:range xsd:integer ;
    skos:definition "Indicates the number of occupants contained by a feature."@en .

core:objectID a owl:ObjectProperty ;
    rdfs:label "objectID"@en ;
    rdfs:range core:ID ;
    skos:definition "Specifies the unique identifier of the ImplicitGeometry."@en .

core:occupantType a owl:ObjectProperty ;
    rdfs:label "occupantType"@en ;
    rdfs:range core:OccupantTypeValue ;
    skos:definition "Indicates the specific type of the occupants that are contained by a feature."@en .

core:relativeGeometry a owl:ObjectProperty ;
    rdfs:label "relativeGeometry"@en ;
    rdfs:domain core:ImplicitGeometry ;
    rdfs:range gmlowl:AbstractGeometry ;
    rdfs:subPropertyOf geo:hasGeometry ;
    skos:definition "Relates to a prototypical geometry in a local coordinate system stored inline with the city model."@en .

core:relativeToTerrain a owl:DatatypeProperty ;
    rdfs:label "relativeToTerrain"@en ;
    rdfs:range core:RelativeToTerrain ;
    skos:definition "Describes the vertical position of the city object relative to the surrounding terrain."@en .

core:relativeToWater a owl:DatatypeProperty ;
    rdfs:label "relativeToWater"@en ;
    rdfs:range core:RelativeToWater ;
    skos:definition "Describes the vertical position of the city object relative to the surrounding water surface."@en .

core:spaceType a owl:DatatypeProperty ;
    rdfs:label "spaceType"@en ;
    rdfs:range core:SpaceType ;
    skos:definition "Specifies the degree of openness of a space."@en .

core:targetResource a owl:DatatypeProperty ;
    rdfs:label "targetResource"@en ;
    rdfs:range xsd:anyURI ;
    skos:definition "Specifies the URI that points to the object in the external information system."@en .

core:transformationMatrix a owl:ObjectProperty ;
    rdfs:label "transformationMatrix"@en ;
    rdfs:range core:TransformationMatrix4x4 ;
    skos:definition "Specifies the mathematical transformation (translation, rotation, and scaling) between the prototypical geometry and the actual spatial position of the object."@en .

core:typeOfArea a owl:ObjectProperty ;
    rdfs:label "typeOfArea"@en ;
    rdfs:range core:QualifiedAreaTypeValue ;
    skos:definition "Indicates the specific type of the QualifiedArea."@en .

core:typeOfVolume a owl:ObjectProperty ;
    rdfs:label "typeOfVolume"@en ;
    rdfs:range core:QualifiedVolumeTypeValue ;
    skos:definition "Indicates the specific type of the QualifiedVolume."@en .

core:xalAddress a owl:ObjectProperty ;
    rdfs:label "xalAddress"@en ;
    rdfs:domain core:Address ;
    rdfs:range core:XALAddress ;
    skos:definition "Relates an OASIS address object to the Address."@en .

<https://www.opengis.net/ont/citygml/common/relatedTo> skos:definition "Relates other city objects to the city object. It also describes how the city objects are related to each other."@en ;
    schema:domainIncludes core:AbstractCityObject,
        core:CityObjectRelation ;
    schema:rangeIncludes core:AbstractCityObject,
        core:CityObjectRelation .

<https://www.opengis.net/ont/citygml/common/value> rdfs:label "value"@en ;
    skos:definition "Specifies the double value."@en ;
    schema:rangeIncludes xsd:double .

core:AbstractDynamizer a owl:Class ;
    rdfs:label "AbstractDynamizer"@en ;
    iso19150-2:isAbstract true ;
    rdfs:subClassOf core:AbstractFeatureWithLifespan .

core:AbstractGenericAttribute a owl:Class ;
    rdfs:label "AbstractGenericAttribute"@en ;
    iso19150-2:isAbstract true ;
    skos:definition "AbstractGenericAttribute is the abstract superclass for all types of generic attributes."@en .

core:AbstractOccupiedSpace a owl:Class ;
    rdfs:label "AbstractOccupiedSpace"@en ;
    iso19150-2:isAbstract true ;
    rdfs:subClassOf [ a owl:Restriction ;
            owl:maxQualifiedCardinality "1"^^xsd:nonNegativeInteger ;
            owl:onClass core:ImplicitGeometry ;
            owl:onProperty core:lod3ImplicitRepresentation ],
        [ a owl:Restriction ;
            owl:allValuesFrom core:ImplicitGeometry ;
            owl:onProperty core:lod3ImplicitRepresentation ],
        [ a owl:Restriction ;
            owl:maxQualifiedCardinality "1"^^xsd:nonNegativeInteger ;
            owl:onClass core:ImplicitGeometry ;
            owl:onProperty core:lod2ImplicitRepresentation ],
        [ a owl:Restriction ;
            owl:maxQualifiedCardinality "1"^^xsd:nonNegativeInteger ;
            owl:onClass core:ImplicitGeometry ;
            owl:onProperty core:lod1ImplicitRepresentation ],
        [ a owl:Restriction ;
            owl:allValuesFrom core:ImplicitGeometry ;
            owl:onProperty core:lod1ImplicitRepresentation ],
        [ a owl:Restriction ;
            owl:allValuesFrom core:ImplicitGeometry ;
            owl:onProperty core:lod2ImplicitRepresentation ],
        core:AbstractPhysicalSpace ;
    owl:disjointWith core:AbstractUnoccupiedSpace .

core:Address a owl:Class ;
    rdfs:label "Address"@en ;
    rdfs:subClassOf [ a owl:Restriction ;
            owl:allValuesFrom gmlowl:MultiPoint ;
            owl:onProperty core:multiPoint ],
        [ a owl:Restriction ;
            owl:maxQualifiedCardinality "1"^^xsd:nonNegativeInteger ;
            owl:onClass gmlowl:MultiPoint ;
            owl:onProperty core:multiPoint ],
        [ a owl:Restriction ;
            owl:allValuesFrom core:XALAddress ;
            owl:onProperty core:xalAddress ],
        [ a owl:Restriction ;
            owl:onClass core:XALAddress ;
            owl:onProperty core:xalAddress ;
            owl:qualifiedCardinality "1"^^xsd:nonNegativeInteger ],
        core:AbstractFeature .

core:DoubleList a owl:Class ;
    rdfs:label "DoubleList"@en ;
    rdfs:subClassOf [ a owl:Restriction ;
            owl:allValuesFrom xsd:double ;
            owl:onProperty core:list ],
        [ a owl:Restriction ;
            owl:onDataRange xsd:double ;
            owl:onProperty core:list ;
            owl:qualifiedCardinality "1"^^xsd:nonNegativeInteger ] ;
    skos:definition "DoubleList is an ordered sequence of double values."@en .

core:IntervalValue a owl:Class ;
    rdfs:label "IntervalValue"@en ;
    rdfs:subClassOf skos:Concept ;
    skos:definition "IntervalValue is a code list used to specify a time period."@en .

core:MimeTypeValue a owl:Class ;
    rdfs:label "MimeTypeValue"@en ;
    rdfs:subClassOf skos:Concept ;
    skos:definition "MimeTypeValue is a code list used to specify the MIME type of a referenced resource."@en .

core:NilReason a owl:Class ;
    rdfs:label "NilReason"@en ;
    rdfs:subClassOf [ a owl:Class ;
            owl:unionOf ( [ a owl:Class ;
                        owl:intersectionOf ( [ a owl:Restriction ;
                                    owl:onClass core:NilReasonEnumeration ;
                                    owl:onProperty core:nilReasonEnumeration ;
                                    owl:qualifiedCardinality "1"^^xsd:nonNegativeInteger ] [ a owl:Restriction ;
                                    owl:cardinality "0"^^xsd:nonNegativeInteger ;
                                    owl:onProperty core:uRI ] ) ] [ a owl:Class ;
                        owl:intersectionOf ( [ a owl:Restriction ;
                                    owl:cardinality "0"^^xsd:nonNegativeInteger ;
                                    owl:onProperty core:nilReasonEnumeration ] [ a owl:Restriction ;
                                    owl:onDataRange xsd:anyURI ;
                                    owl:onProperty core:uRI ;
                                    owl:qualifiedCardinality "1"^^xsd:nonNegativeInteger ] ) ] ) ],
        [ a owl:Restriction ;
            owl:allValuesFrom xsd:anyURI ;
            owl:onProperty core:uRI ],
        [ a owl:Restriction ;
            owl:allValuesFrom core:NilReasonEnumeration ;
            owl:onProperty core:nilReasonEnumeration ] ;
    skos:definition "NilReason is a union type that allows for choosing between two different types of nil reason."@en .

core:NilReasonEnumeration a owl:Class ;
    rdfs:label "NilReasonEnumeration"@en ;
    rdfs:subClassOf skos:Concept ;
    skos:definition "NilReasonEnumeration is a code list that enumerates the different nil reasons."@en .

core:OccupantTypeValue a owl:Class ;
    rdfs:label "OccupantTypeValue"@en ;
    rdfs:subClassOf skos:Concept ;
    skos:definition "OccupantTypeValue is a code list used to classify occupants."@en .

core:QualifiedAreaTypeValue a owl:Class ;
    rdfs:label "QualifiedAreaTypeValue"@en ;
    rdfs:subClassOf skos:Concept ;
    skos:definition "QualifiedAreaTypeValue is a code list used to specify area types."@en .

core:QualifiedVolumeTypeValue a owl:Class ;
    rdfs:label "QualifiedVolumeTypeValue"@en ;
    rdfs:subClassOf skos:Concept ;
    skos:definition "QualifiedVolumeTypeValue is a code list used to specify volume types."@en .

core:RelativeToTerrain a rdfs:Datatype ;
    rdfs:label "RelativeToTerrain"@en ;
    owl:equivalentClass [ a rdfs:Datatype ;
            owl:oneOf ( "entirelyAboveTerrain" "substantiallyAboveTerrain" "substantiallyAboveAndBelowTerrain" "substantiallyBelowTerrain" "entirelyBelowTerrain" ) ] ;
    skos:definition "RelativeToTerrain enumerates the spatial relations of a city object relative to terrain in a qualitative way."@en .

core:RelativeToWater a rdfs:Datatype ;
    rdfs:label "RelativeToWater"@en ;
    owl:equivalentClass [ a rdfs:Datatype ;
            owl:oneOf ( "entirelyAboveWaterSurface" "substantiallyAboveWaterSurface" "substantiallyAboveAndBelowWaterSurface" "substantiallyBelowWaterSurface" "entirelyBelowWaterSurface" "temporarilyAboveAndBelowWaterSurface" ) ] ;
    skos:definition "RelativeToWater enumerates the spatial relations of a city object relative to the water surface in a qualitative way."@en .

core:SpaceType a rdfs:Datatype ;
    rdfs:label "SpaceType"@en ;
    owl:equivalentClass [ a rdfs:Datatype ;
            owl:oneOf ( "closed" "open" "semiOpen" ) ] ;
    skos:definition "SpaceType is an enumeration that characterises a space according to its closure properties."@en .

core:XALAddress a owl:Class ;
    rdfs:label "XALAddress"@en ;
    skos:definition "XALAddress represents address details according to the OASIS xAL standard."@en .

core:nilReason a owl:ObjectProperty ;
    rdfs:label "nilReason"@en ;
    rdfs:range core:NilReason ;
    skos:definition "Specifies the nil reason."@en .

core:nilReasonEnumeration a owl:ObjectProperty ;
    rdfs:label "nilReasonEnumeration"@en ;
    rdfs:range core:NilReasonEnumeration ;
    skos:definition "Indicates a nil reason that is provided in a code list."@en .

core:uRI a owl:DatatypeProperty ;
    rdfs:label "URI"@en ;
    rdfs:range xsd:anyURI ;
    skos:definition "Specifies a URI that points to a resource that describes the nil reason."@en .

core:volume a owl:ObjectProperty ;
    rdfs:label "volume"@en ;
    rdfs:range core:QualifiedVolume ;
    skos:definition "Specifies qualified volumes related to the space."@en .

<https://www.opengis.net/ont/citygml/common/area> rdfs:label "area"@en ;
    skos:definition "Specifies qualified areas related to the space."@en ;
    schema:rangeIncludes core:QualifiedArea .

<https://www.opengis.net/ont/citygml/common/lod0MultiCurve> skos:definition "Relates to a 3D MultiCurve geometry that represents the space in Level of Detail 0."@en,
        "Relates to a 3D MultiCurve geometry that represents the thematic surface in Level of Detail 0."@en ;
    schema:domainIncludes core:AbstractSpace,
        core:AbstractThematicSurface ;
    schema:rangeIncludes gmlowl:MultiCurve .

<https://www.opengis.net/ont/citygml/common/lod0MultiSurface> skos:definition "Relates to a 3D MultiSurface geometry that represents the space in Level of Detail 0."@en,
        "Relates to a 3D MultiSurface geometry that represents the thematic surface in Level of Detail 0."@en ;
    schema:domainIncludes core:AbstractSpace,
        core:AbstractThematicSurface ;
    schema:rangeIncludes gmlowl:MultiSurface .

<https://www.opengis.net/ont/citygml/common/lod2MultiSurface> skos:definition "Relates to a 3D MultiSurface geometry that represents the space in Level of Detail 2."@en,
        "Relates to a 3D MultiSurface geometry that represents the thematic surface in Level of Detail 2."@en ;
    schema:domainIncludes core:AbstractSpace,
        core:AbstractThematicSurface ;
    schema:rangeIncludes gmlowl:MultiSurface .

<https://www.opengis.net/ont/citygml/common/lod3MultiSurface> skos:definition "Relates to a 3D MultiSurface geometry that represents the space in Level of Detail 3."@en,
        "Relates to a 3D MultiSurface geometry that represents the thematic surface in Level of Detail 3."@en ;
    schema:domainIncludes core:AbstractSpace,
        core:AbstractThematicSurface ;
    schema:rangeIncludes gmlowl:MultiSurface .

<https://www.opengis.net/ont/citygml/common/pointCloud> skos:definition "Relates to a 3D PointCloud that represents the physical space."@en,
        "Relates to a 3D PointCloud that represents the thematic surface."@en ;
    schema:domainIncludes core:AbstractPhysicalSpace,
        core:AbstractThematicSurface ;
    schema:rangeIncludes core:AbstractPointCloud .

core:AbstractSpaceBoundary a owl:Class ;
    rdfs:label "AbstractSpaceBoundary"@en ;
    iso19150-2:isAbstract true ;
    rdfs:subClassOf core:AbstractCityObject .

core:AbstractVersion a owl:Class ;
    rdfs:label "AbstractVersion"@en ;
    iso19150-2:isAbstract true ;
    rdfs:subClassOf core:AbstractFeatureWithLifespan .

core:AbstractVersionTransition a owl:Class ;
    rdfs:label "AbstractVersionTransition"@en ;
    iso19150-2:isAbstract true ;
    rdfs:subClassOf core:AbstractFeatureWithLifespan .

core:CityObjectRelation a owl:Class ;
    rdfs:label "CityObjectRelation"@en ;
    rdfs:subClassOf [ a owl:Restriction ;
            owl:allValuesFrom core:AbstractCityObject ;
            owl:onProperty <https://www.opengis.net/ont/citygml/common/relatedTo> ],
        [ a owl:Restriction ;
            owl:onClass core:AbstractCityObject ;
            owl:onProperty <https://www.opengis.net/ont/citygml/common/relatedTo> ;
            owl:qualifiedCardinality "1"^^xsd:nonNegativeInteger ],
        [ a owl:Restriction ;
            owl:allValuesFrom core:RelationTypeValue ;
            owl:onProperty core:relationType ],
        [ a owl:Restriction ;
            owl:onClass core:RelationTypeValue ;
            owl:onProperty core:relationType ;
            owl:qualifiedCardinality "1"^^xsd:nonNegativeInteger ],
        [ a owl:Restriction ;
            owl:allValuesFrom core:AbstractGenericAttribute ;
            owl:onProperty <https://www.opengis.net/ont/citygml/common/genericAttribute> ] ;
    skos:definition "CityObjectRelation represents a specific relation from the city object in which the relation is included to another city object."@en .

core:QualifiedVolume a owl:Class ;
    rdfs:label "QualifiedVolume"@en ;
    rdfs:subClassOf [ a owl:Restriction ;
            owl:onClass core:QualifiedVolume ;
            owl:onProperty core:volume ;
            owl:qualifiedCardinality "1"^^xsd:nonNegativeInteger ],
        [ a owl:Restriction ;
            owl:allValuesFrom core:QualifiedVolumeTypeValue ;
            owl:onProperty core:typeOfVolume ],
        [ a owl:Restriction ;
            owl:onClass core:QualifiedVolumeTypeValue ;
            owl:onProperty core:typeOfVolume ;
            owl:qualifiedCardinality "1"^^xsd:nonNegativeInteger ],
        [ a owl:Restriction ;
            owl:allValuesFrom core:QualifiedVolume ;
            owl:onProperty core:volume ] ;
    skos:definition "QualifiedVolume is an application-dependent measure of the volume of a space."@en .

core:TransformationMatrix4x4 a owl:Class ;
    rdfs:label "TransformationMatrix4x4"@en ;
    rdfs:subClassOf core:DoubleList ;
    skos:definition "TransformationMatrix4x4 is a 4 by 4 matrix represented as a list of sixteen double values in row major order."@en .

core:relationType a owl:ObjectProperty ;
    rdfs:label "relationType"@en ;
    rdfs:range core:RelationTypeValue ;
    skos:definition "Indicates the specific type of the CityObjectRelation."@en .

core:QualifiedArea a owl:Class ;
    rdfs:label "QualifiedArea"@en ;
    rdfs:subClassOf [ a owl:Restriction ;
            owl:allValuesFrom core:QualifiedAreaTypeValue ;
            owl:onProperty core:typeOfArea ],
        [ a owl:Restriction ;
            owl:onClass core:QualifiedAreaTypeValue ;
            owl:onProperty core:typeOfArea ;
            owl:qualifiedCardinality "1"^^xsd:nonNegativeInteger ],
        [ a owl:Restriction ;
            owl:allValuesFrom core:QualifiedArea ;
            owl:onProperty <https://www.opengis.net/ont/citygml/common/area> ],
        [ a owl:Restriction ;
            owl:onClass core:QualifiedArea ;
            owl:onProperty <https://www.opengis.net/ont/citygml/common/area> ;
            owl:qualifiedCardinality "1"^^xsd:nonNegativeInteger ] ;
    skos:definition "QualifiedArea is an application-dependent measure of the area of a space or of a thematic surface."@en .

core:RelationTypeValue a owl:Class ;
    rdfs:label "RelationTypeValue"@en ;
    rdfs:subClassOf skos:Concept ;
    skos:definition "RelationTypeValue is a code list used to classify city object relations."@en .

core:AbstractFeature a owl:Class ;
    rdfs:label "AbstractFeature"@en ;
    iso19150-2:isAbstract true ;
    rdfs:subClassOf [ a owl:Restriction ;
            owl:onClass core:ID ;
            owl:onProperty core:featureID ;
            owl:qualifiedCardinality "1"^^xsd:nonNegativeInteger ],
        [ a owl:Restriction ;
            owl:allValuesFrom xsd:Name ;
            owl:onProperty <https://www.opengis.net/ont/citygml/common/name> ],
        [ a owl:Restriction ;
            owl:allValuesFrom xsd:string ;
            owl:onProperty <https://www.opengis.net/ont/citygml/common/description> ],
        [ a owl:Restriction ;
            owl:maxQualifiedCardinality "1"^^xsd:nonNegativeInteger ;
            owl:onDataRange xsd:string ;
            owl:onProperty <https://www.opengis.net/ont/citygml/common/description> ],
        [ a owl:Restriction ;
            owl:allValuesFrom rdfs:Resource ;
            owl:onProperty core:identifier ],
        [ a owl:Restriction ;
            owl:allValuesFrom core:ID ;
            owl:onProperty core:featureID ],
        [ a owl:Restriction ;
            owl:maxQualifiedCardinality "1"^^xsd:nonNegativeInteger ;
            owl:onClass rdfs:Resource ;
            owl:onProperty core:identifier ],
        iso19109:AnyFeature .

core:AbstractPointCloud a owl:Class ;
    rdfs:label "AbstractPointCloud"@en ;
    iso19150-2:isAbstract true ;
    rdfs:subClassOf core:AbstractFeature .

core:ID a owl:Class ;
    rdfs:label "ID"@en ;
    skos:definition "ID is a basic type that represents a unique identifier."@en .

core:appearanceMember a owl:ObjectProperty ;
    rdfs:label "appearanceMember"@en ;
    rdfs:range core:AbstractAppearance ;
    skos:definition "Specifies the appearances of the CityModel."@en .

core:cityObjectMember a owl:ObjectProperty ;
    rdfs:label "cityObjectMember"@en ;
    rdfs:range core:AbstractCityObject ;
    skos:definition "Specifies the city objects that are part of the CityModel."@en .

core:featureMember a owl:ObjectProperty ;
    rdfs:label "featureMember"@en ;
    rdfs:range core:AbstractFeature ;
    skos:definition "Specifies the feature objects that are part of the CityModel. It allows to include objects that are not derived from a class defined in the CityGML conceptual model, but from the ISO 19109 class AnyFeature."@en .

core:list a owl:DatatypeProperty ;
    rdfs:label "list"@en ;
    rdfs:range xsd:double ;
    skos:definition "Specifies the list of double values."@en .

core:versionMember a owl:ObjectProperty ;
    rdfs:label "versionMember"@en ;
    rdfs:range core:AbstractVersion ;
    skos:definition "Specifies the different versions of the CityModel."@en .

core:versionTransitionMember a owl:ObjectProperty ;
    rdfs:label "versionTransitionMember"@en ;
    rdfs:range core:AbstractVersionTransition ;
    skos:definition "Specifies the transitions between the different versions of the CityModel."@en .

core:AbstractAppearance a owl:Class ;
    rdfs:label "AbstractAppearance"@en ;
    iso19150-2:isAbstract true ;
    rdfs:subClassOf core:AbstractFeatureWithLifespan .

core:AbstractFeatureWithLifespan a owl:Class ;
    rdfs:label "AbstractFeatureWithLifespan"@en ;
    iso19150-2:isAbstract true ;
    rdfs:subClassOf core:AbstractFeature .

core:AbstractPhysicalSpace a owl:Class ;
    rdfs:label "AbstractPhysicalSpace"@en ;
    iso19150-2:isAbstract true ;
    rdfs:subClassOf [ a owl:Restriction ;
            owl:maxQualifiedCardinality "1"^^xsd:nonNegativeInteger ;
            owl:onClass core:AbstractPointCloud ;
            owl:onProperty <https://www.opengis.net/ont/citygml/common/pointCloud> ],
        [ a owl:Restriction ;
            owl:maxQualifiedCardinality "1"^^xsd:nonNegativeInteger ;
            owl:onClass gmlowl:MultiCurve ;
            owl:onProperty core:lod3TerrainIntersectionCurve ],
        [ a owl:Restriction ;
            owl:maxQualifiedCardinality "1"^^xsd:nonNegativeInteger ;
            owl:onClass gmlowl:MultiCurve ;
            owl:onProperty core:lod1TerrainIntersectionCurve ],
        [ a owl:Restriction ;
            owl:maxQualifiedCardinality "1"^^xsd:nonNegativeInteger ;
            owl:onClass gmlowl:MultiCurve ;
            owl:onProperty core:lod2TerrainIntersectionCurve ],
        [ a owl:Restriction ;
            owl:allValuesFrom gmlowl:MultiCurve ;
            owl:onProperty core:lod1TerrainIntersectionCurve ],
        [ a owl:Restriction ;
            owl:allValuesFrom gmlowl:MultiCurve ;
            owl:onProperty core:lod3TerrainIntersectionCurve ],
        [ a owl:Restriction ;
            owl:allValuesFrom gmlowl:MultiCurve ;
            owl:onProperty core:lod2TerrainIntersectionCurve ],
        [ a owl:Restriction ;
            owl:allValuesFrom core:AbstractPointCloud ;
            owl:onProperty <https://www.opengis.net/ont/citygml/common/pointCloud> ],
        core:AbstractSpace .

core:AbstractThematicSurface a owl:Class ;
    rdfs:label "AbstractThematicSurface"@en ;
    iso19150-2:isAbstract true ;
    rdfs:subClassOf [ a owl:Restriction ;
            owl:maxQualifiedCardinality "1"^^xsd:nonNegativeInteger ;
            owl:onClass gmlowl:MultiCurve ;
            owl:onProperty <https://www.opengis.net/ont/citygml/common/lod0MultiCurve> ],
        [ a owl:Restriction ;
            owl:allValuesFrom gmlowl:MultiSurface ;
            owl:onProperty core:lod1MultiSurface ],
        [ a owl:Restriction ;
            owl:maxQualifiedCardinality "1"^^xsd:nonNegativeInteger ;
            owl:onClass gmlowl:MultiSurface ;
            owl:onProperty <https://www.opengis.net/ont/citygml/common/lod3MultiSurface> ],
        [ a owl:Restriction ;
            owl:maxQualifiedCardinality "1"^^xsd:nonNegativeInteger ;
            owl:onClass core:AbstractPointCloud ;
            owl:onProperty <https://www.opengis.net/ont/citygml/common/pointCloud> ],
        [ a owl:Restriction ;
            owl:maxQualifiedCardinality "1"^^xsd:nonNegativeInteger ;
            owl:onClass gmlowl:MultiSurface ;
            owl:onProperty core:lod1MultiSurface ],
        [ a owl:Restriction ;
            owl:allValuesFrom gmlowl:MultiCurve ;
            owl:onProperty <https://www.opengis.net/ont/citygml/common/lod0MultiCurve> ],
        [ a owl:Restriction ;
            owl:allValuesFrom core:QualifiedArea ;
            owl:onProperty <https://www.opengis.net/ont/citygml/common/area> ],
        [ a owl:Restriction ;
            owl:maxQualifiedCardinality "1"^^xsd:nonNegativeInteger ;
            owl:onClass gmlowl:MultiSurface ;
            owl:onProperty <https://www.opengis.net/ont/citygml/common/lod2MultiSurface> ],
        [ a owl:Restriction ;
            owl:allValuesFrom gmlowl:MultiSurface ;
            owl:onProperty <https://www.opengis.net/ont/citygml/common/lod2MultiSurface> ],
        [ a owl:Restriction ;
            owl:allValuesFrom gmlowl:MultiSurface ;
            owl:onProperty <https://www.opengis.net/ont/citygml/common/lod0MultiSurface> ],
        [ a owl:Restriction ;
            owl:maxQualifiedCardinality "1"^^xsd:nonNegativeInteger ;
            owl:onClass gmlowl:MultiSurface ;
            owl:onProperty <https://www.opengis.net/ont/citygml/common/lod0MultiSurface> ],
        [ a owl:Restriction ;
            owl:allValuesFrom core:AbstractPointCloud ;
            owl:onProperty <https://www.opengis.net/ont/citygml/common/pointCloud> ],
        [ a owl:Restriction ;
            owl:allValuesFrom gmlowl:MultiSurface ;
            owl:onProperty <https://www.opengis.net/ont/citygml/common/lod3MultiSurface> ],
        core:AbstractSpaceBoundary .

core:ImplicitGeometry a owl:Class ;
    rdfs:label "ImplicitGeometry"@en ;
    rdfs:subClassOf [ a owl:Restriction ;
            owl:onClass gmlowl:Point ;
            owl:onProperty <https://www.opengis.net/ont/citygml/common/referencePoint> ;
            owl:qualifiedCardinality "1"^^xsd:nonNegativeInteger ],
        [ a owl:Restriction ;
            owl:onClass core:TransformationMatrix4x4 ;
            owl:onProperty core:transformationMatrix ;
            owl:qualifiedCardinality "1"^^xsd:nonNegativeInteger ],
        [ a owl:Restriction ;
            owl:allValuesFrom core:ID ;
            owl:onProperty core:objectID ],
        [ a owl:Restriction ;
            owl:allValuesFrom core:AbstractAppearance ;
            owl:onProperty <https://www.opengis.net/ont/citygml/common/appearance> ],
        [ a owl:Restriction ;
            owl:maxQualifiedCardinality "1"^^xsd:nonNegativeInteger ;
            owl:onDataRange xsd:anyURI ;
            owl:onProperty core:libraryObject ],
        [ a owl:Restriction ;
            owl:allValuesFrom gmlowl:Point ;
            owl:onProperty <https://www.opengis.net/ont/citygml/common/referencePoint> ],
        [ a owl:Restriction ;
            owl:allValuesFrom core:TransformationMatrix4x4 ;
            owl:onProperty core:transformationMatrix ],
        [ a owl:Restriction ;
            owl:allValuesFrom core:MimeTypeValue ;
            owl:onProperty <https://www.opengis.net/ont/citygml/common/mimeType> ],
        [ a owl:Restriction ;
            owl:maxQualifiedCardinality "1"^^xsd:nonNegativeInteger ;
            owl:onClass core:MimeTypeValue ;
            owl:onProperty <https://www.opengis.net/ont/citygml/common/mimeType> ],
        [ a owl:Restriction ;
            owl:allValuesFrom xsd:anyURI ;
            owl:onProperty core:libraryObject ],
        [ a owl:Restriction ;
            owl:maxQualifiedCardinality "1"^^xsd:nonNegativeInteger ;
            owl:onClass gmlowl:AbstractGeometry ;
            owl:onProperty core:relativeGeometry ],
        [ a owl:Restriction ;
            owl:allValuesFrom gmlowl:AbstractGeometry ;
            owl:onProperty core:relativeGeometry ],
        [ a owl:Restriction ;
            owl:onClass core:ID ;
            owl:onProperty core:objectID ;
            owl:qualifiedCardinality "1"^^xsd:nonNegativeInteger ] ;
    skos:definition "ImplicitGeometry is a geometry representation where the shape is stored only once as a prototypical geometry. Examples are a tree or other vegetation object, a traffic light or a traffic sign. This prototypic geometry object can be re-used or referenced many times, wherever the corresponding feature occurs in the 3D city model."@en .

core:AbstractSpace a owl:Class ;
    rdfs:label "AbstractSpace"@en ;
    iso19150-2:isAbstract true ;
    rdfs:subClassOf [ a owl:Restriction ;
            owl:allValuesFrom gmlowl:Solid ;
            owl:onProperty core:lod3Solid ],
        [ a owl:Restriction ;
            owl:maxQualifiedCardinality "1"^^xsd:nonNegativeInteger ;
            owl:onClass gmlowl:MultiCurve ;
            owl:onProperty <https://www.opengis.net/ont/citygml/common/lod0MultiCurve> ],
        [ a owl:Restriction ;
            owl:allValuesFrom gmlowl:MultiSurface ;
            owl:onProperty <https://www.opengis.net/ont/citygml/common/lod2MultiSurface> ],
        [ a owl:Restriction ;
            owl:allValuesFrom gmlowl:MultiCurve ;
            owl:onProperty core:lod3MultiCurve ],
        [ a owl:Restriction ;
            owl:maxQualifiedCardinality "1"^^xsd:nonNegativeInteger ;
            owl:onClass gmlowl:Solid ;
            owl:onProperty core:lod1Solid ],
        [ a owl:Restriction ;
            owl:maxQualifiedCardinality "1"^^xsd:nonNegativeInteger ;
            owl:onClass gmlowl:Solid ;
            owl:onProperty core:lod3Solid ],
        [ a owl:Restriction ;
            owl:allValuesFrom core:SpaceType ;
            owl:onProperty core:spaceType ],
        [ a owl:Restriction ;
            owl:maxQualifiedCardinality "1"^^xsd:nonNegativeInteger ;
            owl:onClass gmlowl:MultiSurface ;
            owl:onProperty <https://www.opengis.net/ont/citygml/common/lod3MultiSurface> ],
        [ a owl:Restriction ;
            owl:allValuesFrom core:QualifiedArea ;
            owl:onProperty <https://www.opengis.net/ont/citygml/common/area> ],
        [ a owl:Restriction ;
            owl:maxQualifiedCardinality "1"^^xsd:nonNegativeInteger ;
            owl:onClass gmlowl:MultiCurve ;
            owl:onProperty core:lod3MultiCurve ],
        [ a owl:Restriction ;
            owl:allValuesFrom gmlowl:MultiSurface ;
            owl:onProperty <https://www.opengis.net/ont/citygml/common/lod0MultiSurface> ],
        [ a owl:Restriction ;
            owl:allValuesFrom core:AbstractSpaceBoundary ;
            owl:onProperty <https://www.opengis.net/ont/citygml/common/boundary> ],
        [ a owl:Restriction ;
            owl:allValuesFrom gmlowl:Point ;
            owl:onProperty core:lod0Point ],
        [ a owl:Restriction ;
            owl:allValuesFrom gmlowl:Solid ;
            owl:onProperty core:lod1Solid ],
        [ a owl:Restriction ;
            owl:maxQualifiedCardinality "1"^^xsd:nonNegativeInteger ;
            owl:onClass gmlowl:MultiSurface ;
            owl:onProperty <https://www.opengis.net/ont/citygml/common/lod2MultiSurface> ],
        [ a owl:Restriction ;
            owl:maxQualifiedCardinality "1"^^xsd:nonNegativeInteger ;
            owl:onClass gmlowl:Point ;
            owl:onProperty core:lod0Point ],
        [ a owl:Restriction ;
            owl:maxQualifiedCardinality "1"^^xsd:nonNegativeInteger ;
            owl:onClass gmlowl:MultiCurve ;
            owl:onProperty core:lod2MultiCurve ],
        [ a owl:Restriction ;
            owl:allValuesFrom gmlowl:MultiSurface ;
            owl:onProperty <https://www.opengis.net/ont/citygml/common/lod3MultiSurface> ],
        [ a owl:Restriction ;
            owl:maxQualifiedCardinality "1"^^xsd:nonNegativeInteger ;
            owl:onDataRange core:SpaceType ;
            owl:onProperty core:spaceType ],
        [ a owl:Restriction ;
            owl:allValuesFrom gmlowl:MultiCurve ;
            owl:onProperty core:lod2MultiCurve ],
        [ a owl:Restriction ;
            owl:maxQualifiedCardinality "1"^^xsd:nonNegativeInteger ;
            owl:onClass gmlowl:MultiSurface ;
            owl:onProperty <https://www.opengis.net/ont/citygml/common/lod0MultiSurface> ],
        [ a owl:Restriction ;
            owl:allValuesFrom gmlowl:MultiCurve ;
            owl:onProperty <https://www.opengis.net/ont/citygml/common/lod0MultiCurve> ],
        [ a owl:Restriction ;
            owl:maxQualifiedCardinality "1"^^xsd:nonNegativeInteger ;
            owl:onClass gmlowl:Solid ;
            owl:onProperty core:lod2Solid ],
        [ a owl:Restriction ;
            owl:allValuesFrom core:QualifiedVolume ;
            owl:onProperty core:volume ],
        [ a owl:Restriction ;
            owl:allValuesFrom gmlowl:Solid ;
            owl:onProperty core:lod2Solid ],
        core:AbstractCityObject ;
    owl:disjointWith core:AbstractSpaceBoundary .

core:AbstractCityObject a owl:Class ;
    rdfs:label "AbstractCityObject"@en ;
    iso19150-2:isAbstract true ;
    rdfs:subClassOf [ a owl:Restriction ;
            owl:allValuesFrom core:AbstractCityObject ;
            owl:onProperty core:generalizesTo ],
        [ a owl:Restriction ;
            owl:allValuesFrom core:RelativeToWater ;
            owl:onProperty core:relativeToWater ],
        [ a owl:Restriction ;
            owl:allValuesFrom core:RelativeToTerrain ;
            owl:onProperty core:relativeToTerrain ],
        [ a owl:Restriction ;
            owl:allValuesFrom core:AbstractAppearance ;
            owl:onProperty <https://www.opengis.net/ont/citygml/common/appearance> ],
        [ a owl:Restriction ;
            owl:allValuesFrom core:AbstractGenericAttribute ;
            owl:onProperty <https://www.opengis.net/ont/citygml/common/genericAttribute> ],
        [ a owl:Restriction ;
            owl:allValuesFrom core:ExternalReference ;
            owl:onProperty core:externalReference ],
        [ a owl:Restriction ;
            owl:maxQualifiedCardinality "1"^^xsd:nonNegativeInteger ;
            owl:onDataRange core:RelativeToWater ;
            owl:onProperty core:relativeToWater ],
        [ a owl:Restriction ;
            owl:allValuesFrom core:CityObjectRelation ;
            owl:onProperty <https://www.opengis.net/ont/citygml/common/relatedTo> ],
        [ a owl:Restriction ;
            owl:maxQualifiedCardinality "1"^^xsd:nonNegativeInteger ;
            owl:onDataRange core:RelativeToTerrain ;
            owl:onProperty core:relativeToTerrain ],
        [ a owl:Restriction ;
            owl:allValuesFrom core:AbstractDynamizer ;
            owl:onProperty core:dynamizer ],
        core:AbstractFeatureWithLifespan .

[] a owl:AllDisjointClasses ;
    owl:members ( core:TransformationMatrix2x2 core:TransformationMatrix3x4 core:TransformationMatrix4x4 ) .

[] a owl:AllDisjointClasses ;
    owl:members ( brid:BridgeRoom bldg:BuildingRoom gen:GenericUnoccupiedSpace tran:AbstractTransportationSpace tran:AuxiliaryTrafficSpace tran:ClearanceSpace tran:Hole tran:TrafficSpace tun:HollowSpace ) .

[] a owl:AllDisjointClasses ;
    owl:members ( core:AbstractAppearance core:AbstractCityObject core:AbstractDynamizer core:AbstractVersion core:AbstractVersionTransition core:CityModel doc:Document wksp:Scenario wksp:Space wksp:Workspace ) .

[] a owl:AllDisjointClasses ;
    owl:members ( bldg:AbstractBuildingSubdivision grp:CityObjectGroup gen:GenericLogicalSpace ) .

[] a owl:AllDisjointClasses ;
    owl:members ( con:AbstractConstructionSurface con:AbstractFillingSurface core:ClosureSurface gen:GenericThematicSurface luse:LandUse tran:AuxiliaryTrafficArea tran:HoleSurface tran:Marking tran:TrafficArea wtr:AbstractWaterBoundarySurface ) .

[] a owl:AllDisjointClasses ;
    owl:members ( gen:CodeAttribute gen:DateAttribute gen:DoubleAttribute gen:GenericAttributeSet gen:IntAttribute gen:MeasureAttribute gen:StringAttribute gen:UriAttribute ) .

[] a owl:AllDisjointClasses ;
    owl:members ( frn:CityFurniture con:AbstractConstruction con:AbstractConstructiveElement con:AbstractFillingElement con:AbstractFurniture con:AbstractInstallation gen:GenericOccupiedSpace veg:AbstractVegetationObject wtr:WaterBody ) .

[] a owl:AllDisjointClasses ;
    owl:members ( app:AbstractSurfaceData core:AbstractFeatureWithLifespan core:AbstractPointCloud core:Address dyn:AbstractTimeseries ) .

[] a owl:AllDisjointClasses ;
    owl:members ( core:AbstractThematicSurface dem:AbstractReliefComponent dem:ReliefFeature ) .

@prefix core: <https://www.opengis.net/ont/citygml/core/> .
@prefix doc: <https://www.opengis.net/ont/citygml/document/> .
@prefix owl: <http://www.w3.org/2002/07/owl#> .
@prefix rdfs: <http://www.w3.org/2000/01/rdf-schema#> .
@prefix schema: <https://schema.org/> .
@prefix skos: <http://www.w3.org/2004/02/skos/core#> .
@prefix time: <http://www.w3.org/2006/time#> .
@prefix xsd: <http://www.w3.org/2001/XMLSchema#> .

<https://www.opengis.net/ont/citygml/document> a owl:Ontology ;
    rdfs:label "Document"@en ;
    owl:imports <http://def.isotc211.org/iso19150/-2/2012/base>,
        <http://www.w3.org/2006/time>,
        <https://www.opengis.net/ont/citygml/common>,
        <https://www.opengis.net/ont/citygml/core> ;
    owl:versionIRI <https://www.opengis.net/ont/citygml/document/3.0.0/> ;
    owl:versionInfo "3.0.0" .

doc:count a owl:DatatypeProperty ;
    rdfs:label "count"@en ;
    rdfs:range xsd:integer .

doc:purpose a owl:DatatypeProperty ;
    rdfs:label "purpose"@en ;
    rdfs:range xsd:string .

doc:tag a owl:ObjectProperty ;
    rdfs:label "tag"@en ;
    rdfs:domain doc:Document ;
    rdfs:range doc:Tag .

doc:title a owl:DatatypeProperty ;
    rdfs:label "title"@en ;
    rdfs:range xsd:string .

doc:uri a owl:DatatypeProperty ;
    rdfs:label "uri"@en ;
    rdfs:range xsd:anyURI .

doc:Document a owl:Class ;
    rdfs:label "Document"@en ;
    rdfs:subClassOf [ a owl:Restriction ;
            owl:allValuesFrom doc:Tag ;
            owl:onProperty doc:tag ],
        [ a owl:Restriction ;
            owl:allValuesFrom doc:Reference ;
            owl:onProperty <https://www.opengis.net/ont/citygml/common/referringTo> ],
        [ a owl:Restriction ;
            owl:allValuesFrom xsd:anyURI ;
            owl:onProperty doc:uri ],
        [ a owl:Restriction ;
            owl:allValuesFrom xsd:string ;
            owl:onProperty doc:title ],
        core:AbstractFeatureWithLifespan .

doc:Tag a owl:Class ;
    rdfs:label "Tag"@en ;
    rdfs:subClassOf [ a owl:Restriction ;
            owl:allValuesFrom xsd:integer ;
            owl:onProperty doc:count ],
        [ a owl:Restriction ;
            owl:allValuesFrom xsd:string ;
            owl:onProperty doc:text ],
        [ a owl:Restriction ;
            owl:onDataRange xsd:string ;
            owl:onProperty doc:text ;
            owl:qualifiedCardinality "1"^^xsd:nonNegativeInteger ] .

doc:coveragePeriod a owl:ObjectProperty ;
    rdfs:label "coveragePeriod"@en ;
    rdfs:range time:Interval .

doc:purposeType a owl:ObjectProperty ;
    rdfs:label "purposeType"@en ;
    rdfs:range doc:PurposeTypeValue .

doc:referenceText a owl:DatatypeProperty ;
    rdfs:label "referenceText"@en ;
    rdfs:range xsd:string .

doc:referringDate a owl:DatatypeProperty ;
    rdfs:label "referringDate"@en ;
    rdfs:range xsd:dateTime .

doc:text a owl:DatatypeProperty ;
    rdfs:label "text"@en ;
    rdfs:range xsd:string .

<https://www.opengis.net/ont/citygml/common/referringTo> schema:domainIncludes doc:Document,
        doc:Reference ;
    schema:rangeIncludes core:AbstractFeatureWithLifespan,
        doc:Reference .

doc:PurposeTypeValue a owl:Class ;
    rdfs:label "PurposeTypeValue"@en ;
    rdfs:subClassOf skos:Concept .

doc:Reference a owl:Class ;
    rdfs:label "Reference"@en ;
    rdfs:subClassOf [ a owl:Restriction ;
            owl:onDataRange xsd:string ;
            owl:onProperty doc:referenceText ;
            owl:qualifiedCardinality "1"^^xsd:nonNegativeInteger ],
        [ a owl:Restriction ;
            owl:allValuesFrom doc:PurposeTypeValue ;
            owl:onProperty doc:purposeType ],
        [ a owl:Restriction ;
            owl:allValuesFrom xsd:string ;
            owl:onProperty doc:referenceText ],
        [ a owl:Restriction ;
            owl:allValuesFrom xsd:dateTime ;
            owl:onProperty doc:referringDate ],
        [ a owl:Restriction ;
            owl:minQualifiedCardinality "1"^^xsd:nonNegativeInteger ;
            owl:onClass doc:PurposeTypeValue ;
            owl:onProperty doc:purposeType ],
        [ a owl:Restriction ;
            owl:allValuesFrom core:AbstractFeatureWithLifespan ;
            owl:onProperty <https://www.opengis.net/ont/citygml/common/referringTo> ],
        [ a owl:Restriction ;
            owl:onDataRange xsd:dateTime ;
            owl:onProperty doc:referringDate ;
            owl:qualifiedCardinality "1"^^xsd:nonNegativeInteger ],
        [ a owl:Restriction ;
            owl:onClass core:AbstractFeatureWithLifespan ;
            owl:onProperty <https://www.opengis.net/ont/citygml/common/referringTo> ;
            owl:qualifiedCardinality "1"^^xsd:nonNegativeInteger ],
        [ a owl:Restriction ;
            owl:allValuesFrom time:Interval ;
            owl:onProperty doc:coveragePeriod ],
        [ a owl:Restriction ;
            owl:onClass time:Interval ;
            owl:onProperty doc:coveragePeriod ;
            owl:qualifiedCardinality "1"^^xsd:nonNegativeInteger ],
        [ a owl:Restriction ;
            owl:allValuesFrom xsd:string ;
            owl:onProperty doc:purpose ] .

@prefix core: <https://www.opengis.net/ont/citygml/core/> .
@prefix dyn: <https://www.opengis.net/ont/citygml/dynamizer/> .
@prefix gmlowl: <http://www.opengis.net/ont/gml#> .
@prefix iso19150-2: <http://def.isotc211.org/iso19150/-2/2012/base#> .
@prefix owl: <http://www.w3.org/2002/07/owl#> .
@prefix rdf: <http://www.w3.org/1999/02/22-rdf-syntax-ns#> .
@prefix rdfs: <http://www.w3.org/2000/01/rdf-schema#> .
@prefix schema: <https://schema.org/> .
@prefix skos: <http://www.w3.org/2004/02/skos/core#> .
@prefix time: <http://www.w3.org/2006/time#> .
@prefix xsd: <http://www.w3.org/2001/XMLSchema#> .

<https://www.opengis.net/ont/citygml/dynamizer> a owl:Ontology ;
    rdfs:label "Dynamizer"@en ;
    owl:imports <http://def.isotc211.org/iso19150/-2/2012/base>,
        <http://www.opengis.net/ont/gml>,
        <http://www.w3.org/2006/time>,
        <https://www.opengis.net/ont/citygml/common>,
        <https://www.opengis.net/ont/citygml/core> ;
    owl:versionIRI <https://www.opengis.net/ont/citygml/dynamizer/3.0.0/> ;
    owl:versionInfo "3.0.0" ;
    skos:definition "The Dynamizer module supports the injection of timeseries data for individual attributes of CityGML features. Timeseries data can either be retrieved from external Sensor APIs (e.g. OGC SensorThings API, OGC Sensor Observation Services, MQTT, proprietary platforms), external standardized timeseries files (e.g. OGC TimeseriesML or OGC Observations & Measurements), external tabulated files (e.g CSV) or can be represented inline as basic time-value pairs."@en .

dyn:TabulatedFileTypeValue a owl:Class ;
    rdfs:label "TabulatedFileTypeValue"@en ;
    rdfs:subClassOf skos:Concept ;
    skos:definition "TabulatedFileTypeValue is a code list used to specify the data format of the referenced external tabulated data file."@en .

dyn:StandardFileTimeseries a owl:Class ;
    rdfs:label "StandardFileTimeseries"@en ;
    rdfs:subClassOf [ a owl:Restriction ;
            owl:allValuesFrom core:MimeTypeValue ;
            owl:onProperty <https://www.opengis.net/ont/citygml/common/mimeType> ],
        [ a owl:Restriction ;
            owl:onClass dyn:StandardFileTypeValue ;
            owl:onProperty dyn:fileType ;
            owl:qualifiedCardinality "1"^^xsd:nonNegativeInteger ],
        [ a owl:Restriction ;
            owl:maxQualifiedCardinality "1"^^xsd:nonNegativeInteger ;
            owl:onClass core:MimeTypeValue ;
            owl:onProperty <https://www.opengis.net/ont/citygml/common/mimeType> ],
        [ a owl:Restriction ;
            owl:onDataRange xsd:anyURI ;
            owl:onProperty dyn:fileLocation ;
            owl:qualifiedCardinality "1"^^xsd:nonNegativeInteger ],
        [ a owl:Restriction ;
            owl:allValuesFrom dyn:StandardFileTypeValue ;
            owl:onProperty dyn:fileType ],
        [ a owl:Restriction ;
            owl:allValuesFrom xsd:anyURI ;
            owl:onProperty dyn:fileLocation ],
        dyn:AbstractAtomicTimeseries .

dyn:TabulatedFileTimeseries a owl:Class ;
    rdfs:label "TabulatedFileTimeseries"@en ;
    rdfs:subClassOf [ a owl:Restriction ;
            owl:allValuesFrom dyn:TimeseriesTypeValue ;
            owl:onProperty dyn:valueType ],
        [ a owl:Restriction ;
            owl:allValuesFrom xsd:integer ;
            owl:onProperty dyn:valueColumnNo ],
        [ a owl:Restriction ;
            owl:allValuesFrom xsd:string ;
            owl:onProperty dyn:fieldSeparator ],
        [ a owl:Restriction ;
            owl:maxQualifiedCardinality "1"^^xsd:nonNegativeInteger ;
            owl:onDataRange xsd:integer ;
            owl:onProperty dyn:idColumnNo ],
        [ a owl:Restriction ;
            owl:onDataRange dyn:TimeseriesTypeValue ;
            owl:onProperty dyn:valueType ;
            owl:qualifiedCardinality "1"^^xsd:nonNegativeInteger ],
        [ a owl:Restriction ;
            owl:allValuesFrom xsd:integer ;
            owl:onProperty dyn:timeColumnNo ],
        [ a owl:Restriction ;
            owl:allValuesFrom xsd:integer ;
            owl:onProperty dyn:idColumnNo ],
        [ a owl:Restriction ;
            owl:allValuesFrom xsd:string ;
            owl:onProperty dyn:idColumnName ],
        [ a owl:Restriction ;
            owl:allValuesFrom xsd:integer ;
            owl:onProperty dyn:numberOfHeaderLines ],
        [ a owl:Restriction ;
            owl:allValuesFrom dyn:StandardFileTypeValue ;
            owl:onProperty dyn:fileType ],
        [ a owl:Restriction ;
            owl:maxQualifiedCardinality "1"^^xsd:nonNegativeInteger ;
            owl:onDataRange xsd:integer ;
            owl:onProperty dyn:valueColumnNo ],
        [ a owl:Restriction ;
            owl:maxQualifiedCardinality "1"^^xsd:nonNegativeInteger ;
            owl:onDataRange xsd:string ;
            owl:onProperty dyn:idColumnName ],
        [ a owl:Restriction ;
            owl:onDataRange xsd:anyURI ;
            owl:onProperty dyn:fileLocation ;
            owl:qualifiedCardinality "1"^^xsd:nonNegativeInteger ],
        [ a owl:Restriction ;
            owl:allValuesFrom xsd:string ;
            owl:onProperty dyn:timeColumnName ],
        [ a owl:Restriction ;
            owl:allValuesFrom xsd:string ;
            owl:onProperty dyn:decimalSymbol ],
        [ a owl:Restriction ;
            owl:maxQualifiedCardinality "1"^^xsd:nonNegativeInteger ;
            owl:onDataRange xsd:string ;
            owl:onProperty dyn:valueColumnName ],
        [ a owl:Restriction ;
            owl:allValuesFrom xsd:anyURI ;
            owl:onProperty dyn:fileLocation ],
        [ a owl:Restriction ;
            owl:allValuesFrom xsd:string ;
            owl:onProperty dyn:idValue ],
        [ a owl:Restriction ;
            owl:maxQualifiedCardinality "1"^^xsd:nonNegativeInteger ;
            owl:onDataRange xsd:string ;
            owl:onProperty dyn:decimalSymbol ],
        [ a owl:Restriction ;
            owl:maxQualifiedCardinality "1"^^xsd:nonNegativeInteger ;
            owl:onDataRange xsd:integer ;
            owl:onProperty dyn:numberOfHeaderLines ],
        [ a owl:Restriction ;
            owl:maxQualifiedCardinality "1"^^xsd:nonNegativeInteger ;
            owl:onDataRange xsd:string ;
            owl:onProperty dyn:idValue ],
        [ a owl:Restriction ;
            owl:maxQualifiedCardinality "1"^^xsd:nonNegativeInteger ;
            owl:onDataRange xsd:integer ;
            owl:onProperty dyn:timeColumnNo ],
        [ a owl:Restriction ;
            owl:allValuesFrom core:MimeTypeValue ;
            owl:onProperty <https://www.opengis.net/ont/citygml/common/mimeType> ],
        [ a owl:Restriction ;
            owl:onDataRange xsd:string ;
            owl:onProperty dyn:fieldSeparator ;
            owl:qualifiedCardinality "1"^^xsd:nonNegativeInteger ],
        [ a owl:Restriction ;
            owl:maxQualifiedCardinality "1"^^xsd:nonNegativeInteger ;
            owl:onDataRange xsd:string ;
            owl:onProperty dyn:timeColumnName ],
        [ a owl:Restriction ;
            owl:maxQualifiedCardinality "1"^^xsd:nonNegativeInteger ;
            owl:onClass core:MimeTypeValue ;
            owl:onProperty <https://www.opengis.net/ont/citygml/common/mimeType> ],
        [ a owl:Restriction ;
            owl:onClass dyn:StandardFileTypeValue ;
            owl:onProperty dyn:fileType ;
            owl:qualifiedCardinality "1"^^xsd:nonNegativeInteger ],
        [ a owl:Restriction ;
            owl:allValuesFrom xsd:string ;
            owl:onProperty dyn:valueColumnName ],
        dyn:AbstractAtomicTimeseries .

dyn:CompositeTimeseries a owl:Class ;
    rdfs:label "CompositeTimeseries"@en ;
    rdfs:subClassOf [ a owl:Restriction ;
            owl:allValuesFrom dyn:TimeseriesComponent ;
            owl:onProperty dyn:component ],
        [ a owl:Restriction ;
            owl:minQualifiedCardinality "1"^^xsd:nonNegativeInteger ;
            owl:onClass dyn:TimeseriesComponent ;
            owl:onProperty dyn:component ],
        dyn:AbstractTimeseries .

dyn:Dynamizer a owl:Class ;
    rdfs:label "Dynamizer"@en ;
    rdfs:subClassOf [ a owl:Restriction ;
            owl:allValuesFrom dyn:SensorConnection ;
            owl:onProperty dyn:sensorConnection ],
        [ a owl:Restriction ;
            owl:maxQualifiedCardinality "1"^^xsd:nonNegativeInteger ;
            owl:onClass time:TemporalPosition ;
            owl:onProperty dyn:startTime ],
        [ a owl:Restriction ;
            owl:maxQualifiedCardinality "1"^^xsd:nonNegativeInteger ;
            owl:onClass time:TemporalPosition ;
            owl:onProperty dyn:endTime ],
        [ a owl:Restriction ;
            owl:allValuesFrom time:TemporalPosition ;
            owl:onProperty dyn:endTime ],
        [ a owl:Restriction ;
            owl:maxQualifiedCardinality "1"^^xsd:nonNegativeInteger ;
            owl:onClass dyn:SensorConnection ;
            owl:onProperty dyn:sensorConnection ],
        [ a owl:Restriction ;
            owl:allValuesFrom xsd:string ;
            owl:onProperty dyn:attributeRef ],
        [ a owl:Restriction ;
            owl:onDataRange xsd:string ;
            owl:onProperty dyn:attributeRef ;
            owl:qualifiedCardinality "1"^^xsd:nonNegativeInteger ],
        [ a owl:Restriction ;
            owl:maxQualifiedCardinality "1"^^xsd:nonNegativeInteger ;
            owl:onClass dyn:AbstractTimeseries ;
            owl:onProperty dyn:dynamicData ],
        [ a owl:Restriction ;
            owl:allValuesFrom dyn:AbstractTimeseries ;
            owl:onProperty dyn:dynamicData ],
        [ a owl:Restriction ;
            owl:allValuesFrom time:TemporalPosition ;
            owl:onProperty dyn:startTime ],
        core:AbstractDynamizer .

dyn:GenericTimeseries a owl:Class ;
    rdfs:label "GenericTimeseries"@en ;
    rdfs:subClassOf [ a owl:Restriction ;
            owl:allValuesFrom dyn:TimeValuePair ;
            owl:onProperty dyn:timeValuePair ],
        [ a owl:Restriction ;
            owl:minQualifiedCardinality "1"^^xsd:nonNegativeInteger ;
            owl:onClass dyn:TimeValuePair ;
            owl:onProperty dyn:timeValuePair ],
        [ a owl:Restriction ;
            owl:allValuesFrom dyn:TimeseriesTypeValue ;
            owl:onProperty dyn:valueType ],
        [ a owl:Restriction ;
            owl:onDataRange dyn:TimeseriesTypeValue ;
            owl:onProperty dyn:valueType ;
            owl:qualifiedCardinality "1"^^xsd:nonNegativeInteger ],
        dyn:AbstractAtomicTimeseries .

dyn:additionalGap a owl:ObjectProperty ;
    rdfs:label "additionalGap"@en ;
    rdfs:range time:TemporalDuration ;
    skos:definition "Specifies how much extra time is added after all repetitions as an additional gap."@en .

dyn:appearanceValue a owl:ObjectProperty ;
    rdfs:label "appearanceValue"@en ;
    rdfs:range core:AbstractAppearance ;
    skos:definition "Specifies the \"Appearance\" value of the TimeValuePair."@en .

dyn:attributeRef a owl:DatatypeProperty ;
    rdfs:label "attributeRef"@en ;
    rdfs:range xsd:string ;
    skos:definition "Specifies the attribute of a CityGML feature whose value is overridden or replaced by the (dynamic) values specified by the Dynamizer."@en .

dyn:authType a owl:ObjectProperty ;
    rdfs:label "authType"@en ;
    rdfs:range dyn:AuthenticationTypeValue ;
    skos:definition "Specifies the type of authentication required to be able to access the Sensor API."@en .

dyn:baseURL a owl:DatatypeProperty ;
    rdfs:label "baseURL"@en ;
    rdfs:range xsd:anyURI ;
    skos:definition "Specifies the base URL of the Sensor API request."@en .

dyn:boolValue a owl:DatatypeProperty ;
    rdfs:label "boolValue"@en ;
    rdfs:range xsd:boolean ;
    skos:definition "Specifies the \"Boolean\" value of the TimeValuePair."@en .

dyn:component a owl:ObjectProperty ;
    rdfs:label "component"@en ;
    rdfs:domain dyn:CompositeTimeseries ;
    rdfs:range dyn:TimeseriesComponent ;
    skos:definition "Relates to the atomic and composite timeseries that are part of the CompositeTimeseries. The referenced timeseries are sequentially ordered."@en .

dyn:connectionType a owl:ObjectProperty ;
    rdfs:label "connectionType"@en ;
    rdfs:range dyn:SensorConnectionTypeValue ;
    skos:definition "Indicates the type of Sensor API to which the SensorConnection refers."@en .

dyn:datastreamID a owl:DatatypeProperty ;
    rdfs:label "datastreamID"@en ;
    rdfs:range xsd:string ;
    skos:definition "Specifies the datastream that is retrieved by the SensorConnection."@en .

dyn:decimalSymbol a owl:DatatypeProperty ;
    rdfs:label "decimalSymbol"@en ;
    rdfs:range xsd:string ;
    skos:definition "Indicates which symbol is used to separate the integer part from the fractional part of a decimal number."@en .

dyn:doubleValue a owl:DatatypeProperty ;
    rdfs:label "doubleValue"@en ;
    rdfs:range xsd:double ;
    skos:definition "Specifies the \"Double\" value of the TimeValuePair."@en .

dyn:dynamicData a owl:ObjectProperty ;
    rdfs:label "dynamicData"@en ;
    rdfs:domain dyn:Dynamizer ;
    rdfs:range dyn:AbstractTimeseries ;
    skos:definition "Relates to the timeseries data that is given either inline within a CityGML dataset or by a link to an external file containing timeseries data."@en .

dyn:endTime a owl:ObjectProperty ;
    rdfs:label "endTime"@en ;
    rdfs:range time:TemporalPosition ;
    skos:definition "Specifies the end of the time span for which the Dynamizer provides dynamic values."@en .

dyn:fieldSeparator a owl:DatatypeProperty ;
    rdfs:label "fieldSeparator"@en ;
    rdfs:range xsd:string ;
    skos:definition "Indicates which symbol is used to separate the individual values in the tabulated file."@en .

dyn:firstTimestamp a owl:ObjectProperty ;
    rdfs:label "firstTimestamp"@en ;
    rdfs:range time:TemporalPosition ;
    skos:definition "Specifies the beginning of the timeseries."@en .

dyn:geometryValue a owl:ObjectProperty ;
    rdfs:label "geometryValue"@en ;
    rdfs:range gmlowl:AbstractGeometry ;
    skos:definition "Specifies the geometry value of the TimeValuePair."@en .

dyn:idColumnName a owl:DatatypeProperty ;
    rdfs:label "idColumnName"@en ;
    rdfs:range xsd:string ;
    skos:definition "Specifies the name of the column that stores the identifier of the time-value-pair."@en .

dyn:idColumnNo a owl:DatatypeProperty ;
    rdfs:label "idColumnNo"@en ;
    rdfs:range xsd:integer ;
    skos:definition "Specifies the number of the column that stores the identifier of the time-value-pair."@en .

dyn:idValue a owl:DatatypeProperty ;
    rdfs:label "idValue"@en ;
    rdfs:range xsd:string ;
    skos:definition "Specifies the value of the identifier for which the time-value-pairs are to be selected."@en .

dyn:implicitGeometryValue a owl:ObjectProperty ;
    rdfs:label "implicitGeometryValue"@en ;
    rdfs:range core:ImplicitGeometry ;
    skos:definition "Specifies the \"ImplicitGeometry\" value of the TimeValuePair."@en .

dyn:intValue a owl:DatatypeProperty ;
    rdfs:label "intValue"@en ;
    rdfs:range xsd:integer ;
    skos:definition "Specifies the \"Integer\" value of the TimeValuePair."@en .

dyn:lastTimestamp a owl:ObjectProperty ;
    rdfs:label "lastTimestamp"@en ;
    rdfs:range time:TemporalPosition ;
    skos:definition "Specifies the end of the timeseries."@en .

dyn:linkToObservation a owl:DatatypeProperty ;
    rdfs:label "linkToObservation"@en ;
    rdfs:range xsd:string ;
    skos:definition "Specifies the complete URL to the observation request."@en .

dyn:linkToSensorDescription a owl:DatatypeProperty ;
    rdfs:label "linkToSensorDescription"@en ;
    rdfs:range xsd:string ;
    skos:definition "Specifies the complete URL to the sensor description request."@en .

dyn:mqttServer a owl:DatatypeProperty ;
    rdfs:label "mqttServer"@en ;
    rdfs:range xsd:string ;
    skos:definition "Specifies the name of the MQTT Server. This attribute is relevant when the MQTT Protocol is used to connect to a Sensor API."@en .

dyn:mqttTopic a owl:DatatypeProperty ;
    rdfs:label "mqttTopic"@en ;
    rdfs:range xsd:string ;
    skos:definition "Names the specific datastream that is retrieved by the SensorConnection. This attribute is relevant when the MQTT Protocol is used to connect to a Sensor API."@en .

dyn:numberOfHeaderLines a owl:DatatypeProperty ;
    rdfs:label "numberOfHeaderLines"@en ;
    rdfs:range xsd:integer ;
    skos:definition "Indicates the number of lines at the beginning of the tabulated file that represent headers."@en .

dyn:observationID a owl:DatatypeProperty ;
    rdfs:label "observationID"@en ;
    rdfs:range xsd:string ;
    skos:definition "Specifies the unique identifier of the observation that is retrieved by the SensorConnection."@en .

dyn:repetitions a owl:DatatypeProperty ;
    rdfs:label "repetitions"@en ;
    rdfs:range xsd:integer ;
    skos:definition "Specifies how often the timeseries that is referenced by the TimeseriesComponent should be iterated."@en .

dyn:sensorConnection a owl:ObjectProperty ;
    rdfs:label "sensorConnection"@en ;
    rdfs:domain dyn:Dynamizer ;
    rdfs:range dyn:SensorConnection ;
    skos:definition "Relates to the sensor API that delivers timeseries data."@en .

dyn:sensorID a owl:DatatypeProperty ;
    rdfs:label "sensorID"@en ;
    rdfs:range xsd:string ;
    skos:definition "Specifies the unique identifier of the sensor from which the SensorConnection retrieves observations."@en .

dyn:sensorLocation a owl:ObjectProperty ;
    rdfs:label "sensorLocation"@en ;
    rdfs:domain dyn:SensorConnection ;
    rdfs:range core:AbstractCityObject ;
    skos:definition "Relates the sensor to the city object where it is located."@en .

dyn:sensorName a owl:DatatypeProperty ;
    rdfs:label "sensorName"@en ;
    rdfs:range xsd:string ;
    skos:definition "Specifies the name of the sensor from which the SensorConnection retrieves observations."@en .

dyn:startTime a owl:ObjectProperty ;
    rdfs:label "startTime"@en ;
    rdfs:range time:TemporalPosition ;
    skos:definition "Specifies the beginning of the time span for which the Dynamizer provides dynamic values."@en .

dyn:stringValue a owl:DatatypeProperty ;
    rdfs:label "stringValue"@en ;
    rdfs:range xsd:string ;
    skos:definition "Specifies the \"String\" value of the TimeValuePair."@en .

dyn:timeColumnName a owl:DatatypeProperty ;
    rdfs:label "timeColumnName"@en ;
    rdfs:range xsd:string ;
    skos:definition "Specifies the name of the column that stores the timestamp of the time-value-pair."@en .

dyn:timeColumnNo a owl:DatatypeProperty ;
    rdfs:label "timeColumnNo"@en ;
    rdfs:range xsd:integer ;
    skos:definition "Specifies the number of the column that stores the timestamp of the time-value-pair."@en .

dyn:timeValuePair a owl:ObjectProperty ;
    rdfs:label "timeValuePair"@en ;
    rdfs:domain dyn:GenericTimeseries ;
    rdfs:range dyn:TimeValuePair ;
    skos:definition "Relates to the time-value-pairs that are part of the GenericTimeseries."@en .

dyn:timeseries a owl:ObjectProperty ;
    rdfs:label "timeseries"@en ;
    rdfs:domain dyn:TimeseriesComponent ;
    rdfs:range dyn:AbstractTimeseries ;
    skos:definition "Relates a timeseries to the TimeseriesComponent."@en .

dyn:timestamp a owl:ObjectProperty ;
    rdfs:label "timestamp"@en ;
    rdfs:range time:TemporalPosition ;
    skos:definition "Specifies the timepoint at which the value of the TimeValuePair is valid."@en .

dyn:uriValue a owl:DatatypeProperty ;
    rdfs:label "uriValue"@en ;
    rdfs:range xsd:anyURI ;
    skos:definition "Specifies the \"URI\" value of the TimeValuePair."@en .

dyn:valueColumnName a owl:DatatypeProperty ;
    rdfs:label "valueColumnName"@en ;
    rdfs:range xsd:string ;
    skos:definition "Specifies the name of the column that stores the value of the time-value-pair."@en .

dyn:valueColumnNo a owl:DatatypeProperty ;
    rdfs:label "valueColumnNo"@en ;
    rdfs:range xsd:integer ;
    skos:definition "Specifies the number of the column that stores the value of the time-value-pair."@en .

dyn:AbstractAtomicTimeseries a owl:Class ;
    rdfs:label "AbstractAtomicTimeseries"@en ;
    iso19150-2:isAbstract true ;
    rdfs:subClassOf [ a owl:Restriction ;
            owl:allValuesFrom xsd:string ;
            owl:onProperty dyn:observationProperty ],
        [ a owl:Restriction ;
            owl:maxQualifiedCardinality "1"^^xsd:nonNegativeInteger ;
            owl:onDataRange xsd:string ;
            owl:onProperty dyn:uom ],
        [ a owl:Restriction ;
            owl:onDataRange xsd:string ;
            owl:onProperty dyn:observationProperty ;
            owl:qualifiedCardinality "1"^^xsd:nonNegativeInteger ],
        [ a owl:Restriction ;
            owl:allValuesFrom xsd:string ;
            owl:onProperty dyn:uom ],
        dyn:AbstractTimeseries ;
    owl:disjointWith dyn:CompositeTimeseries .

dyn:AuthenticationTypeValue a owl:Class ;
    rdfs:label "AuthenticationTypeValue"@en ;
    rdfs:subClassOf skos:Concept ;
    skos:definition "AuthenticationTypeValue is a code list used to specify the authentication method to be used to access the referenced sensor service. Each value provides enough information such that a software application could determine the required access credentials."@en .

dyn:SensorConnectionTypeValue a owl:Class ;
    rdfs:label "SensorConnectionTypeValue"@en ;
    rdfs:subClassOf skos:Concept ;
    skos:definition "SensorConnectionTypeValue is a code list used to specify the type of the referenced sensor service. Each value provides enough information such that a software application would be able to identify the API type and version."@en .

dyn:TimeValuePair a owl:Class ;
    rdfs:label "TimeValuePair"@en ;
    rdfs:subClassOf [ a owl:Restriction ;
            owl:allValuesFrom gmlowl:AbstractGeometry ;
            owl:onProperty dyn:geometryValue ],
        [ a owl:Restriction ;
            owl:allValuesFrom xsd:string ;
            owl:onProperty dyn:stringValue ],
        [ a owl:Restriction ;
            owl:maxQualifiedCardinality "1"^^xsd:nonNegativeInteger ;
            owl:onClass core:AbstractAppearance ;
            owl:onProperty dyn:appearanceValue ],
        [ a owl:Restriction ;
            owl:allValuesFrom xsd:anyURI ;
            owl:onProperty dyn:uriValue ],
        [ a owl:Restriction ;
            owl:allValuesFrom core:ImplicitGeometry ;
            owl:onProperty dyn:implicitGeometryValue ],
        [ a owl:Restriction ;
            owl:maxQualifiedCardinality "1"^^xsd:nonNegativeInteger ;
            owl:onClass core:ImplicitGeometry ;
            owl:onProperty dyn:implicitGeometryValue ],
        [ a owl:Restriction ;
            owl:maxQualifiedCardinality "1"^^xsd:nonNegativeInteger ;
            owl:onDataRange xsd:double ;
            owl:onProperty dyn:doubleValue ],
        [ a owl:Restriction ;
            owl:onClass time:TemporalPosition ;
            owl:onProperty dyn:timestamp ;
            owl:qualifiedCardinality "1"^^xsd:nonNegativeInteger ],
        [ a owl:Restriction ;
            owl:allValuesFrom xsd:integer ;
            owl:onProperty dyn:intValue ],
        [ a owl:Restriction ;
            owl:maxQualifiedCardinality "1"^^xsd:nonNegativeInteger ;
            owl:onDataRange xsd:integer ;
            owl:onProperty dyn:intValue ],
        [ a owl:Restriction ;
            owl:maxQualifiedCardinality "1"^^xsd:nonNegativeInteger ;
            owl:onDataRange xsd:boolean ;
            owl:onProperty dyn:boolValue ],
        [ a owl:Restriction ;
            owl:allValuesFrom core:AbstractAppearance ;
            owl:onProperty dyn:appearanceValue ],
        [ a owl:Restriction ;
            owl:maxQualifiedCardinality "1"^^xsd:nonNegativeInteger ;
            owl:onDataRange xsd:anyURI ;
            owl:onProperty dyn:uriValue ],
        [ a owl:Restriction ;
            owl:allValuesFrom xsd:double ;
            owl:onProperty dyn:doubleValue ],
        [ a owl:Restriction ;
            owl:maxQualifiedCardinality "1"^^xsd:nonNegativeInteger ;
            owl:onDataRange xsd:string ;
            owl:onProperty dyn:stringValue ],
        [ a owl:Restriction ;
            owl:allValuesFrom xsd:boolean ;
            owl:onProperty dyn:boolValue ],
        [ a owl:Restriction ;
            owl:allValuesFrom time:TemporalPosition ;
            owl:onProperty dyn:timestamp ],
        [ a owl:Restriction ;
            owl:maxQualifiedCardinality "1"^^xsd:nonNegativeInteger ;
            owl:onClass gmlowl:AbstractGeometry ;
            owl:onProperty dyn:geometryValue ] ;
    skos:definition "A TimeValuePair represents a value that is valid for a given timepoint. For each TimeValuePair, only one of the value properties can be used mutually exclusive. Which value property has to be provided depends on the selected value type in the GenericTimeSeries feature, in which the TimeValuePair is included."@en .

<https://www.opengis.net/ont/citygml/common/mimeType> rdfs:label "mimeType"@en ;
    skos:definition "Specifies the MIME type of the external timeseries file."@en ;
    schema:rangeIncludes core:MimeTypeValue .

dyn:SensorConnection a owl:Class ;
    rdfs:label "SensorConnection"@en ;
    rdfs:subClassOf [ a owl:Restriction ;
            owl:maxQualifiedCardinality "1"^^xsd:nonNegativeInteger ;
            owl:onDataRange xsd:string ;
            owl:onProperty dyn:sensorName ],
        [ a owl:Restriction ;
            owl:maxQualifiedCardinality "1"^^xsd:nonNegativeInteger ;
            owl:onDataRange xsd:string ;
            owl:onProperty dyn:mqttServer ],
        [ a owl:Restriction ;
            owl:maxQualifiedCardinality "1"^^xsd:nonNegativeInteger ;
            owl:onDataRange xsd:string ;
            owl:onProperty dyn:datastreamID ],
        [ a owl:Restriction ;
            owl:onClass dyn:SensorConnectionTypeValue ;
            owl:onProperty dyn:connectionType ;
            owl:qualifiedCardinality "1"^^xsd:nonNegativeInteger ],
        [ a owl:Restriction ;
            owl:maxQualifiedCardinality "1"^^xsd:nonNegativeInteger ;
            owl:onDataRange xsd:string ;
            owl:onProperty dyn:linkToSensorDescription ],
        [ a owl:Restriction ;
            owl:allValuesFrom xsd:string ;
            owl:onProperty dyn:linkToObservation ],
        [ a owl:Restriction ;
            owl:maxQualifiedCardinality "1"^^xsd:nonNegativeInteger ;
            owl:onClass core:AbstractCityObject ;
            owl:onProperty dyn:sensorLocation ],
        [ a owl:Restriction ;
            owl:allValuesFrom xsd:anyURI ;
            owl:onProperty dyn:baseURL ],
        [ a owl:Restriction ;
            owl:allValuesFrom core:AbstractCityObject ;
            owl:onProperty dyn:sensorLocation ],
        [ a owl:Restriction ;
            owl:maxQualifiedCardinality "1"^^xsd:nonNegativeInteger ;
            owl:onDataRange xsd:anyURI ;
            owl:onProperty dyn:baseURL ],
        [ a owl:Restriction ;
            owl:allValuesFrom dyn:SensorConnectionTypeValue ;
            owl:onProperty dyn:connectionType ],
        [ a owl:Restriction ;
            owl:maxQualifiedCardinality "1"^^xsd:nonNegativeInteger ;
            owl:onDataRange xsd:string ;
            owl:onProperty dyn:observationID ],
        [ a owl:Restriction ;
            owl:maxQualifiedCardinality "1"^^xsd:nonNegativeInteger ;
            owl:onDataRange xsd:string ;
            owl:onProperty dyn:mqttTopic ],
        [ a owl:Restriction ;
            owl:maxQualifiedCardinality "1"^^xsd:nonNegativeInteger ;
            owl:onDataRange xsd:string ;
            owl:onProperty dyn:uom ],
        [ a owl:Restriction ;
            owl:maxQualifiedCardinality "1"^^xsd:nonNegativeInteger ;
            owl:onClass dyn:AuthenticationTypeValue ;
            owl:onProperty dyn:authType ],
        [ a owl:Restriction ;
            owl:allValuesFrom xsd:string ;
            owl:onProperty dyn:sensorName ],
        [ a owl:Restriction ;
            owl:allValuesFrom xsd:string ;
            owl:onProperty dyn:linkToSensorDescription ],
        [ a owl:Restriction ;
            owl:allValuesFrom xsd:string ;
            owl:onProperty dyn:observationProperty ],
        [ a owl:Restriction ;
            owl:allValuesFrom xsd:string ;
            owl:onProperty dyn:uom ],
        [ a owl:Restriction ;
            owl:allValuesFrom xsd:string ;
            owl:onProperty dyn:observationID ],
        [ a owl:Restriction ;
            owl:allValuesFrom xsd:string ;
            owl:onProperty dyn:mqttTopic ],
        [ a owl:Restriction ;
            owl:maxQualifiedCardinality "1"^^xsd:nonNegativeInteger ;
            owl:onDataRange xsd:string ;
            owl:onProperty dyn:sensorID ],
        [ a owl:Restriction ;
            owl:allValuesFrom xsd:string ;
            owl:onProperty dyn:sensorID ],
        [ a owl:Restriction ;
            owl:onDataRange xsd:string ;
            owl:onProperty dyn:observationProperty ;
            owl:qualifiedCardinality "1"^^xsd:nonNegativeInteger ],
        [ a owl:Restriction ;
            owl:allValuesFrom xsd:string ;
            owl:onProperty dyn:datastreamID ],
        [ a owl:Restriction ;
            owl:allValuesFrom dyn:AuthenticationTypeValue ;
            owl:onProperty dyn:authType ],
        [ a owl:Restriction ;
            owl:maxQualifiedCardinality "1"^^xsd:nonNegativeInteger ;
            owl:onDataRange xsd:string ;
            owl:onProperty dyn:linkToObservation ],
        [ a owl:Restriction ;
            owl:allValuesFrom xsd:string ;
            owl:onProperty dyn:mqttServer ] ;
    skos:definition "A SensorConnection provides all details that are required to retrieve a specific datastream from an external sensor web service. This data type comprises the service type (e.g. OGC SensorThings API, OGC Sensor Observation Services, MQTT, proprietary platforms), the URL of the sensor service, the identifier for the sensor or thing, and its observed property as well as information about the required authentication method."@en .

dyn:TimeseriesComponent a owl:Class ;
    rdfs:label "TimeseriesComponent"@en ;
    rdfs:subClassOf [ a owl:Restriction ;
            owl:allValuesFrom dyn:AbstractTimeseries ;
            owl:onProperty dyn:timeseries ],
        [ a owl:Restriction ;
            owl:onClass dyn:AbstractTimeseries ;
            owl:onProperty dyn:timeseries ;
            owl:qualifiedCardinality "1"^^xsd:nonNegativeInteger ],
        [ a owl:Restriction ;
            owl:allValuesFrom time:TemporalDuration ;
            owl:onProperty dyn:additionalGap ],
        [ a owl:Restriction ;
            owl:maxQualifiedCardinality "1"^^xsd:nonNegativeInteger ;
            owl:onClass time:TemporalDuration ;
            owl:onProperty dyn:additionalGap ],
        [ a owl:Restriction ;
            owl:allValuesFrom xsd:integer ;
            owl:onProperty dyn:repetitions ],
        [ a owl:Restriction ;
            owl:onDataRange xsd:integer ;
            owl:onProperty dyn:repetitions ;
            owl:qualifiedCardinality "1"^^xsd:nonNegativeInteger ] ;
    skos:definition "TimeseriesComponent represents an element of a CompositeTimeseries."@en .

dyn:fileLocation a owl:DatatypeProperty ;
    rdfs:label "fileLocation"@en ;
    rdfs:range xsd:anyURI ;
    skos:definition "Specifies the URI that points to the external timeseries file."@en .

dyn:fileType a owl:ObjectProperty ;
    rdfs:label "fileType"@en ;
    rdfs:range dyn:StandardFileTypeValue ;
    skos:definition "Specifies the format used to represent the timeseries data."@en .

dyn:observationProperty a owl:DatatypeProperty ;
    rdfs:label "observationProperty"@en ;
    rdfs:range xsd:string ;
    skos:definition "Specifies the phenomenon for which the atomic timeseries provides observation values."@en .

dyn:uom a owl:DatatypeProperty ;
    rdfs:label "uom"@en ;
    rdfs:range xsd:string ;
    skos:definition "Specifies the unit of measurement of the observation values."@en .

dyn:valueType a owl:DatatypeProperty ;
    rdfs:label "valueType"@en ;
    rdfs:range dyn:TimeseriesTypeValue ;
    skos:definition "Indicates the specific type of the timeseries data."@en .

dyn:StandardFileTypeValue a owl:Class ;
    rdfs:label "StandardFileTypeValue"@en ;
    rdfs:subClassOf skos:Concept ;
    skos:definition "StandardFileTypeValue is a code list used to specify the type of the referenced external timeseries data file. Each value provides information about the standard and version."@en .

dyn:TimeseriesTypeValue a rdfs:Datatype ;
    rdfs:label "TimeseriesTypeValue"@en ;
    owl:equivalentClass [ a rdfs:Datatype ;
            owl:oneOf ( "int" "double" "string" "geometry" "uri" "bool" "implicitGeometry" "appearance" ) ] ;
    skos:definition "TimeseriesTypeValue enumerates the possible value types for GenericTimeseries and TimeValuePair."@en .

dyn:AbstractTimeseries a owl:Class ;
    rdfs:label "AbstractTimeseries"@en ;
    iso19150-2:isAbstract true ;
    rdfs:subClassOf [ a owl:Restriction ;
            owl:allValuesFrom time:TemporalPosition ;
            owl:onProperty dyn:firstTimestamp ],
        [ a owl:Restriction ;
            owl:maxQualifiedCardinality "1"^^xsd:nonNegativeInteger ;
            owl:onClass time:TemporalPosition ;
            owl:onProperty dyn:lastTimestamp ],
        [ a owl:Restriction ;
            owl:allValuesFrom time:TemporalPosition ;
            owl:onProperty dyn:lastTimestamp ],
        [ a owl:Restriction ;
            owl:maxQualifiedCardinality "1"^^xsd:nonNegativeInteger ;
            owl:onClass time:TemporalPosition ;
            owl:onProperty dyn:firstTimestamp ],
        core:AbstractFeature .

[] a owl:AllDisjointClasses ;
    owl:members ( dyn:GenericTimeseries dyn:StandardFileTimeseries dyn:TabulatedFileTimeseries ) .

@prefix core: <https://www.opengis.net/ont/citygml/core/> .
@prefix gen: <https://www.opengis.net/ont/citygml/generics/> .
@prefix owl: <http://www.w3.org/2002/07/owl#> .
@prefix rdfs: <http://www.w3.org/2000/01/rdf-schema#> .
@prefix schema: <https://schema.org/> .
@prefix skos: <http://www.w3.org/2004/02/skos/core#> .
@prefix xsd: <http://www.w3.org/2001/XMLSchema#> .

<https://www.opengis.net/ont/citygml/generics> a owl:Ontology ;
    rdfs:label "Generics"@en ;
    owl:imports <http://def.isotc211.org/iso19150/-2/2012/base>,
        <https://www.opengis.net/ont/citygml/common>,
        <https://www.opengis.net/ont/citygml/core> ;
    owl:versionIRI <https://www.opengis.net/ont/citygml/generics/3.0.0/> ;
    owl:versionInfo "3.0.0" ;
    skos:definition "The Generics module supports application-specific extensions to the CityGML conceptual model. These extensions may be used to model and exchange additional attributes and features not covered by the predefined thematic classes of CityGML. Generic extensions shall only be used if appropriate thematic classes or attributes are not provided by any other CityGML module."@en .

gen:CodeAttribute a owl:Class ;
    rdfs:label "CodeAttribute"@en ;
    rdfs:subClassOf [ a owl:Restriction ;
            owl:onDataRange xsd:double ;
            owl:onProperty <https://www.opengis.net/ont/citygml/common/value> ;
            owl:qualifiedCardinality "1"^^xsd:nonNegativeInteger ],
        [ a owl:Restriction ;
            owl:allValuesFrom xsd:string ;
            owl:onProperty <https://www.opengis.net/ont/citygml/common/name> ],
        [ a owl:Restriction ;
            owl:onDataRange xsd:string ;
            owl:onProperty <https://www.opengis.net/ont/citygml/common/name> ;
            owl:qualifiedCardinality "1"^^xsd:nonNegativeInteger ],
        [ a owl:Restriction ;
            owl:allValuesFrom xsd:double ;
            owl:onProperty <https://www.opengis.net/ont/citygml/common/value> ],
        core:AbstractGenericAttribute ;
    skos:definition "CodeAttribute is a data type used to define generic attributes of type \"Code\"."@en .

gen:DateAttribute a owl:Class ;
    rdfs:label "DateAttribute"@en ;
    rdfs:subClassOf [ a owl:Restriction ;
            owl:allValuesFrom xsd:double ;
            owl:onProperty <https://www.opengis.net/ont/citygml/common/value> ],
        [ a owl:Restriction ;
            owl:onDataRange xsd:double ;
            owl:onProperty <https://www.opengis.net/ont/citygml/common/value> ;
            owl:qualifiedCardinality "1"^^xsd:nonNegativeInteger ],
        [ a owl:Restriction ;
            owl:allValuesFrom xsd:string ;
            owl:onProperty <https://www.opengis.net/ont/citygml/common/name> ],
        [ a owl:Restriction ;
            owl:onDataRange xsd:string ;
            owl:onProperty <https://www.opengis.net/ont/citygml/common/name> ;
            owl:qualifiedCardinality "1"^^xsd:nonNegativeInteger ],
        core:AbstractGenericAttribute ;
    skos:definition "DateAttribute is a data type used to define generic attributes of type \"Date\"."@en .

gen:DoubleAttribute a owl:Class ;
    rdfs:label "DoubleAttribute"@en ;
    rdfs:subClassOf [ a owl:Restriction ;
            owl:onDataRange xsd:string ;
            owl:onProperty <https://www.opengis.net/ont/citygml/common/name> ;
            owl:qualifiedCardinality "1"^^xsd:nonNegativeInteger ],
        [ a owl:Restriction ;
            owl:allValuesFrom xsd:double ;
            owl:onProperty <https://www.opengis.net/ont/citygml/common/value> ],
        [ a owl:Restriction ;
            owl:onDataRange xsd:double ;
            owl:onProperty <https://www.opengis.net/ont/citygml/common/value> ;
            owl:qualifiedCardinality "1"^^xsd:nonNegativeInteger ],
        [ a owl:Restriction ;
            owl:allValuesFrom xsd:string ;
            owl:onProperty <https://www.opengis.net/ont/citygml/common/name> ],
        core:AbstractGenericAttribute ;
    skos:definition "DoubleAttribute is a data type used to define generic attributes of type \"Double\"."@en .

gen:GenericLogicalSpace a owl:Class ;
    rdfs:label "GenericLogicalSpace"@en ;
    rdfs:subClassOf [ a owl:Restriction ;
            owl:allValuesFrom gen:GenericUnoccupiedSpaceUsageValue ;
            owl:onProperty <https://www.opengis.net/ont/citygml/common/usage> ],
        [ a owl:Restriction ;
            owl:allValuesFrom gen:GenericUnoccupiedSpaceFunctionValue ;
            owl:onProperty <https://www.opengis.net/ont/citygml/common/function> ],
        [ a owl:Restriction ;
            owl:allValuesFrom gen:GenericUnoccupiedSpaceClassValue ;
            owl:onProperty <https://www.opengis.net/ont/citygml/common/class> ],
        [ a owl:Restriction ;
            owl:maxQualifiedCardinality "1"^^xsd:nonNegativeInteger ;
            owl:onClass gen:GenericUnoccupiedSpaceClassValue ;
            owl:onProperty <https://www.opengis.net/ont/citygml/common/class> ],
        core:AbstractLogicalSpace .

gen:GenericLogicalSpaceClassValue a owl:Class ;
    rdfs:label "GenericLogicalSpaceClassValue"@en ;
    rdfs:subClassOf skos:Concept ;
    skos:definition "GenericLogicalSpaceClassValue is a code list used to further classify a GenericLogicalSpace."@en .

gen:GenericLogicalSpaceFunctionValue a owl:Class ;
    rdfs:label "GenericLogicalSpaceFunctionValue"@en ;
    rdfs:subClassOf skos:Concept ;
    skos:definition "GenericLogicalSpaceFunctionValue is a code list that enumerates the different purposes of a GenericLogicalSpace."@en .

gen:GenericLogicalSpaceUsageValue a owl:Class ;
    rdfs:label "GenericLogicalSpaceUsageValue"@en ;
    rdfs:subClassOf skos:Concept ;
    skos:definition "GenericLogicalSpaceUsageValue is a code list that enumerates the different uses of a GenericLogicalSpace."@en .

gen:GenericOccupiedSpace a owl:Class ;
    rdfs:label "GenericOccupiedSpace"@en ;
    rdfs:subClassOf [ a owl:Restriction ;
            owl:allValuesFrom gen:GenericUnoccupiedSpaceUsageValue ;
            owl:onProperty <https://www.opengis.net/ont/citygml/common/usage> ],
        [ a owl:Restriction ;
            owl:allValuesFrom gen:GenericUnoccupiedSpaceFunctionValue ;
            owl:onProperty <https://www.opengis.net/ont/citygml/common/function> ],
        [ a owl:Restriction ;
            owl:allValuesFrom gen:GenericUnoccupiedSpaceClassValue ;
            owl:onProperty <https://www.opengis.net/ont/citygml/common/class> ],
        [ a owl:Restriction ;
            owl:maxQualifiedCardinality "1"^^xsd:nonNegativeInteger ;
            owl:onClass gen:GenericUnoccupiedSpaceClassValue ;
            owl:onProperty <https://www.opengis.net/ont/citygml/common/class> ],
        core:AbstractOccupiedSpace .

gen:GenericOccupiedSpaceClassValue a owl:Class ;
    rdfs:label "GenericOccupiedSpaceClassValue"@en ;
    rdfs:subClassOf skos:Concept ;
    skos:definition "GenericOccupiedSpaceClassValue is a code list used to further classify a GenericOccupiedSpace."@en .

gen:GenericOccupiedSpaceFunctionValue a owl:Class ;
    rdfs:label "GenericOccupiedSpaceFunctionValue"@en ;
    rdfs:subClassOf skos:Concept ;
    skos:definition "GenericOccupiedSpaceFunctionValue is a code list that enumerates the different purposes of a GenericOccupiedSpace."@en .

gen:GenericOccupiedSpaceUsageValue a owl:Class ;
    rdfs:label "GenericOccupiedSpaceUsageValue"@en ;
    rdfs:subClassOf skos:Concept ;
    skos:definition "GenericOccupiedSpaceUsageValue is a code list that enumerates the different uses of a GenericOccupiedSpace."@en .

gen:GenericThematicSurface a owl:Class ;
    rdfs:label "GenericThematicSurface"@en ;
    rdfs:subClassOf [ a owl:Restriction ;
            owl:allValuesFrom gen:GenericUnoccupiedSpaceUsageValue ;
            owl:onProperty <https://www.opengis.net/ont/citygml/common/usage> ],
        [ a owl:Restriction ;
            owl:allValuesFrom gen:GenericUnoccupiedSpaceFunctionValue ;
            owl:onProperty <https://www.opengis.net/ont/citygml/common/function> ],
        [ a owl:Restriction ;
            owl:allValuesFrom gen:GenericUnoccupiedSpaceClassValue ;
            owl:onProperty <https://www.opengis.net/ont/citygml/common/class> ],
        [ a owl:Restriction ;
            owl:maxQualifiedCardinality "1"^^xsd:nonNegativeInteger ;
            owl:onClass gen:GenericUnoccupiedSpaceClassValue ;
            owl:onProperty <https://www.opengis.net/ont/citygml/common/class> ],
        core:AbstractThematicSurface .

gen:GenericThematicSurfaceClassValue a owl:Class ;
    rdfs:label "GenericThematicSurfaceClassValue"@en ;
    rdfs:subClassOf skos:Concept ;
    skos:definition "GenericThematicSurfaceClassValue is a code list used to further classify a GenericThematicSurface."@en .

gen:GenericThematicSurfaceFunctionValue a owl:Class ;
    rdfs:label "GenericThematicSurfaceFunctionValue"@en ;
    rdfs:subClassOf skos:Concept ;
    skos:definition "GenericThematicSurfaceFunctionValue is a code list that enumerates the different purposes of a GenericThematicSurface."@en .

gen:GenericThematicSurfaceUsageValue a owl:Class ;
    rdfs:label "GenericThematicSurfaceUsageValue"@en ;
    rdfs:subClassOf skos:Concept ;
    skos:definition "GenericThematicSurfaceUsageValue is a code list that enumerates the different uses of a GenericThematicSurface."@en .

gen:GenericUnoccupiedSpace a owl:Class ;
    rdfs:label "GenericUnoccupiedSpace"@en ;
    rdfs:subClassOf [ a owl:Restriction ;
            owl:allValuesFrom gen:GenericUnoccupiedSpaceUsageValue ;
            owl:onProperty <https://www.opengis.net/ont/citygml/common/usage> ],
        [ a owl:Restriction ;
            owl:allValuesFrom gen:GenericUnoccupiedSpaceFunctionValue ;
            owl:onProperty <https://www.opengis.net/ont/citygml/common/function> ],
        [ a owl:Restriction ;
            owl:allValuesFrom gen:GenericUnoccupiedSpaceClassValue ;
            owl:onProperty <https://www.opengis.net/ont/citygml/common/class> ],
        [ a owl:Restriction ;
            owl:maxQualifiedCardinality "1"^^xsd:nonNegativeInteger ;
            owl:onClass gen:GenericUnoccupiedSpaceClassValue ;
            owl:onProperty <https://www.opengis.net/ont/citygml/common/class> ],
        core:AbstractUnoccupiedSpace .

gen:IntAttribute a owl:Class ;
    rdfs:label "IntAttribute"@en ;
    rdfs:subClassOf [ a owl:Restriction ;
            owl:allValuesFrom xsd:double ;
            owl:onProperty <https://www.opengis.net/ont/citygml/common/value> ],
        [ a owl:Restriction ;
            owl:onDataRange xsd:double ;
            owl:onProperty <https://www.opengis.net/ont/citygml/common/value> ;
            owl:qualifiedCardinality "1"^^xsd:nonNegativeInteger ],
        [ a owl:Restriction ;
            owl:allValuesFrom xsd:string ;
            owl:onProperty <https://www.opengis.net/ont/citygml/common/name> ],
        [ a owl:Restriction ;
            owl:onDataRange xsd:string ;
            owl:onProperty <https://www.opengis.net/ont/citygml/common/name> ;
            owl:qualifiedCardinality "1"^^xsd:nonNegativeInteger ],
        core:AbstractGenericAttribute ;
    skos:definition "IntAttribute is a data type used to define generic attributes of type \"Integer\"."@en .

gen:MeasureAttribute a owl:Class ;
    rdfs:label "MeasureAttribute"@en ;
    rdfs:subClassOf [ a owl:Restriction ;
            owl:allValuesFrom xsd:double ;
            owl:onProperty <https://www.opengis.net/ont/citygml/common/value> ],
        [ a owl:Restriction ;
            owl:onDataRange xsd:double ;
            owl:onProperty <https://www.opengis.net/ont/citygml/common/value> ;
            owl:qualifiedCardinality "1"^^xsd:nonNegativeInteger ],
        [ a owl:Restriction ;
            owl:allValuesFrom xsd:string ;
            owl:onProperty <https://www.opengis.net/ont/citygml/common/name> ],
        [ a owl:Restriction ;
            owl:onDataRange xsd:string ;
            owl:onProperty <https://www.opengis.net/ont/citygml/common/name> ;
            owl:qualifiedCardinality "1"^^xsd:nonNegativeInteger ],
        core:AbstractGenericAttribute ;
    skos:definition "MeasureAttribute is a data type used to define generic attributes of type \"Measure\"."@en .

gen:StringAttribute a owl:Class ;
    rdfs:label "StringAttribute"@en ;
    rdfs:subClassOf [ a owl:Restriction ;
            owl:allValuesFrom xsd:double ;
            owl:onProperty <https://www.opengis.net/ont/citygml/common/value> ],
        [ a owl:Restriction ;
            owl:onDataRange xsd:double ;
            owl:onProperty <https://www.opengis.net/ont/citygml/common/value> ;
            owl:qualifiedCardinality "1"^^xsd:nonNegativeInteger ],
        [ a owl:Restriction ;
            owl:allValuesFrom xsd:string ;
            owl:onProperty <https://www.opengis.net/ont/citygml/common/name> ],
        [ a owl:Restriction ;
            owl:onDataRange xsd:string ;
            owl:onProperty <https://www.opengis.net/ont/citygml/common/name> ;
            owl:qualifiedCardinality "1"^^xsd:nonNegativeInteger ],
        core:AbstractGenericAttribute ;
    skos:definition "StringAttribute is a data type used to define generic attributes of type \"String\"."@en .

gen:UriAttribute a owl:Class ;
    rdfs:label "UriAttribute"@en ;
    rdfs:subClassOf [ a owl:Restriction ;
            owl:allValuesFrom xsd:double ;
            owl:onProperty <https://www.opengis.net/ont/citygml/common/value> ],
        [ a owl:Restriction ;
            owl:onDataRange xsd:double ;
            owl:onProperty <https://www.opengis.net/ont/citygml/common/value> ;
            owl:qualifiedCardinality "1"^^xsd:nonNegativeInteger ],
        [ a owl:Restriction ;
            owl:allValuesFrom xsd:string ;
            owl:onProperty <https://www.opengis.net/ont/citygml/common/name> ],
        [ a owl:Restriction ;
            owl:onDataRange xsd:string ;
            owl:onProperty <https://www.opengis.net/ont/citygml/common/name> ;
            owl:qualifiedCardinality "1"^^xsd:nonNegativeInteger ],
        core:AbstractGenericAttribute ;
    skos:definition "UriAttribute is a data type used to define generic attributes of type \"URI\"."@en .

gen:GenericAttributeSet a owl:Class ;
    rdfs:label "GenericAttributeSet"@en ;
    rdfs:subClassOf [ a owl:Restriction ;
            owl:allValuesFrom xsd:anyURI ;
            owl:onProperty gen:codeSpace ],
        [ a owl:Restriction ;
            owl:onDataRange xsd:string ;
            owl:onProperty <https://www.opengis.net/ont/citygml/common/name> ;
            owl:qualifiedCardinality "1"^^xsd:nonNegativeInteger ],
        [ a owl:Restriction ;
            owl:allValuesFrom xsd:string ;
            owl:onProperty <https://www.opengis.net/ont/citygml/common/name> ],
        [ a owl:Restriction ;
            owl:minQualifiedCardinality "1"^^xsd:nonNegativeInteger ;
            owl:onClass core:AbstractGenericAttribute ;
            owl:onProperty <https://www.opengis.net/ont/citygml/common/genericAttribute> ],
        [ a owl:Restriction ;
            owl:maxQualifiedCardinality "1"^^xsd:nonNegativeInteger ;
            owl:onDataRange xsd:anyURI ;
            owl:onProperty gen:codeSpace ],
        [ a owl:Restriction ;
            owl:allValuesFrom core:AbstractGenericAttribute ;
            owl:onProperty <https://www.opengis.net/ont/citygml/common/genericAttribute> ],
        core:AbstractGenericAttribute ;
    skos:definition "A GenericAttributeSet is a named collection of generic attributes."@en .

<https://www.opengis.net/ont/citygml/common/genericAttribute> skos:definition "Relates to the generic attributes that are part of the GenericAttributeSet."@en ;
    schema:domainIncludes gen:GenericAttributeSet ;
    schema:rangeIncludes core:AbstractGenericAttribute .

gen:codeSpace a owl:DatatypeProperty ;
    rdfs:label "codeSpace"@en ;
    rdfs:range xsd:anyURI ;
    skos:definition "Associates the GenericAttributeSet with an authority that maintains the collection of generic attributes."@en .

<https://www.opengis.net/ont/citygml/common/function> rdfs:label "function"@en ;
    skos:definition "Specifies the intended purposes of the GenericUnoccupiedSpace."@en ;
    schema:rangeIncludes gen:GenericUnoccupiedSpaceFunctionValue .

<https://www.opengis.net/ont/citygml/common/usage> rdfs:label "usage"@en ;
    skos:definition "Specifies the actual uses of the GenericUnoccupiedSpace."@en ;
    schema:rangeIncludes gen:GenericUnoccupiedSpaceUsageValue .

gen:GenericUnoccupiedSpaceFunctionValue a owl:Class ;
    rdfs:label "GenericUnoccupiedSpaceFunctionValue"@en ;
    rdfs:subClassOf skos:Concept ;
    skos:definition "GenericUnoccupiedSpaceFunctionValue is a code list that enumerates the different purposes of a GenericUnoccupiedSpace."@en .

gen:GenericUnoccupiedSpaceUsageValue a owl:Class ;
    rdfs:label "GenericUnoccupiedSpaceUsageValue"@en ;
    rdfs:subClassOf skos:Concept ;
    skos:definition "GenericUnoccupiedSpaceUsageValue is a code list that enumerates the different uses of a GenericUnoccupiedSpace."@en .

<https://www.opengis.net/ont/citygml/common/class> rdfs:label "class"@en ;
    skos:definition "Indicates the specific type of the GenericUnoccupiedSpace."@en ;
    schema:rangeIncludes gen:GenericUnoccupiedSpaceClassValue .

gen:GenericUnoccupiedSpaceClassValue a owl:Class ;
    rdfs:label "GenericUnoccupiedSpaceClassValue"@en ;
    rdfs:subClassOf skos:Concept ;
    skos:definition "GenericUnoccupiedSpaceClassValue is a code list used to further classify a GenericUnoccupiedSpace."@en .

<https://www.opengis.net/ont/citygml/common/value> rdfs:label "value"@en ;
    skos:definition "Specifies the \"Double\" value."@en ;
    schema:rangeIncludes xsd:double .

<https://www.opengis.net/ont/citygml/common/name> rdfs:label "name"@en ;
    skos:definition "Specifies the name of the DoubleAttribute."@en ;
    schema:rangeIncludes xsd:string .

@prefix core: <https://www.opengis.net/ont/citygml/core/> .
@prefix luse: <https://www.opengis.net/ont/citygml/landuse/> .
@prefix owl: <http://www.w3.org/2002/07/owl#> .
@prefix rdfs: <http://www.w3.org/2000/01/rdf-schema#> .
@prefix schema: <https://schema.org/> .
@prefix skos: <http://www.w3.org/2004/02/skos/core#> .
@prefix xsd: <http://www.w3.org/2001/XMLSchema#> .

<https://www.opengis.net/ont/citygml/landuse> a owl:Ontology ;
    rdfs:label "LandUse"@en ;
    owl:imports <http://def.isotc211.org/iso19150/-2/2012/base>,
        <https://www.opengis.net/ont/citygml/common>,
        <https://www.opengis.net/ont/citygml/core> ;
    owl:versionIRI <https://www.opengis.net/ont/citygml/landuse/3.0.0/> ;
    owl:versionInfo "3.0.0" ;
    skos:definition "The LandUse module supports representation of areas of the earth’s surface dedicated to a specific land use."@en .

luse:LandUse a owl:Class ;
    rdfs:label "LandUse"@en ;
    rdfs:subClassOf [ a owl:Restriction ;
            owl:allValuesFrom luse:LandUseUsageValue ;
            owl:onProperty <https://www.opengis.net/ont/citygml/common/usage> ],
        [ a owl:Restriction ;
            owl:allValuesFrom luse:LandUseFunctionValue ;
            owl:onProperty <https://www.opengis.net/ont/citygml/common/function> ],
        [ a owl:Restriction ;
            owl:allValuesFrom luse:LandUseClassValue ;
            owl:onProperty <https://www.opengis.net/ont/citygml/common/class> ],
        [ a owl:Restriction ;
            owl:maxQualifiedCardinality "1"^^xsd:nonNegativeInteger ;
            owl:onClass luse:LandUseClassValue ;
            owl:onProperty <https://www.opengis.net/ont/citygml/common/class> ],
        core:AbstractThematicSurface .

<https://www.opengis.net/ont/citygml/common/function> rdfs:label "function"@en ;
    skos:definition "Specifies the intended purposes of the LandUse."@en ;
    schema:rangeIncludes luse:LandUseFunctionValue .

<https://www.opengis.net/ont/citygml/common/usage> rdfs:label "usage"@en ;
    skos:definition "Specifies the actual uses of the LandUse."@en ;
    schema:rangeIncludes luse:LandUseUsageValue .

<https://www.opengis.net/ont/citygml/common/class> rdfs:label "class"@en ;
    skos:definition "Indicates the specific type of the LandUse."@en ;
    schema:rangeIncludes luse:LandUseClassValue .

luse:LandUseFunctionValue a owl:Class ;
    rdfs:label "LandUseFunctionValue"@en ;
    rdfs:subClassOf skos:Concept ;
    skos:definition "LandUseFunctionValue is a code list that enumerates the different purposes of a LandUse."@en .

luse:LandUseUsageValue a owl:Class ;
    rdfs:label "LandUseUsageValue"@en ;
    rdfs:subClassOf skos:Concept ;
    skos:definition "LandUseUsageValue is a code list that enumerates the different uses of a LandUse."@en .

luse:LandUseClassValue a owl:Class ;
    rdfs:label "LandUseClassValue"@en ;
    rdfs:subClassOf skos:Concept ;
    skos:definition "LandUseClassValue is a code list used to further classify a LandUse."@en .

@prefix core: <https://www.opengis.net/ont/citygml/core/> .
@prefix gmlowl: <http://www.opengis.net/ont/gml#> .
@prefix owl: <http://www.w3.org/2002/07/owl#> .
@prefix pcl: <https://www.opengis.net/ont/citygml/pointcloud/> .
@prefix rdfs: <http://www.w3.org/2000/01/rdf-schema#> .
@prefix schema: <https://schema.org/> .
@prefix skos: <http://www.w3.org/2004/02/skos/core#> .
@prefix xsd: <http://www.w3.org/2001/XMLSchema#> .

<https://www.opengis.net/ont/citygml/pointcloud> a owl:Ontology ;
    rdfs:label "PointCloud"@en ;
    owl:imports <http://def.isotc211.org/iso19150/-2/2012/base>,
        <http://www.opengis.net/ont/gml>,
        <https://www.opengis.net/ont/citygml/common>,
        <https://www.opengis.net/ont/citygml/core> ;
    owl:versionIRI <https://www.opengis.net/ont/citygml/pointcloud/3.0.0/> ;
    owl:versionInfo "3.0.0" ;
    skos:definition "The PointCloud module supports representation of CityGML features by a collection of points."@en .

pcl:PointCloud a owl:Class ;
    rdfs:label "PointCloud"@en ;
    rdfs:subClassOf [ a owl:Restriction ;
            owl:maxQualifiedCardinality "1"^^xsd:nonNegativeInteger ;
            owl:onDataRange xsd:anyURI ;
            owl:onProperty pcl:pointFile ],
        [ a owl:Restriction ;
            owl:allValuesFrom core:MimeTypeValue ;
            owl:onProperty <https://www.opengis.net/ont/citygml/common/mimeType> ],
        [ a owl:Restriction ;
            owl:allValuesFrom xsd:string ;
            owl:onProperty pcl:pointFileSrsName ],
        [ a owl:Restriction ;
            owl:allValuesFrom xsd:anyURI ;
            owl:onProperty pcl:pointFile ],
        [ a owl:Restriction ;
            owl:maxQualifiedCardinality "1"^^xsd:nonNegativeInteger ;
            owl:onClass gmlowl:MultiPoint ;
            owl:onProperty pcl:points ],
        [ a owl:Restriction ;
            owl:maxQualifiedCardinality "1"^^xsd:nonNegativeInteger ;
            owl:onClass core:MimeTypeValue ;
            owl:onProperty <https://www.opengis.net/ont/citygml/common/mimeType> ],
        [ a owl:Restriction ;
            owl:allValuesFrom gmlowl:MultiPoint ;
            owl:onProperty pcl:points ],
        [ a owl:Restriction ;
            owl:maxQualifiedCardinality "1"^^xsd:nonNegativeInteger ;
            owl:onDataRange xsd:string ;
            owl:onProperty pcl:pointFileSrsName ],
        core:AbstractPointCloud .

<https://www.opengis.net/ont/citygml/common/mimeType> rdfs:label "mimeType"@en ;
    skos:definition "Specifies the MIME type of the external point cloud file."@en ;
    schema:rangeIncludes core:MimeTypeValue .

pcl:pointFile a owl:DatatypeProperty ;
    rdfs:label "pointFile"@en ;
    rdfs:range xsd:anyURI ;
    skos:definition "Specifies the URI that points to the external point cloud file."@en .

pcl:pointFileSrsName a owl:DatatypeProperty ;
    rdfs:label "pointFileSrsName"@en ;
    rdfs:range xsd:string ;
    skos:definition "Indicates the coordinate reference system used by the external point cloud file."@en .

pcl:points a owl:ObjectProperty ;
    rdfs:label "points"@en ;
    rdfs:domain pcl:PointCloud ;
    rdfs:range gmlowl:MultiPoint ;
    skos:definition "Relates to the 3D MultiPoint geometry of the PointCloud stored inline with the city model."@en .

@prefix core: <https://www.opengis.net/ont/citygml/core/> .
@prefix dem: <https://www.opengis.net/ont/citygml/relief/> .
@prefix gmlowl: <http://www.opengis.net/ont/gml#> .
@prefix iso19107-cm: <http://def.isotc211.org/iso19107/2003/CoordinateGeometry#> .
@prefix iso19123: <http://def.isotc211.org/iso19123/2005/DiscreteCoverages#> .
@prefix iso19150-2: <http://def.isotc211.org/iso19150/-2/2012/base#> .
@prefix owl: <http://www.w3.org/2002/07/owl#> .
@prefix rdf: <http://www.w3.org/1999/02/22-rdf-syntax-ns#> .
@prefix rdfs: <http://www.w3.org/2000/01/rdf-schema#> .
@prefix schema: <https://schema.org/> .
@prefix skos: <http://www.w3.org/2004/02/skos/core#> .
@prefix xsd: <http://www.w3.org/2001/XMLSchema#> .

<https://www.opengis.net/ont/citygml/relief> a owl:Ontology ;
    rdfs:label "Relief"@en ;
    owl:imports <http://def.isotc211.org/iso19150/-2/2012/base>,
        <http://www.opengis.net/ont/gml>,
        <https://www.opengis.net/ont/citygml/common>,
        <https://www.opengis.net/ont/citygml/core> ;
    owl:versionIRI <https://www.opengis.net/ont/citygml/relief/3.0.0/> ;
    owl:versionInfo "3.0.0" ;
    skos:definition "The Relief module supports representation of the terrain. CityGML supports terrain representations at different levels of detail, reflecting different accuracies or resolutions. Terrain may be specified as a regular raster or grid, as a TIN, by break lines, and/or by mass points."@en .

dem:ReliefFeature a owl:Class ;
    rdfs:label "ReliefFeature"@en ;
    rdfs:subClassOf [ a owl:Restriction ;
            owl:onClass core:IntegerBetween0and3 ;
            owl:onProperty dem:lod ;
            owl:qualifiedCardinality "1"^^xsd:nonNegativeInteger ],
        [ a owl:Restriction ;
            owl:allValuesFrom dem:AbstractReliefComponent ;
            owl:onProperty dem:reliefComponent ],
        [ a owl:Restriction ;
            owl:minQualifiedCardinality "1"^^xsd:nonNegativeInteger ;
            owl:onClass dem:AbstractReliefComponent ;
            owl:onProperty dem:reliefComponent ],
        [ a owl:Restriction ;
            owl:allValuesFrom core:IntegerBetween0and3 ;
            owl:onProperty dem:lod ],
        core:AbstractSpaceBoundary .

<https://www.opengis.net/ont/citygml/common/pointCloud> skos:definition "Relates to the 3D PointCloud of the MassPointRelief."@en ;
    schema:domainIncludes dem:MassPointRelief ;
    schema:rangeIncludes core:AbstractPointCloud .

dem:RasterRelief a owl:Class ;
    rdfs:label "RasterRelief"@en ;
    rdfs:subClassOf [ a owl:Restriction ;
            owl:allValuesFrom iso19123:CV_DiscreteGridPointCoverage ;
            owl:onProperty dem:grid ],
        [ a owl:Restriction ;
            owl:onClass iso19123:CV_DiscreteGridPointCoverage ;
            owl:onProperty dem:grid ;
            owl:qualifiedCardinality "1"^^xsd:nonNegativeInteger ],
        dem:AbstractReliefComponent .

dem:TINRelief a owl:Class ;
    rdfs:label "TINRelief"@en ;
    rdfs:subClassOf [ a owl:Restriction ;
            owl:allValuesFrom iso19107-cm:GM_TriangulatedSurface ;
            owl:onProperty dem:tin ],
        [ a owl:Restriction ;
            owl:onClass iso19107-cm:GM_TriangulatedSurface ;
            owl:onProperty dem:tin ;
            owl:qualifiedCardinality "1"^^xsd:nonNegativeInteger ],
        dem:AbstractReliefComponent .

dem:breaklines a owl:ObjectProperty ;
    rdfs:label "breaklines"@en ;
    rdfs:domain dem:BreaklineRelief ;
    rdfs:range gmlowl:MultiCurve ;
    skos:definition "Relates to the 3D MultiCurve geometry of the MassPointRelief. This association role is used to represent break lines."@en .

dem:extent a owl:ObjectProperty ;
    rdfs:label "extent"@en ;
    rdfs:domain dem:AbstractReliefComponent ;
    rdfs:range gmlowl:Surface ;
    skos:definition "Indicates the geometrical extent of the terrain component. The geometrical extent is provided as a 2D Surface geometry."@en .

dem:grid a owl:ObjectProperty ;
    rdfs:label "grid"@en ;
    rdfs:domain dem:RasterRelief ;
    rdfs:range iso19123:CV_DiscreteGridPointCoverage ;
    skos:definition "Relates to the DiscreteGridPointCoverage of the RasterRelief."@en .

dem:reliefComponent a owl:ObjectProperty ;
    rdfs:label "reliefComponent"@en ;
    rdfs:domain dem:ReliefFeature ;
    rdfs:range dem:AbstractReliefComponent ;
    skos:definition "Relates to the terrain components that are part of the ReliefFeature."@en .

dem:reliefPoints a owl:ObjectProperty ;
    rdfs:label "reliefPoints"@en ;
    rdfs:domain dem:MassPointRelief ;
    rdfs:range gmlowl:MultiPoint ;
    skos:definition "Relates to the 3D MultiPoint geometry of the MassPointRelief."@en .

dem:ridgeOrValleyLines a owl:ObjectProperty ;
    rdfs:label "ridgeOrValleyLines"@en ;
    rdfs:domain dem:BreaklineRelief ;
    rdfs:range gmlowl:MultiCurve ;
    skos:definition "Relates to the 3D MultiCurve geometry of the MassPointRelief. This association role is used to represent ridge or valley lines."@en .

dem:tin a owl:ObjectProperty ;
    rdfs:label "tin"@en ;
    rdfs:domain dem:TINRelief ;
    rdfs:range iso19107-cm:GM_TriangulatedSurface ;
    skos:definition "Relates to the triangulated surface of the TINRelief."@en .

dem:BreaklineRelief a owl:Class ;
    rdfs:label "BreaklineRelief"@en ;
    rdfs:subClassOf [ a owl:Restriction ;
            owl:allValuesFrom gmlowl:MultiCurve ;
            owl:onProperty dem:ridgeOrValleyLines ],
        [ a owl:Restriction ;
            owl:maxQualifiedCardinality "1"^^xsd:nonNegativeInteger ;
            owl:onClass gmlowl:MultiCurve ;
            owl:onProperty dem:ridgeOrValleyLines ],
        [ a owl:Restriction ;
            owl:allValuesFrom gmlowl:MultiCurve ;
            owl:onProperty dem:breaklines ],
        [ a owl:Restriction ;
            owl:maxQualifiedCardinality "1"^^xsd:nonNegativeInteger ;
            owl:onClass gmlowl:MultiCurve ;
            owl:onProperty dem:breaklines ],
        dem:AbstractReliefComponent .

dem:MassPointRelief a owl:Class ;
    rdfs:label "MassPointRelief"@en ;
    rdfs:subClassOf [ a owl:Restriction ;
            owl:allValuesFrom gmlowl:MultiPoint ;
            owl:onProperty dem:reliefPoints ],
        [ a owl:Restriction ;
            owl:maxQualifiedCardinality "1"^^xsd:nonNegativeInteger ;
            owl:onClass gmlowl:MultiPoint ;
            owl:onProperty dem:reliefPoints ],
        [ a owl:Restriction ;
            owl:allValuesFrom core:AbstractPointCloud ;
            owl:onProperty <https://www.opengis.net/ont/citygml/common/pointCloud> ],
        [ a owl:Restriction ;
            owl:maxQualifiedCardinality "1"^^xsd:nonNegativeInteger ;
            owl:onClass core:AbstractPointCloud ;
            owl:onProperty <https://www.opengis.net/ont/citygml/common/pointCloud> ],
        dem:AbstractReliefComponent .

dem:lod a owl:ObjectProperty ;
    rdfs:label "lod"@en ;
    rdfs:range core:IntegerBetween0and3 ;
    skos:definition "Indicates the Level of Detail of the terrain component."@en .

dem:AbstractReliefComponent a owl:Class ;
    rdfs:label "AbstractReliefComponent"@en ;
    iso19150-2:isAbstract true ;
    rdfs:subClassOf [ a owl:Restriction ;
            owl:allValuesFrom core:IntegerBetween0and3 ;
            owl:onProperty dem:lod ],
        [ a owl:Restriction ;
            owl:onClass core:IntegerBetween0and3 ;
            owl:onProperty dem:lod ;
            owl:qualifiedCardinality "1"^^xsd:nonNegativeInteger ],
        [ a owl:Restriction ;
            owl:allValuesFrom gmlowl:Surface ;
            owl:onProperty dem:extent ],
        [ a owl:Restriction ;
            owl:maxQualifiedCardinality "1"^^xsd:nonNegativeInteger ;
            owl:onClass gmlowl:Surface ;
            owl:onProperty dem:extent ],
        core:AbstractSpaceBoundary .

[] a owl:AllDisjointClasses ;
    owl:members ( dem:BreaklineRelief dem:MassPointRelief dem:RasterRelief dem:TINRelief ) .

@prefix owl:   <http://www.w3.org/2002/07/owl#> .
@prefix skos:  <http://www.w3.org/2004/02/skos/core#> .
@prefix rdfs:  <http://www.w3.org/2000/01/rdf-schema#> .
@prefix vers:  <https://www.opengis.net/ont/citygml/versioning/> .
@prefix type:  <https://www.opengis.net/ont/citygml/type#> .

<https://www.opengis.net/ont/citygml/type> a owl:Ontology ;
    rdfs:label "Type"@en ;
    owl:imports <http://www.w3.org/2004/02/skos/core>,
        <https://www.opengis.net/ont/citygml/versioning>;
    skos:definition "An ontology containing the default values, schemes, and collections for the CityGML 3.0 transactionType concept."@en .


type:transactionTypeScheme a    skos:ConceptScheme,
                                owl:NamedIndividual ;
    skos:definition  "An SKOS Concept Scheme of the TransactionTypeValues from the CityGML 3.0 Versioning module."@en .

type:insert a   vers:TransactionTypeValue,
                owl:NamedIndividual ;
    rdfs:label       "insert"@en ;
    skos:inScheme    vers:transactionTypeScheme ;
    skos:definition  "A new feature is added to the version."@en .

type:delete a   vers:TransactionTypeValue,
                owl:NamedIndividual ;
    rdfs:label       "delete"@en ;
    skos:inScheme    vers:transactionTypeScheme ;
    skos:definition  "An old feature is removed from the version."@en .

type:replace a  vers:TransactionTypeValue,
                owl:NamedIndividual ;
    rdfs:label       "replace"@en ;
    skos:inScheme    vers:transactionTypeScheme ;
    skos:definition  "An old feature is replaced with a new feature between versions."@en .

type:defaultTransactionTypes a  skos:Collection,
                                owl:NamedIndividual ;
    rdfs:label       "defaultTransactionTypes"@en ;
    skos:member      type:insert,
                     type:delete,
                     type:replace ;
    skos:definition  "An SKOS collection for the default transaction type values from the CityGML 3.0 Versioning module."@en .
@prefix core: <https://www.opengis.net/ont/citygml/core/> .
@prefix iso19150-2: <http://def.isotc211.org/iso19150/-2/2012/base#> .
@prefix owl: <http://www.w3.org/2002/07/owl#> .
@prefix rdf: <http://www.w3.org/1999/02/22-rdf-syntax-ns#> .
@prefix rdfs: <http://www.w3.org/2000/01/rdf-schema#> .
@prefix schema: <https://schema.org/> .
@prefix skos: <http://www.w3.org/2004/02/skos/core#> .
@prefix tran: <https://www.opengis.net/ont/citygml/transportation/> .
@prefix xsd: <http://www.w3.org/2001/XMLSchema#> .

<https://www.opengis.net/ont/citygml/transportation> a owl:Ontology ;
    rdfs:label "Transportation"@en ;
    owl:imports <http://def.isotc211.org/iso19150/-2/2012/base>,
        <https://www.opengis.net/ont/citygml/common>,
        <https://www.opengis.net/ont/citygml/core> ;
    owl:versionIRI <https://www.opengis.net/ont/citygml/transportation/3.0.0/> ;
    owl:versionInfo "3.0.0" ;
    skos:definition "The Transportation module supports representation of the transportation infrastructure. Transportation features include roads, tracks, waterways, railways, and squares. Transportation features may be represented as a network and/or as a collection of spaces or surface elements embedded in a three-dimensional space."@en .

tran:AuxiliaryTrafficAreaClassValue a owl:Class ;
    rdfs:label "AuxiliaryTrafficAreaClassValue"@en ;
    rdfs:subClassOf skos:Concept ;
    skos:definition "AuxiliaryTrafficAreaClassValue is a code list used to further classify an AuxiliaryTrafficArea."@en .

tran:AuxiliaryTrafficAreaFunctionValue a owl:Class ;
    rdfs:label "AuxiliaryTrafficAreaFunctionValue"@en ;
    rdfs:subClassOf skos:Concept ;
    skos:definition "AuxiliaryTrafficAreaFunctionValue is a code list that enumerates the different purposes of an AuxiliaryTrafficArea."@en .

tran:AuxiliaryTrafficAreaUsageValue a owl:Class ;
    rdfs:label "AuxiliaryTrafficAreaUsageValue"@en ;
    rdfs:subClassOf skos:Concept ;
    skos:definition "AuxiliaryTrafficAreaUsageValue is a code list that enumerates the different uses of an AuxiliaryTrafficArea."@en .

tran:AuxiliaryTrafficSpaceClassValue a owl:Class ;
    rdfs:label "AuxiliaryTrafficSpaceClassValue"@en ;
    rdfs:subClassOf skos:Concept ;
    skos:definition "AuxiliaryTrafficSpaceClassValue is a code list used to further classify an AuxiliaryTrafficSpace."@en .

tran:AuxiliaryTrafficSpaceFunctionValue a owl:Class ;
    rdfs:label "AuxiliaryTrafficSpaceFunctionValue"@en ;
    rdfs:subClassOf skos:Concept ;
    skos:definition "AuxiliaryTrafficSpaceFunctionValue is a code list that enumerates the different purposes of an AuxiliaryTrafficSpace."@en .

tran:AuxiliaryTrafficSpaceUsageValue a owl:Class ;
    rdfs:label "AuxiliaryTrafficSpaceUsageValue"@en ;
    rdfs:subClassOf skos:Concept ;
    skos:definition "AuxiliaryTrafficSpaceUsageValue is a code list that enumerates the different uses of an AuxiliaryTrafficSpace."@en .

tran:ClearanceSpaceClassValue a owl:Class ;
    rdfs:label "ClearanceSpaceClassValue"@en ;
    rdfs:subClassOf skos:Concept ;
    skos:definition "ClearanceSpaceClassValue is a code list used to further classify a ClearanceSpace."@en .

tran:HoleClassValue a owl:Class ;
    rdfs:label "HoleClassValue"@en ;
    rdfs:subClassOf skos:Concept ;
    skos:definition "HoleClassValue is a code list used to further classify a Hole."@en .

tran:HoleSurface a owl:Class ;
    rdfs:label "HoleSurface"@en ;
    rdfs:subClassOf core:AbstractThematicSurface .

tran:IntersectionClassValue a owl:Class ;
    rdfs:label "IntersectionClassValue"@en ;
    rdfs:subClassOf skos:Concept ;
    skos:definition "IntersectionClassValue is a code list used to further classify an Intersection."@en .

tran:MarkingClassValue a owl:Class ;
    rdfs:label "MarkingClassValue"@en ;
    rdfs:subClassOf skos:Concept ;
    skos:definition "MarkingClassValue is a code list used to further classify a Marking."@en .

tran:RailwayClassValue a owl:Class ;
    rdfs:label "RailwayClassValue"@en ;
    rdfs:subClassOf skos:Concept ;
    skos:definition "RailwayClassValue is a code list used to further classify a Railway."@en .

tran:RailwayFunctionValue a owl:Class ;
    rdfs:label "RailwayFunctionValue"@en ;
    rdfs:subClassOf skos:Concept ;
    skos:definition "RailwayFunctionValue is a code list that enumerates the different purposes of a Railway."@en .

tran:RailwayUsageValue a owl:Class ;
    rdfs:label "RailwayUsageValue"@en ;
    rdfs:subClassOf skos:Concept ;
    skos:definition "RailwayUsageValue is a code list that enumerates the different uses of a Railway."@en .

tran:SectionClassValue a owl:Class ;
    rdfs:label "SectionClassValue"@en ;
    rdfs:subClassOf skos:Concept ;
    skos:definition "SectionClassValue is a code list used to further classify a Section."@en .

tran:SquareClassValue a owl:Class ;
    rdfs:label "SquareClassValue"@en ;
    rdfs:subClassOf skos:Concept ;
    skos:definition "SquareClassValue is a code list used to further classify a Square."@en .

tran:SquareFunctionValue a owl:Class ;
    rdfs:label "SquareFunctionValue"@en ;
    rdfs:subClassOf skos:Concept ;
    skos:definition "SquareFunctionValue is a code list that enumerates the different purposes of a Square."@en .

tran:SquareUsageValue a owl:Class ;
    rdfs:label "SquareUsageValue"@en ;
    rdfs:subClassOf skos:Concept ;
    skos:definition "SquareUsageValue is a code list that enumerates the different uses of a Square."@en .

tran:TrackClassValue a owl:Class ;
    rdfs:label "TrackClassValue"@en ;
    rdfs:subClassOf skos:Concept ;
    skos:definition "TrackClassValue is a code list used to further classify a Track."@en .

tran:TrackFunctionValue a owl:Class ;
    rdfs:label "TrackFunctionValue"@en ;
    rdfs:subClassOf skos:Concept ;
    skos:definition "TrackFunctionValue is a code list that enumerates the different purposes of a Track."@en .

tran:TrackUsageValue a owl:Class ;
    rdfs:label "TrackUsageValue"@en ;
    rdfs:subClassOf skos:Concept ;
    skos:definition "TrackUsageValue is a code list that enumerates the different uses of a Track."@en .

tran:TrafficAreaClassValue a owl:Class ;
    rdfs:label "TrafficAreaClassValue"@en ;
    rdfs:subClassOf skos:Concept ;
    skos:definition "TrafficAreaClassValue is a code list used to further classify a TrafficArea."@en .

tran:TrafficAreaFunctionValue a owl:Class ;
    rdfs:label "TrafficAreaFunctionValue"@en ;
    rdfs:subClassOf skos:Concept ;
    skos:definition "TrafficAreaFunctionValue is a code list that enumerates the different purposes of a TrafficArea."@en .

tran:TrafficAreaUsageValue a owl:Class ;
    rdfs:label "TrafficAreaUsageValue"@en ;
    rdfs:subClassOf skos:Concept ;
    skos:definition "TrafficAreaUsageValue is a code list that enumerates the different uses of a TrafficArea."@en .

tran:TrafficSpaceClassValue a owl:Class ;
    rdfs:label "TrafficSpaceClassValue"@en ;
    rdfs:subClassOf skos:Concept ;
    skos:definition "TrafficSpaceClassValue is a code list used to further classify a TrafficSpace."@en .

tran:TrafficSpaceFunctionValue a owl:Class ;
    rdfs:label "TrafficSpaceFunctionValue"@en ;
    rdfs:subClassOf skos:Concept ;
    skos:definition "TrafficSpaceFunctionValue is a code list that enumerates the different purposes of a TrafficSpace."@en .

tran:TrafficSpaceUsageValue a owl:Class ;
    rdfs:label "TrafficSpaceUsageValue"@en ;
    rdfs:subClassOf skos:Concept ;
    skos:definition "TrafficSpaceUsageValue is a code list that enumerates the different uses of a TrafficSpace."@en .

tran:WaterwayClassValue a owl:Class ;
    rdfs:label "WaterwayClassValue"@en ;
    rdfs:subClassOf skos:Concept ;
    skos:definition "WaterwayClassValue is a code list used to further classify a Waterway."@en .

tran:WaterwayFunctionValue a owl:Class ;
    rdfs:label "WaterwayFunctionValue"@en ;
    rdfs:subClassOf skos:Concept ;
    skos:definition "WaterwayFunctionValue is a code list that enumerates the different purposes of a Waterway."@en .

tran:WaterwayUsageValue a owl:Class ;
    rdfs:label "WaterwayUsageValue"@en ;
    rdfs:subClassOf skos:Concept ;
    skos:definition "WaterwayUsageValue is a code list that enumerates the different uses of a Waterway."@en .

tran:Square a owl:Class ;
    rdfs:label "Square"@en ;
    rdfs:subClassOf [ a owl:Restriction ;
            owl:allValuesFrom tran:RoadUsageValue ;
            owl:onProperty <https://www.opengis.net/ont/citygml/common/usage> ],
        [ a owl:Restriction ;
            owl:allValuesFrom tran:RoadFunctionValue ;
            owl:onProperty <https://www.opengis.net/ont/citygml/common/function> ],
        [ a owl:Restriction ;
            owl:allValuesFrom tran:RoadClassValue ;
            owl:onProperty <https://www.opengis.net/ont/citygml/common/class> ],
        [ a owl:Restriction ;
            owl:maxQualifiedCardinality "1"^^xsd:nonNegativeInteger ;
            owl:onClass tran:RoadClassValue ;
            owl:onProperty <https://www.opengis.net/ont/citygml/common/class> ],
        tran:AbstractTransportationSpace .

tran:auxiliaryTrafficSpace a owl:ObjectProperty ;
    rdfs:label "auxiliaryTrafficSpace"@en ;
    rdfs:domain tran:AbstractTransportationSpace ;
    rdfs:range tran:AuxiliaryTrafficSpace ;
    skos:definition "Relates to the auxiliary traffic spaces that are part of the transportation space."@en .

tran:clearanceSpace a owl:ObjectProperty ;
    rdfs:label "clearanceSpace"@en ;
    rdfs:domain tran:TrafficSpace ;
    rdfs:range tran:ClearanceSpace ;
    skos:definition "Relates to the clearance spaces that are part of the TrafficSpace."@en .

tran:hole a owl:ObjectProperty ;
    rdfs:label "hole"@en ;
    rdfs:domain tran:AbstractTransportationSpace ;
    rdfs:range tran:Hole ;
    skos:definition "Relates to the holes that are part of the transportation space."@en .

tran:marking a owl:ObjectProperty ;
    rdfs:label "marking"@en ;
    rdfs:domain tran:AbstractTransportationSpace ;
    rdfs:range tran:Marking ;
    skos:definition "Relates to the markings that are part of the transportation space."@en .

tran:predecessor a owl:ObjectProperty ;
    rdfs:label "predecessor"@en ;
    rdfs:domain tran:TrafficSpace ;
    rdfs:range tran:TrafficSpace ;
    skos:definition "Indicates the predecessor(s) of the TrafficSpace."@en .

tran:successor a owl:ObjectProperty ;
    rdfs:label "successor"@en ;
    rdfs:domain tran:TrafficSpace ;
    rdfs:range tran:TrafficSpace ;
    skos:definition "Indicates the successor(s) of the TrafficSpace."@en .

tran:trafficSpace a owl:ObjectProperty ;
    rdfs:label "trafficSpace"@en ;
    rdfs:domain tran:AbstractTransportationSpace ;
    rdfs:range tran:TrafficSpace ;
    skos:definition "Relates to the traffic spaces that are part of the transportation space."@en .

<https://www.opengis.net/ont/citygml/common/boundary> skos:definition "Relates to the auxiliary traffic areas that bound the AuxiliaryTrafficSpace. This relation is inherited from the Core module."@en,
        "Relates to the traffic areas that bound the TrafficSpace. This relation is inherited from the Core module."@en ;
    schema:domainIncludes tran:AuxiliaryTrafficSpace,
        tran:TrafficSpace ;
    schema:rangeIncludes tran:AuxiliaryTrafficArea,
        tran:TrafficArea .

<https://www.opengis.net/ont/citygml/common/occupancy> rdfs:label "occupancy"@en ;
    skos:definition "Provides information on the residency of persons, vehicles, or other moving features in the transportation space."@en ;
    schema:rangeIncludes core:Occupancy .

tran:AuxiliaryTrafficArea a owl:Class ;
    rdfs:label "AuxiliaryTrafficArea"@en ;
    rdfs:subClassOf [ a owl:Restriction ;
            owl:allValuesFrom tran:RoadUsageValue ;
            owl:onProperty <https://www.opengis.net/ont/citygml/common/usage> ],
        [ a owl:Restriction ;
            owl:allValuesFrom tran:SurfaceMaterialValue ;
            owl:onProperty tran:surfaceMaterial ],
        [ a owl:Restriction ;
            owl:maxQualifiedCardinality "1"^^xsd:nonNegativeInteger ;
            owl:onClass tran:RoadClassValue ;
            owl:onProperty <https://www.opengis.net/ont/citygml/common/class> ],
        [ a owl:Restriction ;
            owl:allValuesFrom tran:RoadFunctionValue ;
            owl:onProperty <https://www.opengis.net/ont/citygml/common/function> ],
        [ a owl:Restriction ;
            owl:maxQualifiedCardinality "1"^^xsd:nonNegativeInteger ;
            owl:onClass tran:SurfaceMaterialValue ;
            owl:onProperty tran:surfaceMaterial ],
        [ a owl:Restriction ;
            owl:allValuesFrom tran:RoadClassValue ;
            owl:onProperty <https://www.opengis.net/ont/citygml/common/class> ],
        core:AbstractThematicSurface .

tran:ClearanceSpace a owl:Class ;
    rdfs:label "ClearanceSpace"@en ;
    rdfs:subClassOf [ a owl:Restriction ;
            owl:allValuesFrom tran:RoadClassValue ;
            owl:onProperty <https://www.opengis.net/ont/citygml/common/class> ],
        core:AbstractUnoccupiedSpace .

tran:Hole a owl:Class ;
    rdfs:label "Hole"@en ;
    rdfs:subClassOf [ a owl:Restriction ;
            owl:allValuesFrom tran:RoadClassValue ;
            owl:onProperty <https://www.opengis.net/ont/citygml/common/class> ],
        [ a owl:Restriction ;
            owl:maxQualifiedCardinality "1"^^xsd:nonNegativeInteger ;
            owl:onClass tran:RoadClassValue ;
            owl:onProperty <https://www.opengis.net/ont/citygml/common/class> ],
        core:AbstractUnoccupiedSpace .

tran:Marking a owl:Class ;
    rdfs:label "Marking"@en ;
    rdfs:subClassOf [ a owl:Restriction ;
            owl:allValuesFrom tran:RoadClassValue ;
            owl:onProperty <https://www.opengis.net/ont/citygml/common/class> ],
        [ a owl:Restriction ;
            owl:maxQualifiedCardinality "1"^^xsd:nonNegativeInteger ;
            owl:onClass tran:RoadClassValue ;
            owl:onProperty <https://www.opengis.net/ont/citygml/common/class> ],
        core:AbstractThematicSurface .

tran:TrafficArea a owl:Class ;
    rdfs:label "TrafficArea"@en ;
    rdfs:subClassOf [ a owl:Restriction ;
            owl:allValuesFrom tran:RoadFunctionValue ;
            owl:onProperty <https://www.opengis.net/ont/citygml/common/function> ],
        [ a owl:Restriction ;
            owl:maxQualifiedCardinality "1"^^xsd:nonNegativeInteger ;
            owl:onClass tran:SurfaceMaterialValue ;
            owl:onProperty tran:surfaceMaterial ],
        [ a owl:Restriction ;
            owl:allValuesFrom tran:RoadClassValue ;
            owl:onProperty <https://www.opengis.net/ont/citygml/common/class> ],
        [ a owl:Restriction ;
            owl:allValuesFrom tran:SurfaceMaterialValue ;
            owl:onProperty tran:surfaceMaterial ],
        [ a owl:Restriction ;
            owl:maxQualifiedCardinality "1"^^xsd:nonNegativeInteger ;
            owl:onClass tran:RoadClassValue ;
            owl:onProperty <https://www.opengis.net/ont/citygml/common/class> ],
        [ a owl:Restriction ;
            owl:allValuesFrom tran:RoadUsageValue ;
            owl:onProperty <https://www.opengis.net/ont/citygml/common/usage> ],
        core:AbstractThematicSurface .

tran:AuxiliaryTrafficSpace a owl:Class ;
    rdfs:label "AuxiliaryTrafficSpace"@en ;
    rdfs:subClassOf [ a owl:Restriction ;
            owl:allValuesFrom tran:RoadClassValue ;
            owl:onProperty <https://www.opengis.net/ont/citygml/common/class> ],
        [ a owl:Restriction ;
            owl:allValuesFrom tran:GranularityValue ;
            owl:onProperty tran:granularity ],
        [ a owl:Restriction ;
            owl:maxQualifiedCardinality "1"^^xsd:nonNegativeInteger ;
            owl:onClass tran:RoadClassValue ;
            owl:onProperty <https://www.opengis.net/ont/citygml/common/class> ],
        [ a owl:Restriction ;
            owl:onDataRange tran:GranularityValue ;
            owl:onProperty tran:granularity ;
            owl:qualifiedCardinality "1"^^xsd:nonNegativeInteger ],
        [ a owl:Restriction ;
            owl:allValuesFrom tran:RoadFunctionValue ;
            owl:onProperty <https://www.opengis.net/ont/citygml/common/function> ],
        [ a owl:Restriction ;
            owl:allValuesFrom tran:AuxiliaryTrafficArea ;
            owl:onProperty <https://www.opengis.net/ont/citygml/common/boundary> ],
        [ a owl:Restriction ;
            owl:allValuesFrom tran:RoadUsageValue ;
            owl:onProperty <https://www.opengis.net/ont/citygml/common/usage> ],
        core:AbstractUnoccupiedSpace .

tran:Railway a owl:Class ;
    rdfs:label "Railway"@en ;
    rdfs:subClassOf [ a owl:Restriction ;
            owl:allValuesFrom tran:RoadUsageValue ;
            owl:onProperty <https://www.opengis.net/ont/citygml/common/usage> ],
        [ a owl:Restriction ;
            owl:allValuesFrom tran:RoadClassValue ;
            owl:onProperty <https://www.opengis.net/ont/citygml/common/class> ],
        [ a owl:Restriction ;
            owl:maxQualifiedCardinality "1"^^xsd:nonNegativeInteger ;
            owl:onClass tran:RoadClassValue ;
            owl:onProperty <https://www.opengis.net/ont/citygml/common/class> ],
        [ a owl:Restriction ;
            owl:allValuesFrom tran:Section ;
            owl:onProperty <https://www.opengis.net/ont/citygml/common/section> ],
        [ a owl:Restriction ;
            owl:allValuesFrom tran:Intersection ;
            owl:onProperty <https://www.opengis.net/ont/citygml/common/intersection> ],
        [ a owl:Restriction ;
            owl:allValuesFrom tran:RoadFunctionValue ;
            owl:onProperty <https://www.opengis.net/ont/citygml/common/function> ],
        tran:AbstractTransportationSpace .

tran:Road a owl:Class ;
    rdfs:label "Road"@en ;
    rdfs:subClassOf [ a owl:Restriction ;
            owl:allValuesFrom tran:RoadClassValue ;
            owl:onProperty <https://www.opengis.net/ont/citygml/common/class> ],
        [ a owl:Restriction ;
            owl:allValuesFrom tran:RoadUsageValue ;
            owl:onProperty <https://www.opengis.net/ont/citygml/common/usage> ],
        [ a owl:Restriction ;
            owl:allValuesFrom tran:Intersection ;
            owl:onProperty <https://www.opengis.net/ont/citygml/common/intersection> ],
        [ a owl:Restriction ;
            owl:allValuesFrom tran:RoadFunctionValue ;
            owl:onProperty <https://www.opengis.net/ont/citygml/common/function> ],
        [ a owl:Restriction ;
            owl:allValuesFrom tran:Section ;
            owl:onProperty <https://www.opengis.net/ont/citygml/common/section> ],
        [ a owl:Restriction ;
            owl:maxQualifiedCardinality "1"^^xsd:nonNegativeInteger ;
            owl:onClass tran:RoadClassValue ;
            owl:onProperty <https://www.opengis.net/ont/citygml/common/class> ],
        tran:AbstractTransportationSpace .

tran:Track a owl:Class ;
    rdfs:label "Track"@en ;
    rdfs:subClassOf [ a owl:Restriction ;
            owl:allValuesFrom tran:RoadUsageValue ;
            owl:onProperty <https://www.opengis.net/ont/citygml/common/usage> ],
        [ a owl:Restriction ;
            owl:allValuesFrom tran:RoadFunctionValue ;
            owl:onProperty <https://www.opengis.net/ont/citygml/common/function> ],
        [ a owl:Restriction ;
            owl:allValuesFrom tran:Section ;
            owl:onProperty <https://www.opengis.net/ont/citygml/common/section> ],
        [ a owl:Restriction ;
            owl:allValuesFrom tran:Intersection ;
            owl:onProperty <https://www.opengis.net/ont/citygml/common/intersection> ],
        [ a owl:Restriction ;
            owl:maxQualifiedCardinality "1"^^xsd:nonNegativeInteger ;
            owl:onClass tran:RoadClassValue ;
            owl:onProperty <https://www.opengis.net/ont/citygml/common/class> ],
        [ a owl:Restriction ;
            owl:allValuesFrom tran:RoadClassValue ;
            owl:onProperty <https://www.opengis.net/ont/citygml/common/class> ],
        tran:AbstractTransportationSpace .

tran:Waterway a owl:Class ;
    rdfs:label "Waterway"@en ;
    rdfs:subClassOf [ a owl:Restriction ;
            owl:allValuesFrom tran:Intersection ;
            owl:onProperty <https://www.opengis.net/ont/citygml/common/intersection> ],
        [ a owl:Restriction ;
            owl:maxQualifiedCardinality "1"^^xsd:nonNegativeInteger ;
            owl:onClass tran:RoadClassValue ;
            owl:onProperty <https://www.opengis.net/ont/citygml/common/class> ],
        [ a owl:Restriction ;
            owl:allValuesFrom tran:RoadUsageValue ;
            owl:onProperty <https://www.opengis.net/ont/citygml/common/usage> ],
        [ a owl:Restriction ;
            owl:allValuesFrom tran:RoadFunctionValue ;
            owl:onProperty <https://www.opengis.net/ont/citygml/common/function> ],
        [ a owl:Restriction ;
            owl:allValuesFrom tran:Section ;
            owl:onProperty <https://www.opengis.net/ont/citygml/common/section> ],
        [ a owl:Restriction ;
            owl:allValuesFrom tran:RoadClassValue ;
            owl:onProperty <https://www.opengis.net/ont/citygml/common/class> ],
        tran:AbstractTransportationSpace .

<https://www.opengis.net/ont/citygml/common/intersection> skos:definition "Relates to the intersections that are part of the Railway."@en,
        "Relates to the intersections that are part of the Road."@en,
        "Relates to the intersections that are part of the Track."@en,
        "Relates to the intersections that are part of the Waterway."@en ;
    schema:domainIncludes tran:Railway,
        tran:Road,
        tran:Track,
        tran:Waterway ;
    schema:rangeIncludes tran:Intersection .

<https://www.opengis.net/ont/citygml/common/section> skos:definition "Relates to the sections that are part of the Railway."@en,
        "Relates to the sections that are part of the Road."@en,
        "Relates to the sections that are part of the Track."@en,
        "Relates to the sections that are part of the Waterway."@en ;
    schema:domainIncludes tran:Railway,
        tran:Road,
        tran:Track,
        tran:Waterway ;
    schema:rangeIncludes tran:Section .

tran:granularity a owl:DatatypeProperty ;
    rdfs:label "granularity"@en ;
    rdfs:range tran:GranularityValue ;
    skos:definition "Defines whether traffic spaces are represented by individual ways or by individual lanes, depending on the desired level of spatial and semantic decomposition."@en .

tran:surfaceMaterial a owl:ObjectProperty ;
    rdfs:label "surfaceMaterial"@en ;
    rdfs:range tran:SurfaceMaterialValue ;
    skos:definition "Specifies the type of pavement of the AuxiliaryTrafficArea."@en .

tran:trafficDirection a owl:DatatypeProperty ;
    rdfs:label "trafficDirection"@en ;
    rdfs:range tran:TrafficDirectionValue ;
    skos:definition "Indicates the direction of traffic flow relative to the corresponding linear geometry representation."@en .

tran:GranularityValue a rdfs:Datatype ;
    rdfs:label "GranularityValue"@en ;
    owl:equivalentClass [ a rdfs:Datatype ;
            owl:oneOf ( "lane" "way" ) ] ;
    skos:definition "GranularityValue enumerates the different levels of granularity in which transportation objects are represented."@en .

tran:SurfaceMaterialValue a owl:Class ;
    rdfs:label "SurfaceMaterialValue"@en ;
    rdfs:subClassOf skos:Concept ;
    skos:definition "SurfaceMaterialValue is a code list that enumerates the different surface materials."@en .

tran:TrafficDirectionValue a rdfs:Datatype ;
    rdfs:label "TrafficDirectionValue"@en ;
    owl:equivalentClass [ a rdfs:Datatype ;
            owl:oneOf ( "forwards" "backwards" "both" ) ] ;
    skos:definition "TrafficDirectionValue enumerates the allowed directions of travel of a mobile object."@en .

tran:Intersection a owl:Class ;
    rdfs:label "Intersection"@en ;
    rdfs:subClassOf [ a owl:Restriction ;
            owl:allValuesFrom tran:RoadClassValue ;
            owl:onProperty <https://www.opengis.net/ont/citygml/common/class> ],
        [ a owl:Restriction ;
            owl:maxQualifiedCardinality "1"^^xsd:nonNegativeInteger ;
            owl:onClass tran:RoadClassValue ;
            owl:onProperty <https://www.opengis.net/ont/citygml/common/class> ],
        tran:AbstractTransportationSpace .

tran:Section a owl:Class ;
    rdfs:label "Section"@en ;
    rdfs:subClassOf [ a owl:Restriction ;
            owl:allValuesFrom tran:RoadClassValue ;
            owl:onProperty <https://www.opengis.net/ont/citygml/common/class> ],
        [ a owl:Restriction ;
            owl:maxQualifiedCardinality "1"^^xsd:nonNegativeInteger ;
            owl:onClass tran:RoadClassValue ;
            owl:onProperty <https://www.opengis.net/ont/citygml/common/class> ],
        tran:AbstractTransportationSpace .

<https://www.opengis.net/ont/citygml/common/function> rdfs:label "function"@en ;
    skos:definition "Specifies the intended purposes of the Road."@en ;
    schema:rangeIncludes tran:RoadFunctionValue .

<https://www.opengis.net/ont/citygml/common/usage> rdfs:label "usage"@en ;
    skos:definition "Specifies the actual uses of the Road."@en ;
    schema:rangeIncludes tran:RoadUsageValue .

tran:RoadFunctionValue a owl:Class ;
    rdfs:label "RoadFunctionValue"@en ;
    rdfs:subClassOf skos:Concept ;
    skos:definition "RoadFunctionValue is a code list that enumerates the different purposes of a Road."@en .

tran:RoadUsageValue a owl:Class ;
    rdfs:label "RoadUsageValue"@en ;
    rdfs:subClassOf skos:Concept ;
    skos:definition "RoadUsageValue is a code list that enumerates the different uses of a Road."@en .

tran:TrafficSpace a owl:Class ;
    rdfs:label "TrafficSpace"@en ;
    rdfs:subClassOf [ a owl:Restriction ;
            owl:allValuesFrom core:Occupancy ;
            owl:onProperty <https://www.opengis.net/ont/citygml/common/occupancy> ],
        [ a owl:Restriction ;
            owl:maxQualifiedCardinality "1"^^xsd:nonNegativeInteger ;
            owl:onDataRange tran:TrafficDirectionValue ;
            owl:onProperty tran:trafficDirection ],
        [ a owl:Restriction ;
            owl:maxQualifiedCardinality "1"^^xsd:nonNegativeInteger ;
            owl:onClass tran:RoadClassValue ;
            owl:onProperty <https://www.opengis.net/ont/citygml/common/class> ],
        [ a owl:Restriction ;
            owl:allValuesFrom tran:TrafficSpace ;
            owl:onProperty tran:successor ],
        [ a owl:Restriction ;
            owl:allValuesFrom tran:TrafficArea ;
            owl:onProperty <https://www.opengis.net/ont/citygml/common/boundary> ],
        [ a owl:Restriction ;
            owl:allValuesFrom tran:GranularityValue ;
            owl:onProperty tran:granularity ],
        [ a owl:Restriction ;
            owl:onDataRange tran:GranularityValue ;
            owl:onProperty tran:granularity ;
            owl:qualifiedCardinality "1"^^xsd:nonNegativeInteger ],
        [ a owl:Restriction ;
            owl:allValuesFrom tran:RoadClassValue ;
            owl:onProperty <https://www.opengis.net/ont/citygml/common/class> ],
        [ a owl:Restriction ;
            owl:allValuesFrom tran:RoadFunctionValue ;
            owl:onProperty <https://www.opengis.net/ont/citygml/common/function> ],
        [ a owl:Restriction ;
            owl:allValuesFrom tran:TrafficSpace ;
            owl:onProperty tran:predecessor ],
        [ a owl:Restriction ;
            owl:allValuesFrom tran:RoadUsageValue ;
            owl:onProperty <https://www.opengis.net/ont/citygml/common/usage> ],
        [ a owl:Restriction ;
            owl:allValuesFrom tran:ClearanceSpace ;
            owl:onProperty tran:clearanceSpace ],
        [ a owl:Restriction ;
            owl:allValuesFrom tran:TrafficDirectionValue ;
            owl:onProperty tran:trafficDirection ],
        core:AbstractUnoccupiedSpace .

tran:AbstractTransportationSpace a owl:Class ;
    rdfs:label "AbstractTransportationSpace"@en ;
    iso19150-2:isAbstract true ;
    rdfs:subClassOf [ a owl:Restriction ;
            owl:allValuesFrom tran:TrafficSpace ;
            owl:onProperty tran:trafficSpace ],
        [ a owl:Restriction ;
            owl:allValuesFrom tran:TrafficDirectionValue ;
            owl:onProperty tran:trafficDirection ],
        [ a owl:Restriction ;
            owl:allValuesFrom tran:Marking ;
            owl:onProperty tran:marking ],
        [ a owl:Restriction ;
            owl:maxQualifiedCardinality "1"^^xsd:nonNegativeInteger ;
            owl:onDataRange tran:TrafficDirectionValue ;
            owl:onProperty tran:trafficDirection ],
        [ a owl:Restriction ;
            owl:allValuesFrom core:Occupancy ;
            owl:onProperty <https://www.opengis.net/ont/citygml/common/occupancy> ],
        [ a owl:Restriction ;
            owl:allValuesFrom tran:Hole ;
            owl:onProperty tran:hole ],
        [ a owl:Restriction ;
            owl:allValuesFrom tran:AuxiliaryTrafficSpace ;
            owl:onProperty tran:auxiliaryTrafficSpace ],
        core:AbstractUnoccupiedSpace .

<https://www.opengis.net/ont/citygml/common/class> rdfs:label "class"@en ;
    skos:definition "Indicates the specific type of the Road."@en ;
    schema:rangeIncludes tran:RoadClassValue .

tran:RoadClassValue a owl:Class ;
    rdfs:label "RoadClassValue"@en ;
    rdfs:subClassOf skos:Concept ;
    skos:definition "RoadClassValue is a code list used to further classify a Road."@en .

[] a owl:AllDisjointClasses ;
    owl:members ( tran:Intersection tran:Railway tran:Road tran:Section tran:Square tran:Track tran:Waterway ) .

@prefix con: <https://www.opengis.net/ont/citygml/construction/> .
@prefix core: <https://www.opengis.net/ont/citygml/core/> .
@prefix iso19150-2: <http://def.isotc211.org/iso19150/-2/2012/base#> .
@prefix owl: <http://www.w3.org/2002/07/owl#> .
@prefix rdfs: <http://www.w3.org/2000/01/rdf-schema#> .
@prefix schema: <https://schema.org/> .
@prefix skos: <http://www.w3.org/2004/02/skos/core#> .
@prefix tun: <https://www.opengis.net/ont/citygml/tunnel/> .
@prefix xsd: <http://www.w3.org/2001/XMLSchema#> .

<https://www.opengis.net/ont/citygml/tunnel> a owl:Ontology ;
    rdfs:label "Tunnel"@en ;
    owl:imports <http://def.isotc211.org/iso19150/-2/2012/base>,
        <https://www.opengis.net/ont/citygml/common>,
        <https://www.opengis.net/ont/citygml/construction>,
        <https://www.opengis.net/ont/citygml/core> ;
    owl:versionIRI <https://www.opengis.net/ont/citygml/tunnel/3.0.0/> ;
    owl:versionInfo "3.0.0" ;
    skos:definition "The Tunnel module supports representation of thematic and spatial aspects of tunnels, tunnel parts, tunnel installations, and interior tunnel structures."@en .

tun:TunnelClassValue a owl:Class ;
    rdfs:label "TunnelClassValue"@en ;
    rdfs:subClassOf skos:Concept ;
    skos:definition "TunnelClassValue is a code list used to further classify a Tunnel."@en .

tun:TunnelConstructiveElementClassValue a owl:Class ;
    rdfs:label "TunnelConstructiveElementClassValue"@en ;
    rdfs:subClassOf skos:Concept ;
    skos:definition "TunnelConstructiveElementClassValue is a code list used to further classify a TunnelConstructiveElement."@en .

tun:TunnelConstructiveElementFunctionValue a owl:Class ;
    rdfs:label "TunnelConstructiveElementFunctionValue"@en ;
    rdfs:subClassOf skos:Concept ;
    skos:definition "TunnelConstructiveElementFunctionValue is a code list that enumerates the different purposes of a TunnelConstructiveElement."@en .

tun:TunnelConstructiveElementUsageValue a owl:Class ;
    rdfs:label "TunnelConstructiveElementUsageValue"@en ;
    rdfs:subClassOf skos:Concept ;
    skos:definition "TunnelConstructiveElementUsageValue is a code list that enumerates the different uses of a TunnelConstructiveElement."@en .

tun:TunnelFunctionValue a owl:Class ;
    rdfs:label "TunnelFunctionValue"@en ;
    rdfs:subClassOf skos:Concept ;
    skos:definition "TunnelFunctionValue is a code list that enumerates the different purposes of a Tunnel."@en .

tun:TunnelFurnitureClassValue a owl:Class ;
    rdfs:label "TunnelFurnitureClassValue"@en ;
    rdfs:subClassOf skos:Concept ;
    skos:definition "TunnelFurnitureClassValue is a code list used to further classify a TunnelFurniture."@en .

tun:TunnelFurnitureFunctionValue a owl:Class ;
    rdfs:label "TunnelFurnitureFunctionValue"@en ;
    rdfs:subClassOf skos:Concept ;
    skos:definition "TunnelFurnitureFunctionValue is a code list that enumerates the different purposes of a TunnelFurniture."@en .

tun:TunnelFurnitureUsageValue a owl:Class ;
    rdfs:label "TunnelFurnitureUsageValue"@en ;
    rdfs:subClassOf skos:Concept ;
    skos:definition "TunnelFurnitureUsageValue is a code list that enumerates the different uses of a TunnelFurniture."@en .

tun:TunnelInstallationClassValue a owl:Class ;
    rdfs:label "TunnelInstallationClassValue"@en ;
    rdfs:subClassOf skos:Concept ;
    skos:definition "TunnelInstallationClassValue is a code list used to further classify a TunnelInstallation."@en .

tun:TunnelInstallationFunctionValue a owl:Class ;
    rdfs:label "TunnelInstallationFunctionValue"@en ;
    rdfs:subClassOf skos:Concept ;
    skos:definition "TunnelInstallationFunctionValue is a code list that enumerates the different purposes of a TunnelInstallation."@en .

tun:TunnelInstallationUsageValue a owl:Class ;
    rdfs:label "TunnelInstallationUsageValue"@en ;
    rdfs:subClassOf skos:Concept ;
    skos:definition "TunnelInstallationUsageValue is a code list that enumerates the different uses of a TunnelInstallation."@en .

tun:TunnelUsageValue a owl:Class ;
    rdfs:label "TunnelUsageValue"@en ;
    rdfs:subClassOf skos:Concept ;
    skos:definition "TunnelUsageValue is a code list that enumerates the different uses of a Tunnel."@en .

<https://www.opengis.net/ont/citygml/common/boundary> skos:definition "Relates to the surfaces that bound the HollowSpace. This relation is inherited from the Core module."@en ;
    schema:domainIncludes tun:HollowSpace ;
    schema:rangeIncludes core:AbstractThematicSurface .

tun:Tunnel a owl:Class ;
    rdfs:label "Tunnel"@en ;
    rdfs:subClassOf [ a owl:Restriction ;
            owl:allValuesFrom tun:TunnelPart ;
            owl:onProperty tun:tunnelPart ],
        tun:AbstractTunnel ;
    owl:disjointWith tun:TunnelPart .

tun:hollowSpace a owl:ObjectProperty ;
    rdfs:label "hollowSpace"@en ;
    rdfs:domain tun:AbstractTunnel ;
    rdfs:range tun:HollowSpace ;
    skos:definition "Relates the hollow spaces to the Tunnel or TunnelPart."@en .

tun:tunnelConstructiveElement a owl:ObjectProperty ;
    rdfs:label "tunnelConstructiveElement"@en ;
    rdfs:domain tun:AbstractTunnel ;
    rdfs:range tun:TunnelConstructiveElement ;
    skos:definition "Relates the constructive elements to the Tunnel or TunnelPart."@en .

tun:tunnelPart a owl:ObjectProperty ;
    rdfs:label "tunnelPart"@en ;
    rdfs:domain tun:Tunnel ;
    rdfs:range tun:TunnelPart ;
    skos:definition "Relates the tunnel parts to the Tunnel."@en .

<https://www.opengis.net/ont/citygml/common/tunnelFurniture> skos:definition "Relates the furniture objects to the HollowSpace."@en,
        "Relates the furniture objects to the Tunnel or TunnelPart."@en ;
    schema:domainIncludes tun:AbstractTunnel,
        tun:HollowSpace ;
    schema:rangeIncludes tun:TunnelFurniture .

<https://www.opengis.net/ont/citygml/common/tunnelInstallation> skos:definition "Relates the installation objects to the HollowSpace."@en,
        "Relates the installation objects to the Tunnel or TunnelPart."@en ;
    schema:domainIncludes tun:AbstractTunnel,
        tun:HollowSpace ;
    schema:rangeIncludes tun:TunnelInstallation .

tun:TunnelConstructiveElement a owl:Class ;
    rdfs:label "TunnelConstructiveElement"@en ;
    rdfs:subClassOf [ a owl:Restriction ;
            owl:allValuesFrom tun:HollowSpaceUsageValue ;
            owl:onProperty <https://www.opengis.net/ont/citygml/common/usage> ],
        [ a owl:Restriction ;
            owl:allValuesFrom tun:HollowSpaceFunctionValue ;
            owl:onProperty <https://www.opengis.net/ont/citygml/common/function> ],
        [ a owl:Restriction ;
            owl:allValuesFrom tun:HollowSpaceClassValue ;
            owl:onProperty <https://www.opengis.net/ont/citygml/common/class> ],
        [ a owl:Restriction ;
            owl:maxQualifiedCardinality "1"^^xsd:nonNegativeInteger ;
            owl:onClass tun:HollowSpaceClassValue ;
            owl:onProperty <https://www.opengis.net/ont/citygml/common/class> ],
        con:AbstractConstructiveElement .

tun:TunnelFurniture a owl:Class ;
    rdfs:label "TunnelFurniture"@en ;
    rdfs:subClassOf [ a owl:Restriction ;
            owl:allValuesFrom tun:HollowSpaceClassValue ;
            owl:onProperty <https://www.opengis.net/ont/citygml/common/class> ],
        [ a owl:Restriction ;
            owl:maxQualifiedCardinality "1"^^xsd:nonNegativeInteger ;
            owl:onClass tun:HollowSpaceClassValue ;
            owl:onProperty <https://www.opengis.net/ont/citygml/common/class> ],
        [ a owl:Restriction ;
            owl:allValuesFrom tun:HollowSpaceUsageValue ;
            owl:onProperty <https://www.opengis.net/ont/citygml/common/usage> ],
        [ a owl:Restriction ;
            owl:allValuesFrom tun:HollowSpaceFunctionValue ;
            owl:onProperty <https://www.opengis.net/ont/citygml/common/function> ],
        con:AbstractFurniture .

tun:TunnelInstallation a owl:Class ;
    rdfs:label "TunnelInstallation"@en ;
    rdfs:subClassOf [ a owl:Restriction ;
            owl:allValuesFrom tun:HollowSpaceUsageValue ;
            owl:onProperty <https://www.opengis.net/ont/citygml/common/usage> ],
        [ a owl:Restriction ;
            owl:allValuesFrom tun:HollowSpaceFunctionValue ;
            owl:onProperty <https://www.opengis.net/ont/citygml/common/function> ],
        [ a owl:Restriction ;
            owl:allValuesFrom tun:HollowSpaceClassValue ;
            owl:onProperty <https://www.opengis.net/ont/citygml/common/class> ],
        [ a owl:Restriction ;
            owl:maxQualifiedCardinality "1"^^xsd:nonNegativeInteger ;
            owl:onClass tun:HollowSpaceClassValue ;
            owl:onProperty <https://www.opengis.net/ont/citygml/common/class> ],
        con:AbstractInstallation .

tun:TunnelPart a owl:Class ;
    rdfs:label "TunnelPart"@en ;
    rdfs:subClassOf tun:AbstractTunnel .

<https://www.opengis.net/ont/citygml/common/function> rdfs:label "function"@en ;
    skos:definition "Specifies the intended purposes of the HollowSpace."@en ;
    schema:rangeIncludes tun:HollowSpaceFunctionValue .

<https://www.opengis.net/ont/citygml/common/usage> rdfs:label "usage"@en ;
    skos:definition "Specifies the actual uses of the HollowSpace."@en ;
    schema:rangeIncludes tun:HollowSpaceUsageValue .

tun:HollowSpace a owl:Class ;
    rdfs:label "HollowSpace"@en ;
    rdfs:subClassOf [ a owl:Restriction ;
            owl:allValuesFrom tun:TunnelFurniture ;
            owl:onProperty <https://www.opengis.net/ont/citygml/common/tunnelFurniture> ],
        [ a owl:Restriction ;
            owl:allValuesFrom tun:TunnelInstallation ;
            owl:onProperty <https://www.opengis.net/ont/citygml/common/tunnelInstallation> ],
        [ a owl:Restriction ;
            owl:allValuesFrom core:AbstractThematicSurface ;
            owl:onProperty <https://www.opengis.net/ont/citygml/common/boundary> ],
        [ a owl:Restriction ;
            owl:allValuesFrom tun:HollowSpaceUsageValue ;
            owl:onProperty <https://www.opengis.net/ont/citygml/common/usage> ],
        [ a owl:Restriction ;
            owl:allValuesFrom tun:HollowSpaceFunctionValue ;
            owl:onProperty <https://www.opengis.net/ont/citygml/common/function> ],
        [ a owl:Restriction ;
            owl:allValuesFrom tun:HollowSpaceClassValue ;
            owl:onProperty <https://www.opengis.net/ont/citygml/common/class> ],
        [ a owl:Restriction ;
            owl:maxQualifiedCardinality "1"^^xsd:nonNegativeInteger ;
            owl:onClass tun:HollowSpaceClassValue ;
            owl:onProperty <https://www.opengis.net/ont/citygml/common/class> ],
        core:AbstractUnoccupiedSpace .

tun:AbstractTunnel a owl:Class ;
    rdfs:label "AbstractTunnel"@en ;
    iso19150-2:isAbstract true ;
    rdfs:subClassOf [ a owl:Restriction ;
            owl:maxQualifiedCardinality "1"^^xsd:nonNegativeInteger ;
            owl:onClass tun:HollowSpaceClassValue ;
            owl:onProperty <https://www.opengis.net/ont/citygml/common/class> ],
        [ a owl:Restriction ;
            owl:allValuesFrom tun:HollowSpace ;
            owl:onProperty tun:hollowSpace ],
        [ a owl:Restriction ;
            owl:allValuesFrom tun:TunnelInstallation ;
            owl:onProperty <https://www.opengis.net/ont/citygml/common/tunnelInstallation> ],
        [ a owl:Restriction ;
            owl:allValuesFrom tun:HollowSpaceClassValue ;
            owl:onProperty <https://www.opengis.net/ont/citygml/common/class> ],
        [ a owl:Restriction ;
            owl:allValuesFrom tun:HollowSpaceFunctionValue ;
            owl:onProperty <https://www.opengis.net/ont/citygml/common/function> ],
        [ a owl:Restriction ;
            owl:allValuesFrom tun:TunnelFurniture ;
            owl:onProperty <https://www.opengis.net/ont/citygml/common/tunnelFurniture> ],
        [ a owl:Restriction ;
            owl:allValuesFrom tun:TunnelConstructiveElement ;
            owl:onProperty tun:tunnelConstructiveElement ],
        [ a owl:Restriction ;
            owl:allValuesFrom tun:HollowSpaceUsageValue ;
            owl:onProperty <https://www.opengis.net/ont/citygml/common/usage> ],
        con:AbstractConstruction .

tun:HollowSpaceFunctionValue a owl:Class ;
    rdfs:label "HollowSpaceFunctionValue"@en ;
    rdfs:subClassOf skos:Concept ;
    skos:definition "HollowSpaceFunctionValue is a code list that enumerates the different purposes of a HollowSpace."@en .

tun:HollowSpaceUsageValue a owl:Class ;
    rdfs:label "HollowSpaceUsageValue"@en ;
    rdfs:subClassOf skos:Concept ;
    skos:definition "HollowSpaceUsageValue is a code list that enumerates the different uses of a HollowSpace."@en .

<https://www.opengis.net/ont/citygml/common/class> rdfs:label "class"@en ;
    skos:definition "Indicates the specific type of the HollowSpace."@en ;
    schema:rangeIncludes tun:HollowSpaceClassValue .

tun:HollowSpaceClassValue a owl:Class ;
    rdfs:label "HollowSpaceClassValue"@en ;
    rdfs:subClassOf skos:Concept ;
    skos:definition "HollowSpaceClassValue is a code list used to further classify a HollowSpace."@en .

@prefix core: <https://www.opengis.net/ont/citygml/core/> .
@prefix iso19150-2: <http://def.isotc211.org/iso19150/-2/2012/base#> .
@prefix owl: <http://www.w3.org/2002/07/owl#> .
@prefix rdfs: <http://www.w3.org/2000/01/rdf-schema#> .
@prefix sc: <http://shapechange.net/resources/ont/base#> .
@prefix schema: <https://schema.org/> .
@prefix skos: <http://www.w3.org/2004/02/skos/core#> .
@prefix veg: <https://www.opengis.net/ont/citygml/vegetation/> .
@prefix xsd: <http://www.w3.org/2001/XMLSchema#> .

<https://www.opengis.net/ont/citygml/vegetation> a owl:Ontology ;
    rdfs:label "Vegetation"@en ;
    owl:imports <http://def.isotc211.org/iso19150/-2/2012/base>,
        <http://shapechange.net/resources/ont/base>,
        <https://www.opengis.net/ont/citygml/common>,
        <https://www.opengis.net/ont/citygml/core> ;
    owl:versionIRI <https://www.opengis.net/ont/citygml/vegetation/3.0.0/> ;
    owl:versionInfo "3.0.0" ;
    skos:definition "The Vegetation module supports representation of vegetation objects with vegetation-specific thematic classes. CityGML’s vegetation model distinguishes between solitary vegetation objects like trees, and vegetation areas which represent biotopes like forests or other plant communities."@en .

veg:PlantCover a owl:Class ;
    rdfs:label "PlantCover"@en ;
    rdfs:subClassOf [ a owl:Restriction ;
            owl:maxQualifiedCardinality "1"^^xsd:nonNegativeInteger ;
            owl:onDataRange sc:Measure ;
            owl:onProperty veg:averageHeight ],
        [ a owl:Restriction ;
            owl:allValuesFrom sc:Measure ;
            owl:onProperty veg:maxHeight ],
        [ a owl:Restriction ;
            owl:maxQualifiedCardinality "1"^^xsd:nonNegativeInteger ;
            owl:onDataRange sc:Measure ;
            owl:onProperty veg:minHeight ],
        [ a owl:Restriction ;
            owl:allValuesFrom sc:Measure ;
            owl:onProperty veg:minHeight ],
        [ a owl:Restriction ;
            owl:allValuesFrom sc:Measure ;
            owl:onProperty veg:averageHeight ],
        [ a owl:Restriction ;
            owl:allValuesFrom veg:PlantCoverFunctionValue ;
            owl:onProperty <https://www.opengis.net/ont/citygml/common/function> ],
        [ a owl:Restriction ;
            owl:allValuesFrom veg:PlantCoverUsageValue ;
            owl:onProperty <https://www.opengis.net/ont/citygml/common/usage> ],
        [ a owl:Restriction ;
            owl:allValuesFrom veg:PlantCoverClassValue ;
            owl:onProperty <https://www.opengis.net/ont/citygml/common/class> ],
        [ a owl:Restriction ;
            owl:maxQualifiedCardinality "1"^^xsd:nonNegativeInteger ;
            owl:onDataRange sc:Measure ;
            owl:onProperty veg:maxHeight ],
        [ a owl:Restriction ;
            owl:maxQualifiedCardinality "1"^^xsd:nonNegativeInteger ;
            owl:onClass veg:PlantCoverClassValue ;
            owl:onProperty <https://www.opengis.net/ont/citygml/common/class> ],
        veg:AbstractVegetationObject ;
    owl:disjointWith veg:SolitaryVegetationObject .

veg:SolitaryVegetationObjectClassValue a owl:Class ;
    rdfs:label "SolitaryVegetationObjectClassValue"@en ;
    rdfs:subClassOf skos:Concept ;
    skos:definition "SolitaryVegetationObjectClassValue is a code list used to further classify a SolitaryVegetationObject."@en .

veg:SolitaryVegetationObjectFunctionValue a owl:Class ;
    rdfs:label "SolitaryVegetationObjectFunctionValue"@en ;
    rdfs:subClassOf skos:Concept ;
    skos:definition "SolitaryVegetationObjectFunctionValue is a code list that enumerates the different purposes of a SolitaryVegetationObject."@en .

veg:SolitaryVegetationObjectUsageValue a owl:Class ;
    rdfs:label "SolitaryVegetationObjectUsageValue"@en ;
    rdfs:subClassOf skos:Concept ;
    skos:definition "SolitaryVegetationObjectUsageValue is a code list that enumerates the different uses of a SolitaryVegetationObject."@en .

veg:SolitaryVegetationObject a owl:Class ;
    rdfs:label "SolitaryVegetationObject"@en ;
    rdfs:subClassOf [ a owl:Restriction ;
            owl:maxQualifiedCardinality "1"^^xsd:nonNegativeInteger ;
            owl:onDataRange sc:Measure ;
            owl:onProperty veg:crownDiameter ],
        [ a owl:Restriction ;
            owl:allValuesFrom veg:PlantCoverClassValue ;
            owl:onProperty <https://www.opengis.net/ont/citygml/common/class> ],
        [ a owl:Restriction ;
            owl:allValuesFrom veg:SpeciesValue ;
            owl:onProperty veg:species ],
        [ a owl:Restriction ;
            owl:allValuesFrom sc:Measure ;
            owl:onProperty veg:crownDiameter ],
        [ a owl:Restriction ;
            owl:maxQualifiedCardinality "1"^^xsd:nonNegativeInteger ;
            owl:onDataRange sc:Measure ;
            owl:onProperty veg:height ],
        [ a owl:Restriction ;
            owl:allValuesFrom veg:PlantCoverUsageValue ;
            owl:onProperty <https://www.opengis.net/ont/citygml/common/usage> ],
        [ a owl:Restriction ;
            owl:allValuesFrom sc:Measure ;
            owl:onProperty veg:maxRootBallDepth ],
        [ a owl:Restriction ;
            owl:maxQualifiedCardinality "1"^^xsd:nonNegativeInteger ;
            owl:onClass veg:PlantCoverClassValue ;
            owl:onProperty <https://www.opengis.net/ont/citygml/common/class> ],
        [ a owl:Restriction ;
            owl:allValuesFrom sc:Measure ;
            owl:onProperty veg:trunkDiameter ],
        [ a owl:Restriction ;
            owl:allValuesFrom sc:Measure ;
            owl:onProperty veg:rootBallDiameter ],
        [ a owl:Restriction ;
            owl:maxQualifiedCardinality "1"^^xsd:nonNegativeInteger ;
            owl:onDataRange sc:Measure ;
            owl:onProperty veg:maxRootBallDepth ],
        [ a owl:Restriction ;
            owl:maxQualifiedCardinality "1"^^xsd:nonNegativeInteger ;
            owl:onDataRange sc:Measure ;
            owl:onProperty veg:rootBallDiameter ],
        [ a owl:Restriction ;
            owl:allValuesFrom sc:Measure ;
            owl:onProperty veg:height ],
        [ a owl:Restriction ;
            owl:allValuesFrom veg:PlantCoverFunctionValue ;
            owl:onProperty <https://www.opengis.net/ont/citygml/common/function> ],
        [ a owl:Restriction ;
            owl:maxQualifiedCardinality "1"^^xsd:nonNegativeInteger ;
            owl:onClass veg:SpeciesValue ;
            owl:onProperty veg:species ],
        [ a owl:Restriction ;
            owl:maxQualifiedCardinality "1"^^xsd:nonNegativeInteger ;
            owl:onDataRange sc:Measure ;
            owl:onProperty veg:trunkDiameter ],
        veg:AbstractVegetationObject .

<https://www.opengis.net/ont/citygml/common/function> rdfs:label "function"@en ;
    skos:definition "Specifies the intended purposes of the PlantCover."@en ;
    schema:rangeIncludes veg:PlantCoverFunctionValue .

<https://www.opengis.net/ont/citygml/common/usage> rdfs:label "usage"@en ;
    skos:definition "Specifies the actual uses of the PlantCover."@en ;
    schema:rangeIncludes veg:PlantCoverUsageValue .

veg:AbstractVegetationObject a owl:Class ;
    rdfs:label "AbstractVegetationObject"@en ;
    iso19150-2:isAbstract true ;
    rdfs:subClassOf core:AbstractOccupiedSpace .

veg:averageHeight a owl:DatatypeProperty ;
    rdfs:label "averageHeight"@en ;
    rdfs:range sc:Measure ;
    skos:definition "Specifies the average height of the PlantCover."@en .

veg:crownDiameter a owl:DatatypeProperty ;
    rdfs:label "crownDiameter"@en ;
    rdfs:range sc:Measure ;
    skos:definition "Specifies the diameter of the SolitaryCityObject's crown."@en .

veg:height a owl:DatatypeProperty ;
    rdfs:label "height"@en ;
    rdfs:range sc:Measure ;
    skos:definition "Distance between the highest point of the vegetation object and the lowest point of the terrain at the bottom of the object."@en .

veg:maxHeight a owl:DatatypeProperty ;
    rdfs:label "maxHeight"@en ;
    rdfs:range sc:Measure ;
    skos:definition "Specifies the maximum height of the PlantCover."@en .

veg:maxRootBallDepth a owl:DatatypeProperty ;
    rdfs:label "maxRootBallDepth"@en ;
    rdfs:range sc:Measure ;
    skos:definition "Specifies the vertical distance between the lowest point of the SolitaryVegetationObject's root ball and the terrain surface."@en .

veg:minHeight a owl:DatatypeProperty ;
    rdfs:label "minHeight"@en ;
    rdfs:range sc:Measure ;
    skos:definition "Specifies the minimum height of the PlantCover."@en .

veg:rootBallDiameter a owl:DatatypeProperty ;
    rdfs:label "rootBallDiameter"@en ;
    rdfs:range sc:Measure ;
    skos:definition "Specifies the diameter of the SolitaryCityObject's root ball."@en .

veg:species a owl:ObjectProperty ;
    rdfs:label "species"@en ;
    rdfs:range veg:SpeciesValue ;
    skos:definition "Indicates the botanical name of the SolitaryVegetationObject."@en .

veg:trunkDiameter a owl:DatatypeProperty ;
    rdfs:label "trunkDiameter"@en ;
    rdfs:range sc:Measure ;
    skos:definition "Specifies the diameter of the SolitaryCityObject's trunk."@en .

veg:PlantCoverFunctionValue a owl:Class ;
    rdfs:label "PlantCoverFunctionValue"@en ;
    rdfs:subClassOf skos:Concept ;
    skos:definition "PlantCoverFunctionValue is a code list that enumerates the different purposes of a PlantCover."@en .

veg:PlantCoverUsageValue a owl:Class ;
    rdfs:label "PlantCoverUsageValue"@en ;
    rdfs:subClassOf skos:Concept ;
    skos:definition "PlantCoverUsageValue is a code list that enumerates the different uses of a PlantCover."@en .

veg:SpeciesValue a owl:Class ;
    rdfs:label "SpeciesValue"@en ;
    rdfs:subClassOf skos:Concept ;
    skos:definition "A SpeciesValue is a code list that enumerates the species of a SolitaryVegetationObject."@en .

<https://www.opengis.net/ont/citygml/common/class> rdfs:label "class"@en ;
    skos:definition "Indicates the specific type of the PlantCover."@en ;
    schema:rangeIncludes veg:PlantCoverClassValue .

veg:PlantCoverClassValue a owl:Class ;
    rdfs:label "PlantCoverClassValue"@en ;
    rdfs:subClassOf skos:Concept ;
    skos:definition "PlantCoverClassValue is a code list used to further classify a PlantCover."@en .

@prefix core: <https://www.opengis.net/ont/citygml/core/> .
@prefix owl: <http://www.w3.org/2002/07/owl#> .
@prefix rdf: <http://www.w3.org/1999/02/22-rdf-syntax-ns#> .
@prefix rdfs: <http://www.w3.org/2000/01/rdf-schema#> .
@prefix schema: <https://schema.org/> .
@prefix skos: <http://www.w3.org/2004/02/skos/core#> .
@prefix vers: <https://www.opengis.net/ont/citygml/versioning/> .
@prefix xsd: <http://www.w3.org/2001/XMLSchema#> .

<https://www.opengis.net/ont/citygml/versioning> a owl:Ontology ;
    rdfs:label "Versioning"@en ;
    owl:imports <http://def.isotc211.org/iso19150/-2/2012/base>,
        <https://www.opengis.net/ont/citygml/common>,
        <https://www.opengis.net/ont/citygml/core> ;
    owl:versionIRI <https://www.opengis.net/ont/citygml/versioning/3.0.0/> ;
    owl:versionInfo "3.0.0" ;
    skos:definition "The Versioning module supports representation of multiple versions of CityGML features within a single CityGML model. In addition, also the version transitions and transactions that lead to the different versions can be represented."@en .

vers:TransactionTypeValue a owl:Class ;
    rdfs:label "TransactionTypeValue"@en ;
    rdfs:subClassOf skos:Concept ;
    owl:equivalentClass [ a rdfs:Datatype ;
            owl:oneOf ( "insert" "delete" "replace" ) ] ;
    skos:definition "TransactionTypeValue enumerates the three possible types of transactions: insert, delete, or replace."@en .

<https://www.opengis.net/ont/citygml/common/versionMember> skos:definition "Relates to all city objects that are part of the city model version."@en ;
    schema:domainIncludes vers:Version ;
    schema:rangeIncludes core:AbstractFeatureWithLifespan .

vers:tag a owl:DatatypeProperty ;
    rdfs:label "tag"@en ;
    rdfs:range xsd:string ;
    skos:definition "Allows for adding keywords to the city model version."@en .

vers:transaction a owl:ObjectProperty ;
    rdfs:label "transaction"@en ;
    rdfs:domain vers:VersionTransition ;
    rdfs:range vers:Transaction ;
    skos:definition "Relates to all transactions that have been applied as part of the VersionTransition."@en .

vers:clonePredecessor a owl:DatatypeProperty ;
    rdfs:label "clonePredecessor"@en ;
    rdfs:range xsd:boolean ;
    skos:definition "Indicates whether the set of city object instances belonging to the successor version of the city model is either explicitly enumerated within the successor version object (attribute clonePredecessor=false),  or has to be derived from the modifications of the city model provided as a list of transactions on the city object versions contained in the predecessor version (attribute clonePredecessor=true)."@en .

vers:from a owl:ObjectProperty ;
    rdfs:label "from"@en ;
    rdfs:domain vers:VersionTransition ;
    rdfs:range vers:Version ;
    skos:definition "Relates to the predecessor version of the VersionTransition."@en .

vers:newFeature a owl:ObjectProperty ;
    rdfs:label "newFeature"@en ;
    rdfs:domain vers:Transaction ;
    rdfs:range core:AbstractFeatureWithLifespan ;
    skos:definition "Relates to the version of the city object subsequent to the Transaction."@en .

vers:oldFeature a owl:ObjectProperty ;
    rdfs:label "oldFeature"@en ;
    rdfs:domain vers:Transaction ;
    rdfs:range core:AbstractFeatureWithLifespan ;
    skos:definition "Relates to the version of the city object prior to the Transaction."@en .

vers:reason a owl:DatatypeProperty ;
    rdfs:label "reason"@en ;
    rdfs:range xsd:string ;
    skos:definition "Specifies why the VersionTransition has been carried out."@en .

vers:to a owl:ObjectProperty ;
    rdfs:label "to"@en ;
    rdfs:domain vers:VersionTransition ;
    rdfs:range vers:Version ;
    skos:definition "Relates to the successor version of the VersionTransition."@en .

vers:VersionTransition a owl:Class ;
    rdfs:label "VersionTransition"@en ;
    rdfs:subClassOf [ a owl:Restriction ;
            owl:allValuesFrom xsd:boolean ;
            owl:onProperty vers:clonePredecessor ],
        [ a owl:Restriction ;
            owl:allValuesFrom xsd:string ;
            owl:onProperty vers:reason ],
        [ a owl:Restriction ;
            owl:allValuesFrom vers:Transaction ;
            owl:onProperty vers:transaction ],
        [ a owl:Restriction ;
            owl:maxQualifiedCardinality "1"^^xsd:nonNegativeInteger ;
            owl:onDataRange xsd:string ;
            owl:onProperty vers:reason ],
        [ a owl:Restriction ;
            owl:onDataRange xsd:boolean ;
            owl:onProperty vers:clonePredecessor ;
            owl:qualifiedCardinality "1"^^xsd:nonNegativeInteger ],
        [ a owl:Restriction ;
            owl:allValuesFrom vers:TransitionTypeValue ;
            owl:onProperty vers:type ],
        [ a owl:Restriction ;
            owl:maxQualifiedCardinality "1"^^xsd:nonNegativeInteger ;
            owl:onClass vers:Version ;
            owl:onProperty vers:from ],
        [ a owl:Restriction ;
            owl:maxQualifiedCardinality "1"^^xsd:nonNegativeInteger ;
            owl:onDataRange vers:TransitionTypeValue ;
            owl:onProperty vers:type ],
        [ a owl:Restriction ;
            owl:allValuesFrom vers:Version ;
            owl:onProperty vers:to ],
        [ a owl:Restriction ;
            owl:maxQualifiedCardinality "1"^^xsd:nonNegativeInteger ;
            owl:onClass vers:Version ;
            owl:onProperty vers:to ],
        [ a owl:Restriction ;
            owl:allValuesFrom vers:Version ;
            owl:onProperty vers:from ],
        core:AbstractVersionTransition .

vers:Transaction a owl:Class ;
    rdfs:label "Transaction"@en ;
    rdfs:subClassOf [ a owl:Restriction ;
            owl:allValuesFrom core:AbstractFeatureWithLifespan ;
            owl:onProperty vers:newFeature ],
        [ a owl:Restriction ;
            owl:maxQualifiedCardinality "1"^^xsd:nonNegativeInteger ;
            owl:onClass core:AbstractFeatureWithLifespan ;
            owl:onProperty vers:newFeature ],
        [ a owl:Restriction ;
            owl:allValuesFrom core:AbstractFeatureWithLifespan ;
            owl:onProperty vers:oldFeature ],
        [ a owl:Restriction ;
            owl:maxQualifiedCardinality "1"^^xsd:nonNegativeInteger ;
            owl:onClass core:AbstractFeatureWithLifespan ;
            owl:onProperty vers:oldFeature ],
        [ a owl:Restriction ;
            owl:allValuesFrom vers:TransitionTypeValue ;
            owl:onProperty vers:type ],
        [ a owl:Restriction ;
            owl:onDataRange vers:TransitionTypeValue ;
            owl:onProperty vers:type ;
            owl:qualifiedCardinality "1"^^xsd:nonNegativeInteger ] ;
    skos:definition "Transaction represents a modification of the city model by the creation, termination, or replacement of a specific city object. While the creation of a city object also marks its first object version, the termination marks the end of existence of a real world object and, hence, also terminates the final version of a city object. The replacement of a city object means that a specific version of it is replaced by a new version."@en .

vers:type a owl:DatatypeProperty ;
    rdfs:label "type"@en ;
    rdfs:range vers:TransitionTypeValue ;
    skos:definition "Indicates the specific type of the VersionTransition."@en .

vers:TransitionTypeValue a rdfs:Datatype ;
    rdfs:label "TransitionTypeValue"@en ;
    owl:equivalentClass [ a rdfs:Datatype ;
            owl:oneOf ( "planned" "realized" "historicalSuccession" "fork" "merge" ) ] ;
    skos:definition "TransitionTypeValue enumerates the different kinds of version transitions. “planned” and “fork” should be used in cases when from one city model version multiple successor versions are being created. “realized” and “merge” should be used when different city model versions are converging into a common successor version."@en .

vers:Version a owl:Class ;
    rdfs:label "Version"@en ;
    rdfs:subClassOf [ a owl:Restriction ;
            owl:allValuesFrom core:AbstractFeatureWithLifespan ;
            owl:onProperty <https://www.opengis.net/ont/citygml/common/versionMember> ],
        [ a owl:Restriction ;
            owl:allValuesFrom xsd:string ;
            owl:onProperty vers:tag ],
        core:AbstractVersion .

@prefix core: <https://www.opengis.net/ont/citygml/core/> .
@prefix iso19150-2: <http://def.isotc211.org/iso19150/-2/2012/base#> .
@prefix owl: <http://www.w3.org/2002/07/owl#> .
@prefix rdfs: <http://www.w3.org/2000/01/rdf-schema#> .
@prefix schema: <https://schema.org/> .
@prefix skos: <http://www.w3.org/2004/02/skos/core#> .
@prefix wtr: <https://www.opengis.net/ont/citygml/waterbody/> .
@prefix xsd: <http://www.w3.org/2001/XMLSchema#> .

<https://www.opengis.net/ont/citygml/waterbody> a owl:Ontology ;
    rdfs:label "WaterBody"@en ;
    owl:imports <http://def.isotc211.org/iso19150/-2/2012/base>,
        <https://www.opengis.net/ont/citygml/common>,
        <https://www.opengis.net/ont/citygml/core> ;
    owl:versionIRI <https://www.opengis.net/ont/citygml/waterbody/3.0.0/> ;
    owl:versionInfo "3.0.0" ;
    skos:definition "The WaterBody module supports representation of the thematic aspects and 3D geometry of rivers, canals, lakes, and basins. It does, however, not inherit any hydrological or other dynamic aspects of fluid flow."@en .

wtr:WaterGroundSurface a owl:Class ;
    rdfs:label "WaterGroundSurface"@en ;
    rdfs:subClassOf wtr:AbstractWaterBoundarySurface ;
    owl:disjointWith wtr:WaterSurface .

<https://www.opengis.net/ont/citygml/common/boundary> schema:domainIncludes wtr:WaterBody ;
    schema:rangeIncludes wtr:AbstractWaterBoundarySurface .

<https://www.opengis.net/ont/citygml/common/function> rdfs:label "function"@en ;
    skos:definition "Specifies the intended purposes of the WaterBody."@en ;
    schema:rangeIncludes wtr:WaterBodyFunctionValue .

<https://www.opengis.net/ont/citygml/common/usage> rdfs:label "usage"@en ;
    skos:definition "Specifies the actual uses of the WaterBody."@en ;
    schema:rangeIncludes wtr:WaterBodyUsageValue .

wtr:WaterBody a owl:Class ;
    rdfs:label "WaterBody"@en ;
    rdfs:subClassOf [ a owl:Restriction ;
            owl:allValuesFrom wtr:AbstractWaterBoundarySurface ;
            owl:onProperty <https://www.opengis.net/ont/citygml/common/boundary> ],
        [ a owl:Restriction ;
            owl:allValuesFrom wtr:WaterBodyUsageValue ;
            owl:onProperty <https://www.opengis.net/ont/citygml/common/usage> ],
        [ a owl:Restriction ;
            owl:allValuesFrom wtr:WaterBodyClassValue ;
            owl:onProperty <https://www.opengis.net/ont/citygml/common/class> ],
        [ a owl:Restriction ;
            owl:maxQualifiedCardinality "1"^^xsd:nonNegativeInteger ;
            owl:onClass wtr:WaterBodyClassValue ;
            owl:onProperty <https://www.opengis.net/ont/citygml/common/class> ],
        [ a owl:Restriction ;
            owl:allValuesFrom wtr:WaterBodyFunctionValue ;
            owl:onProperty <https://www.opengis.net/ont/citygml/common/function> ],
        core:AbstractOccupiedSpace .

wtr:WaterSurface a owl:Class ;
    rdfs:label "WaterSurface"@en ;
    rdfs:subClassOf [ a owl:Restriction ;
            owl:allValuesFrom wtr:WaterLevelValue ;
            owl:onProperty wtr:waterLevel ],
        [ a owl:Restriction ;
            owl:maxQualifiedCardinality "1"^^xsd:nonNegativeInteger ;
            owl:onClass wtr:WaterLevelValue ;
            owl:onProperty wtr:waterLevel ],
        wtr:AbstractWaterBoundarySurface .

<https://www.opengis.net/ont/citygml/common/class> rdfs:label "class"@en ;
    skos:definition "Indicates the specific type of the WaterBody."@en ;
    schema:rangeIncludes wtr:WaterBodyClassValue .

wtr:WaterBodyFunctionValue a owl:Class ;
    rdfs:label "WaterBodyFunctionValue"@en ;
    rdfs:subClassOf skos:Concept ;
    skos:definition "WaterBodyFunctionValue is a code list that enumerates the different purposes of a WaterBody."@en .

wtr:WaterBodyUsageValue a owl:Class ;
    rdfs:label "WaterBodyUsageValue"@en ;
    rdfs:subClassOf skos:Concept ;
    skos:definition "WaterBodyUsageValue is a code list that enumerates the different uses of a WaterBody."@en .

wtr:waterLevel a owl:ObjectProperty ;
    rdfs:label "waterLevel"@en ;
    rdfs:range wtr:WaterLevelValue ;
    skos:definition "Specifies the level of the WaterSurface."@en .

wtr:WaterBodyClassValue a owl:Class ;
    rdfs:label "WaterBodyClassValue"@en ;
    rdfs:subClassOf skos:Concept ;
    skos:definition "WaterBodyClassValue is a code list used to further classify a WaterBody."@en .

wtr:WaterLevelValue a owl:Class ;
    rdfs:label "WaterLevelValue"@en ;
    rdfs:subClassOf skos:Concept ;
    skos:definition "WaterLevelValue is a code list that enumerates the different levels of a water surface."@en .

wtr:AbstractWaterBoundarySurface a owl:Class ;
    rdfs:label "AbstractWaterBoundarySurface"@en ;
    iso19150-2:isAbstract true ;
    rdfs:subClassOf core:AbstractThematicSurface .

@prefix core: <https://www.opengis.net/ont/citygml/core/> .
@prefix owl: <http://www.w3.org/2002/07/owl#> .
@prefix rdfs: <http://www.w3.org/2000/01/rdf-schema#> .
@prefix schema: <https://schema.org/> .
@prefix skos: <http://www.w3.org/2004/02/skos/core#> .
@prefix vers: <https://www.opengis.net/ont/citygml/versioning/> .
@prefix wksp: <https://www.opengis.net/ont/citygml/workspace/> .
@prefix xsd: <http://www.w3.org/2001/XMLSchema#> .

<https://www.opengis.net/ont/citygml/workspace> a owl:Ontology ;
    rdfs:label "Workspace"@en ;
    owl:imports <http://def.isotc211.org/iso19150/-2/2012/base>,
        <https://www.opengis.net/ont/citygml/common>,
        <https://www.opengis.net/ont/citygml/core>,
        <https://www.opengis.net/ont/citygml/versioning> ;
    owl:versionIRI <https://www.opengis.net/ont/citygml/workspace/3.0.0/> ;
    owl:versionInfo "3.0.0" ;
    skos:definition "This pattern provides a starting point for modeling a GML Application Schema which is a specialized xml schema that uses the Geographic Markup Language to model Features to provide the basis for interoperability within a community of interest."@en .

wksp:ConcensusSpace a owl:Class ;
    rdfs:label "ConcensusSpace"@en ;
    rdfs:subClassOf wksp:Space ;
    owl:disjointWith wksp:PropositionSpace .

<https://www.opengis.net/ont/citygml/common/versionMember> schema:domainIncludes wksp:Scenario ;
    schema:rangeIncludes vers:Version .

wksp:PropositionSpace a owl:Class ;
    rdfs:label "PropositionSpace"@en ;
    rdfs:subClassOf wksp:Space .

wksp:Workspace a owl:Class ;
    rdfs:label "Workspace"@en ;
    rdfs:subClassOf [ a owl:Restriction ;
            owl:allValuesFrom wksp:Space ;
            owl:onProperty wksp:spaceMember ],
        [ a owl:Restriction ;
            owl:maxQualifiedCardinality "2"^^xsd:nonNegativeInteger ;
            owl:onClass wksp:Space ;
            owl:onProperty wksp:spaceMember ],
        [ a owl:Restriction ;
            owl:minQualifiedCardinality "1"^^xsd:nonNegativeInteger ;
            owl:onClass wksp:Space ;
            owl:onProperty wksp:spaceMember ],
        [ a owl:Restriction ;
            owl:allValuesFrom xsd:string ;
            owl:onProperty wksp:creator ],
        core:AbstractFeatureWithLifespan .

wksp:versionTransitionMember a owl:ObjectProperty ;
    rdfs:label "versionTransitionMember"@en ;
    rdfs:domain wksp:Scenario ;
    rdfs:range vers:VersionTransition .

wksp:scenarioMember a owl:ObjectProperty ;
    rdfs:label "scenarioMember"@en ;
    rdfs:domain wksp:Space ;
    rdfs:range wksp:Scenario .

wksp:creator a owl:DatatypeProperty ;
    rdfs:label "creator"@en ;
    rdfs:range xsd:string .

wksp:spaceMember a owl:ObjectProperty ;
    rdfs:label "spaceMember"@en ;
    rdfs:domain wksp:Workspace ;
    rdfs:range wksp:Space .

wksp:Scenario a owl:Class ;
    rdfs:label "Scenario"@en ;
    rdfs:subClassOf [ a owl:Restriction ;
            owl:allValuesFrom vers:VersionTransition ;
            owl:onProperty wksp:versionTransitionMember ],
        [ a owl:Restriction ;
            owl:allValuesFrom vers:Version ;
            owl:onProperty <https://www.opengis.net/ont/citygml/common/versionMember> ],
        [ a owl:Restriction ;
            owl:allValuesFrom xsd:string ;
            owl:onProperty wksp:creator ],
        core:AbstractFeatureWithLifespan .

wksp:Space a owl:Class ;
    rdfs:label "Space"@en ;
    rdfs:subClassOf [ a owl:Restriction ;
            owl:minQualifiedCardinality "1"^^xsd:nonNegativeInteger ;
            owl:onClass wksp:Scenario ;
            owl:onProperty wksp:scenarioMember ],
        [ a owl:Restriction ;
            owl:allValuesFrom xsd:string ;
            owl:onProperty wksp:creator ],
        [ a owl:Restriction ;
            owl:allValuesFrom wksp:Scenario ;
            owl:onProperty wksp:scenarioMember ],
        core:AbstractFeatureWithLifespan .

